<?xml version="1.0" encoding="UTF-8"?>
<rdf:RDF 
         xml:base="http://www.geonames.org/ontology"
         xmlns:skos="http://www.w3.org/2004/02/skos/core#"
         xmlns:gn="http://www.geonames.org/ontology#"
         xmlns:owl="http://www.w3.org/2002/07/owl#"
         xmlns:rdf="http://www.w3.org/1999/02/22-rdf-syntax-ns#"
         xmlns:rdfs="http://www.w3.org/2000/01/rdf-schema#"
         xmlns:dcterms="http://purl.org/dc/terms/"
         xmlns:foaf="http://xmlns.com/foaf/0.1/">

<!-- Ontology Information -->
  <owl:Ontology rdf:about="http://www.geonames.org/ontology">
    <rdfs:label xml:lang="en">Geonames ontology</rdfs:label>
    <dcterms:isReferencedBy rdf:resource="http://www.geonames.org/ontology/documentation.html"/>
    <foaf:isPrimaryTopicOf rdf:resource="http://www.geonames.org/ontology/documentation.html"/>
    <rdfs:comment>Modifications from version 2.0 to 2.1 : 
      removed gn:inCountry ObjectProperty and gn:Country class, replaced by gn:countryCode DatatypeProperty.
      gn:name and gn:alternateName declared as subproperties of skos:prefLabel and skos:altLabel respectively, no more need for the "Full" ontology present in version 2.0.
      Updated list of feature codes. Mappings from codes to external resources (GEMET) are removed. 
      A further SKOS publication of feature codes will include status, dates, multilingual translations and mappings with other concept schemes.</rdfs:comment>
    <rdfs:comment>Modifications from version 2.1 to 2.21 : 
      added gn:shortName property. 
      gn:officialName is now a subproperty of skos:prefLabel .
      added gn:parentADM1, gn:parentADM2, gn:parentADM3, gn:parentADM4, gn:parentCountry properties, with respective range restrictions on feature codes.</rdfs:comment>
    <rdfs:comment>The recommended prefix for geonames ontology namespace is gn:</rdfs:comment>
    <rdfs:comment>WARNING : Version 2.2 should not be used - namespaces errors in the release, no backward compatibility</rdfs:comment>
    <owl:versionInfo xml:lang="en">Version 2.21 - 2010-10-05</owl:versionInfo>
  </owl:Ontology>

<!-- Classes -->
  <owl:Class rdf:about="http://www.geonames.org/ontology#Class">
    <rdfs:comment xml:lang="en">A class of features.</rdfs:comment>
    <rdfs:label xml:lang="en">Class</rdfs:label>
    <rdfs:subClassOf rdf:resource="http://www.w3.org/2004/02/skos/core#ConceptScheme"/>
  </owl:Class>

  <owl:Class rdf:about="http://www.geonames.org/ontology#Code">
    <rdfs:comment xml:lang="en">A feature code.</rdfs:comment>
    <rdfs:label xml:lang="en">Code</rdfs:label>
    <rdfs:subClassOf rdf:resource="http://www.w3.org/2004/02/skos/core#Concept"/>
  </owl:Class>

  <owl:Class rdf:about="http://www.geonames.org/ontology#Feature">
    <rdfs:comment xml:lang="en">A geographical object uniquely defined by its geonames id.</rdfs:comment>
    <rdfs:label xml:lang="en">Feature</rdfs:label>
    <rdfs:subClassOf rdf:resource="http://www.w3.org/2003/01/geo/wgs84_pos#SpatialThing"/>
    <rdfs:subClassOf>
      <owl:Restriction>
        <owl:cardinality rdf:datatype="http://www.w3.org/2001/XMLSchema#nonNegativeInteger">1</owl:cardinality>
        <owl:onProperty rdf:resource="http://www.geonames.org/ontology#featureClass"/>
      </owl:Restriction>
    </rdfs:subClassOf>
    <rdfs:subClassOf>
      <owl:Restriction>
        <owl:maxCardinality rdf:datatype="http://www.w3.org/2001/XMLSchema#nonNegativeInteger">1</owl:maxCardinality>
        <owl:onProperty rdf:resource="http://www.geonames.org/ontology#featureCode"/>
      </owl:Restriction>
    </rdfs:subClassOf>
  </owl:Class>

  <owl:Class rdf:about="http://www.geonames.org/ontology#Map">
    <rdfs:comment xml:lang="en">A Web page displaying a map</rdfs:comment>
    <rdfs:label xml:lang="en">Map</rdfs:label>
    <rdfs:subClassOf rdf:resource="http://xmlns.com/foaf/0.1/Document"/>
  </owl:Class>

  <owl:Class rdf:about="http://www.geonames.org/ontology#RDFData">
    <rdfs:comment xml:lang="en">A Document containing RDF description of one or several features.</rdfs:comment>
    <rdfs:label xml:lang="en">RDF Data</rdfs:label>
    <rdfs:subClassOf rdf:resource="http://xmlns.com/foaf/0.1/Document"/>
  </owl:Class>

  <owl:Class rdf:about="http://www.geonames.org/ontology#WikipediaArticle">
    <rdfs:comment xml:lang="en">A Wikipedia article</rdfs:comment>
    <rdfs:label xml:lang="en">Wikipedia Article</rdfs:label>
    <rdfs:subClassOf rdf:resource="http://xmlns.com/foaf/0.1/Document"/>
  </owl:Class>

  <owl:Class rdf:about="http://www.w3.org/2003/01/geo/wgs84_pos#SpatialThing"/>
  <owl:Class rdf:about="http://www.w3.org/2004/02/skos/core#Concept"/>
  <owl:Class rdf:about="http://www.w3.org/2004/02/skos/core#ConceptScheme"/>
  <owl:Class rdf:about="http://xmlns.com/foaf/0.1/Document"/>

<!-- Datatypes -->
  <rdfs:Datatype rdf:about="http://www.w3.org/2001/XMLSchema#integer"/>

<!-- Annotation Properties -->
  <owl:AnnotationProperty rdf:about="http://www.w3.org/2000/01/rdf-schema#comment"/>
  <owl:AnnotationProperty rdf:about="http://www.w3.org/2000/01/rdf-schema#label"/>
  <owl:AnnotationProperty rdf:about="http://www.w3.org/2002/07/owl#versionInfo"/>

<!-- Datatype Properties -->
  <owl:DatatypeProperty rdf:about="http://www.geonames.org/ontology#alternateName">
    <rdfs:subPropertyOf rdf:resource="http://www.w3.org/2004/02/skos/core#altLabel"/>
  </owl:DatatypeProperty>

  <owl:DatatypeProperty rdf:about="http://www.geonames.org/ontology#countryCode">
    <rdf:type rdf:resource="http://www.w3.org/2002/07/owl#FunctionalProperty"/>
    <rdfs:comment xml:lang="en">A two letters country code in the ISO 3166 list</rdfs:comment>
    <rdfs:comment xml:lang="en">The countryCode value for a Feature is equal to the countryCode value of the parentCountry value.</rdfs:comment>
    <rdfs:domain rdf:resource="http://www.geonames.org/ontology#Feature"/>
    <rdfs:label xml:lang="en">ISO country code</rdfs:label>
  </owl:DatatypeProperty>

  <owl:DatatypeProperty rdf:about="http://www.geonames.org/ontology#name">
    <rdf:type rdf:resource="http://www.w3.org/2002/07/owl#FunctionalProperty"/>
    <rdfs:comment xml:lang="en">The main international name of a feature. The value has no xml:lang tag.</rdfs:comment>
    <rdfs:subPropertyOf rdf:resource="http://www.w3.org/2000/01/rdf-schema#label"/>
    <rdfs:label xml:lang="en">name</rdfs:label>
  </owl:DatatypeProperty>

  <owl:DatatypeProperty rdf:about="http://www.geonames.org/ontology#officialName">
    <rdfs:comment xml:lang="en">A name in an official local language</rdfs:comment>
    <rdfs:domain rdf:resource="http://www.geonames.org/ontology#Feature"/>
    <rdfs:label xml:lang="en">official name</rdfs:label>
    <rdfs:subPropertyOf rdf:resource="http://www.w3.org/2004/02/skos/core#prefLabel"/>
  </owl:DatatypeProperty>

  <owl:DatatypeProperty rdf:about="http://www.geonames.org/ontology#population">
    <rdf:type rdf:resource="http://www.w3.org/2002/07/owl#FunctionalProperty"/>
    <rdfs:domain rdf:resource="http://www.geonames.org/ontology#Feature"/>
    <rdfs:label xml:lang="en">population</rdfs:label>
    <rdfs:range rdf:resource="http://www.w3.org/2001/XMLSchema#integer"/>
  </owl:DatatypeProperty>

  <owl:DatatypeProperty rdf:about="http://www.geonames.org/ontology#postalCode">
    <rdfs:domain rdf:resource="http://www.geonames.org/ontology#Feature"/>
    <rdfs:label xml:lang="en">postal code</rdfs:label>
  </owl:DatatypeProperty>

  <owl:DatatypeProperty rdf:about="http://www.geonames.org/ontology#shortName">
    <rdfs:domain rdf:resource="http://www.geonames.org/ontology#Feature"/>
    <rdfs:label xml:lang="en">short name</rdfs:label>
    <rdfs:subPropertyOf rdf:resource="http://www.geonames.org/ontology#alternateName"/>
  </owl:DatatypeProperty>

  <owl:DatatypeProperty rdf:about="http://www.w3.org/2004/02/skos/core#altLabel">
    <rdfs:label xml:lang="en">alternative label</rdfs:label>
  </owl:DatatypeProperty>

  <owl:DatatypeProperty rdf:about="http://www.w3.org/2004/02/skos/core#definition"/>
  <owl:DatatypeProperty rdf:about="http://www.w3.org/2004/02/skos/core#prefLabel">
    <rdfs:comment xml:lang="en">This attribute is used to represent a feature preferred label in a natural language. The generic geonames "name" is represented using rdfs:label</rdfs:comment>
    <rdfs:label xml:lang="en">preferred label</rdfs:label>
  </owl:DatatypeProperty>

<!-- Object Properties -->
  <owl:ObjectProperty rdf:about="http://purl.org/dc/terms/subject"/>
  <owl:FunctionalProperty rdf:about="http://www.geonames.org/ontology#childrenFeatures">
    <rdf:type rdf:resource="http://www.w3.org/2002/07/owl#ObjectProperty"/>
    <rdfs:comment xml:lang="en">Links to an RDF document containing the descriptions of children features</rdfs:comment>
    <rdfs:domain rdf:resource="http://www.geonames.org/ontology#Feature"/>
    <rdfs:label xml:lang="en">children features</rdfs:label>
    <rdfs:range rdf:resource="http://www.geonames.org/ontology#RDFData"/>
  </owl:FunctionalProperty>

  <owl:ObjectProperty rdf:about="http://www.geonames.org/ontology#featureClass">
    <rdfs:comment xml:lang="en">The main category of the feature, as defined in geonames taxonomy.</rdfs:comment>
    <rdfs:domain rdf:resource="http://www.geonames.org/ontology#Feature"/>
    <rdfs:label xml:lang="en">feature class</rdfs:label>
    <rdfs:range rdf:resource="http://www.geonames.org/ontology#Class"/>
    <rdfs:subPropertyOf rdf:resource="http://purl.org/dc/terms/subject"/>
  </owl:ObjectProperty>

  <owl:FunctionalProperty rdf:about="http://www.geonames.org/ontology#featureCode">
    <rdf:type rdf:resource="http://www.w3.org/2002/07/owl#ObjectProperty"/>
    <rdfs:comment xml:lang="en">Type of the feature, as defined in geonames taxonomy.</rdfs:comment>
    <rdfs:domain rdf:resource="http://www.geonames.org/ontology#Feature"/>
    <rdfs:label xml:lang="en">feature code</rdfs:label>
    <rdfs:range rdf:resource="http://www.geonames.org/ontology#Code"/>
    <rdfs:subPropertyOf rdf:resource="http://purl.org/dc/terms/subject"/>
  </owl:FunctionalProperty>

  <owl:ObjectProperty rdf:about="http://www.geonames.org/ontology#locatedIn">
    <rdfs:comment xml:lang="en">Indicates that the subject resource is located in the object feature</rdfs:comment>
    <rdfs:label xml:lang="en">located in</rdfs:label>
    <rdfs:range rdf:resource="http://www.geonames.org/ontology#Feature"/>
  </owl:ObjectProperty>

  <owl:ObjectProperty rdf:about="http://www.geonames.org/ontology#locationMap">
    <rdfs:comment xml:lang="en">A geonames map centered on the feature.</rdfs:comment>
    <rdfs:domain rdf:resource="http://www.geonames.org/ontology#Feature"/>
    <rdfs:label xml:lang="en">map</rdfs:label>
    <rdfs:range rdf:resource="http://www.geonames.org/ontology#Map"/>
  </owl:ObjectProperty>

  <owl:ObjectProperty rdf:about="http://www.geonames.org/ontology#nearby">
    <rdf:type rdf:resource="http://www.w3.org/2002/07/owl#SymmetricProperty"/>
    <rdfs:comment xml:lang="en">A feature close to the reference feature</rdfs:comment>
    <rdfs:domain rdf:resource="http://www.geonames.org/ontology#Feature"/>
    <rdfs:label xml:lang="en">nearby</rdfs:label>
    <rdfs:range rdf:resource="http://www.geonames.org/ontology#Feature"/>
  </owl:ObjectProperty>

  <owl:ObjectProperty rdf:about="http://www.geonames.org/ontology#nearbyFeatures">
    <rdfs:comment xml:lang="en">Links to an RDF document containing the descriptions of nearby features</rdfs:comment>
    <rdfs:domain rdf:resource="http://www.geonames.org/ontology#Feature"/>
    <rdfs:label xml:lang="en">nearby features</rdfs:label>
    <rdfs:range rdf:resource="http://www.geonames.org/ontology#RDFData"/>
  </owl:ObjectProperty>

  <owl:ObjectProperty rdf:about="http://www.geonames.org/ontology#neighbour">
    <rdf:type rdf:resource="http://www.w3.org/2002/07/owl#SymmetricProperty"/>
    <rdfs:comment xml:lang="en">A feature sharing a common boarder with the reference feature</rdfs:comment>
    <rdfs:domain rdf:resource="http://www.geonames.org/ontology#Feature"/>
    <rdfs:label xml:lang="en">neighbour</rdfs:label>
    <rdfs:range rdf:resource="http://www.geonames.org/ontology#Feature"/>
  </owl:ObjectProperty>

  <owl:ObjectProperty rdf:about="http://www.geonames.org/ontology#neighbouringFeatures">
    <rdfs:comment xml:lang="en">Links to an RDF document containing the descriptions of neighbouring features. Applies when the feature has definite boarders.</rdfs:comment>
    <rdfs:domain rdf:resource="http://www.geonames.org/ontology#Feature"/>
    <rdfs:label xml:lang="en">neighbouring features</rdfs:label>
    <rdfs:range rdf:resource="http://www.geonames.org/ontology#RDFData"/>
  </owl:ObjectProperty>

  <owl:FunctionalProperty rdf:about="http://www.geonames.org/ontology#parentADM1">
    <rdf:type rdf:resource="http://www.w3.org/2002/07/owl#ObjectProperty"/>
    <rdfs:domain rdf:resource="http://www.geonames.org/ontology#Feature"/>
    <rdfs:label xml:lang="en">level 1 administrative parent</rdfs:label>
    <rdfs:range>
      <owl:Restriction>
        <owl:hasValue rdf:resource="http://www.geonames.org/ontology#A.ADM1"/>
        <owl:onProperty rdf:resource="http://www.geonames.org/ontology#featureCode"/>
      </owl:Restriction>
    </rdfs:range>
    <rdfs:subPropertyOf rdf:resource="http://www.geonames.org/ontology#parentFeature"/>
  </owl:FunctionalProperty>

  <owl:FunctionalProperty rdf:about="http://www.geonames.org/ontology#parentADM2">
    <rdf:type rdf:resource="http://www.w3.org/2002/07/owl#ObjectProperty"/>
    <rdfs:domain rdf:resource="http://www.geonames.org/ontology#Feature"/>
    <rdfs:label xml:lang="en">level 2 administrative parent</rdfs:label>
    <rdfs:range>
      <owl:Restriction>
        <owl:hasValue rdf:resource="http://www.geonames.org/ontology#A.ADM2"/>
        <owl:onProperty rdf:resource="http://www.geonames.org/ontology#featureCode"/>
      </owl:Restriction>
    </rdfs:range>
    <rdfs:subPropertyOf rdf:resource="http://www.geonames.org/ontology#parentFeature"/>
  </owl:FunctionalProperty>

  <owl:FunctionalProperty rdf:about="http://www.geonames.org/ontology#parentADM3">
    <rdf:type rdf:resource="http://www.w3.org/2002/07/owl#ObjectProperty"/>
    <rdfs:domain rdf:resource="http://www.geonames.org/ontology#Feature"/>
    <rdfs:label xml:lang="en">level 3 administrative parent</rdfs:label>
    <rdfs:range>
      <owl:Restriction>
        <owl:hasValue rdf:resource="http://www.geonames.org/ontology#A.ADM3"/>
        <owl:onProperty rdf:resource="http://www.geonames.org/ontology#featureCode"/>
      </owl:Restriction>
    </rdfs:range>
    <rdfs:subPropertyOf rdf:resource="http://www.geonames.org/ontology#parentFeature"/>
  </owl:FunctionalProperty>

  <owl:FunctionalProperty rdf:about="http://www.geonames.org/ontology#parentADM4">
    <rdf:type rdf:resource="http://www.w3.org/2002/07/owl#ObjectProperty"/>
    <rdfs:domain rdf:resource="http://www.geonames.org/ontology#Feature"/>
    <rdfs:label xml:lang="en">level 4 administrative parent</rdfs:label>
    <rdfs:range>
      <owl:Restriction>
        <owl:hasValue rdf:resource="http://www.geonames.org/ontology#A.ADM4"/>
        <owl:onProperty rdf:resource="http://www.geonames.org/ontology#featureCode"/>
      </owl:Restriction>
    </rdfs:range>
    <rdfs:subPropertyOf rdf:resource="http://www.geonames.org/ontology#parentFeature"/>
  </owl:FunctionalProperty>

  <owl:FunctionalProperty rdf:about="http://www.geonames.org/ontology#parentCountry">
    <rdf:type rdf:resource="http://www.w3.org/2002/07/owl#ObjectProperty"/>
    <rdfs:domain rdf:resource="http://www.geonames.org/ontology#Feature"/>
    <rdfs:label xml:lang="en">parent country</rdfs:label>
    <rdfs:range>
      <owl:Restriction>
        <owl:hasValue rdf:resource="http://www.geonames.org/ontology#A.PCLI"/>
        <owl:onProperty rdf:resource="http://www.geonames.org/ontology#featureCode"/>
      </owl:Restriction>
    </rdfs:range>
    <rdfs:subPropertyOf rdf:resource="http://www.geonames.org/ontology#parentFeature"/>
  </owl:FunctionalProperty>

  <owl:ObjectProperty rdf:about="http://www.geonames.org/ontology#parentFeature">
    <rdf:type rdf:resource="http://www.w3.org/2002/07/owl#TransitiveProperty"/>
    <rdfs:comment xml:lang="en">A feature parent of the current one, in either administrative or physical subdivision.</rdfs:comment>
    <rdfs:domain rdf:resource="http://www.geonames.org/ontology#Feature"/>
    <rdfs:label xml:lang="en">parent feature</rdfs:label>
    <rdfs:range rdf:resource="http://www.geonames.org/ontology#Feature"/>
  </owl:ObjectProperty>

  <owl:ObjectProperty rdf:about="http://www.geonames.org/ontology#wikipediaArticle">
    <rdfs:comment xml:lang="en">A Wikipedia article of which subject is the resource.</rdfs:comment>
    <rdfs:domain rdf:resource="http://www.geonames.org/ontology#Feature"/>
    <rdfs:label xml:lang="en">wikipedia article</rdfs:label>
    <rdfs:range rdf:resource="http://www.geonames.org/ontology#WikipediaArticle"/>
  </owl:ObjectProperty>

  <owl:ObjectProperty rdf:about="http://www.w3.org/2004/02/skos/core#inScheme"/>

<!-- Instances -->
  <gn:Class rdf:about="http://www.geonames.org/ontology#A">
    <rdfs:comment xml:lang="en">country, state, region ...</rdfs:comment>
  </gn:Class>

  <gn:Code rdf:about="http://www.geonames.org/ontology#A.ADM1">
    <skos:definition xml:lang="en">a primary administrative division of a country, such as a state in the United States</skos:definition>
    <skos:inScheme rdf:resource="http://www.geonames.org/ontology#A"/>
    <skos:prefLabel xml:lang="en">first-order administrative division</skos:prefLabel>
  </gn:Code>

  <gn:Code rdf:about="http://www.geonames.org/ontology#A.ADM2">
    <skos:definition xml:lang="en">a subdivision of a first-order administrative division</skos:definition>
    <skos:inScheme rdf:resource="http://www.geonames.org/ontology#A"/>
    <skos:prefLabel xml:lang="en">second-order administrative division</skos:prefLabel>
  </gn:Code>

  <gn:Code rdf:about="http://www.geonames.org/ontology#A.ADM3">
    <skos:definition xml:lang="en">a subdivision of a second-order administrative division</skos:definition>
    <skos:inScheme rdf:resource="http://www.geonames.org/ontology#A"/>
    <skos:prefLabel xml:lang="en">third-order administrative division</skos:prefLabel>
  </gn:Code>

  <gn:Code rdf:about="http://www.geonames.org/ontology#A.ADM4">
    <skos:definition xml:lang="en">a subdivision of a third-order administrative division</skos:definition>
    <skos:inScheme rdf:resource="http://www.geonames.org/ontology#A"/>
    <skos:prefLabel xml:lang="en">fourth-order administrative division</skos:prefLabel>
  </gn:Code>

  <gn:Code rdf:about="http://www.geonames.org/ontology#A.ADMD">
    <skos:definition xml:lang="en">an administrative division of a country, undifferentiated as to administrative level</skos:definition>
    <skos:inScheme rdf:resource="http://www.geonames.org/ontology#A"/>
    <skos:prefLabel xml:lang="en">administrative division</skos:prefLabel>
  </gn:Code>

  <gn:Code rdf:about="http://www.geonames.org/ontology#A.LTER">
    <skos:definition xml:lang="en">a tract of land leased by the United Kingdom from the People's Republic of China to form part of Hong Kong</skos:definition>
    <skos:inScheme rdf:resource="http://www.geonames.org/ontology#A"/>
    <skos:prefLabel xml:lang="en">leased area</skos:prefLabel>
  </gn:Code>

  <gn:Code rdf:about="http://www.geonames.org/ontology#A.PCL">
    <skos:definition xml:lang="en">_</skos:definition>
    <skos:inScheme rdf:resource="http://www.geonames.org/ontology#A"/>
    <skos:prefLabel xml:lang="en">political entity</skos:prefLabel>
  </gn:Code>

  <gn:Code rdf:about="http://www.geonames.org/ontology#A.PCLD">
    <skos:definition xml:lang="en">_</skos:definition>
    <skos:inScheme rdf:resource="http://www.geonames.org/ontology#A"/>
    <skos:prefLabel xml:lang="en">dependent political entity</skos:prefLabel>
  </gn:Code>

  <gn:Code rdf:about="http://www.geonames.org/ontology#A.PCLF">
    <skos:definition xml:lang="en">_</skos:definition>
    <skos:inScheme rdf:resource="http://www.geonames.org/ontology#A"/>
    <skos:prefLabel xml:lang="en">freely associated state</skos:prefLabel>
  </gn:Code>

  <gn:Code rdf:about="http://www.geonames.org/ontology#A.PCLI">
    <skos:definition xml:lang="en">_</skos:definition>
    <skos:inScheme rdf:resource="http://www.geonames.org/ontology#A"/>
    <skos:prefLabel xml:lang="en">independent political entity</skos:prefLabel>
  </gn:Code>

  <gn:Code rdf:about="http://www.geonames.org/ontology#A.PCLIX">
    <skos:definition xml:lang="en">_</skos:definition>
    <skos:inScheme rdf:resource="http://www.geonames.org/ontology#A"/>
    <skos:prefLabel xml:lang="en">section of independent political entity</skos:prefLabel>
  </gn:Code>

  <gn:Code rdf:about="http://www.geonames.org/ontology#A.PCLS">
    <skos:definition xml:lang="en">_</skos:definition>
    <skos:inScheme rdf:resource="http://www.geonames.org/ontology#A"/>
    <skos:prefLabel xml:lang="en">semi-independent political entity</skos:prefLabel>
  </gn:Code>

  <gn:Code rdf:about="http://www.geonames.org/ontology#A.PRSH">
    <skos:definition xml:lang="en">an ecclesiastical district</skos:definition>
    <skos:inScheme rdf:resource="http://www.geonames.org/ontology#A"/>
    <skos:prefLabel xml:lang="en">parish</skos:prefLabel>
  </gn:Code>

  <gn:Code rdf:about="http://www.geonames.org/ontology#A.TERR">
    <skos:definition xml:lang="en">_</skos:definition>
    <skos:inScheme rdf:resource="http://www.geonames.org/ontology#A"/>
    <skos:prefLabel xml:lang="en">territory</skos:prefLabel>
  </gn:Code>

  <gn:Code rdf:about="http://www.geonames.org/ontology#A.ZN">
    <skos:definition xml:lang="en">_</skos:definition>
    <skos:inScheme rdf:resource="http://www.geonames.org/ontology#A"/>
    <skos:prefLabel xml:lang="en">zone</skos:prefLabel>
  </gn:Code>

  <gn:Code rdf:about="http://www.geonames.org/ontology#A.ZNB">
    <skos:definition xml:lang="en">a zone recognized as a buffer between two nations in which military presence is minimal or absent</skos:definition>
    <skos:inScheme rdf:resource="http://www.geonames.org/ontology#A"/>
    <skos:prefLabel xml:lang="en">buffer zone</skos:prefLabel>
  </gn:Code>

  <gn:Class rdf:about="http://www.geonames.org/ontology#H">
    <rdfs:comment xml:lang="en">stream, lake, ...</rdfs:comment>
  </gn:Class>

  <gn:Code rdf:about="http://www.geonames.org/ontology#H.AIRS">
    <skos:definition xml:lang="en">a place on a waterbody where floatplanes land and take off</skos:definition>
    <skos:inScheme rdf:resource="http://www.geonames.org/ontology#H"/>
    <skos:prefLabel xml:lang="en">seaplane landing area</skos:prefLabel>
  </gn:Code>

  <gn:Code rdf:about="http://www.geonames.org/ontology#H.ANCH">
    <skos:definition xml:lang="en">an area where vessels may anchor</skos:definition>
    <skos:inScheme rdf:resource="http://www.geonames.org/ontology#H"/>
    <skos:prefLabel xml:lang="en">anchorage</skos:prefLabel>
  </gn:Code>

  <gn:Code rdf:about="http://www.geonames.org/ontology#H.BAY">
    <skos:definition xml:lang="en">a coastal indentation between two capes or headlands, larger than a cove but smaller than a gulf</skos:definition>
    <skos:inScheme rdf:resource="http://www.geonames.org/ontology#H"/>
    <skos:prefLabel xml:lang="en">bay</skos:prefLabel>
  </gn:Code>

  <gn:Code rdf:about="http://www.geonames.org/ontology#H.BAYS">
    <skos:definition xml:lang="en">coastal indentations between two capes or headlands, larger than a cove but smaller than a gulf</skos:definition>
    <skos:inScheme rdf:resource="http://www.geonames.org/ontology#H"/>
    <skos:prefLabel xml:lang="en">bays</skos:prefLabel>
  </gn:Code>

  <gn:Code rdf:about="http://www.geonames.org/ontology#H.BGHT">
    <skos:definition xml:lang="en">an open body of water forming a slight recession in a coastline</skos:definition>
    <skos:inScheme rdf:resource="http://www.geonames.org/ontology#H"/>
    <skos:prefLabel xml:lang="en">bight(s)</skos:prefLabel>
  </gn:Code>

  <gn:Code rdf:about="http://www.geonames.org/ontology#H.BNK">
    <skos:definition xml:lang="en">an elevation, typically located on a shelf, over which the depth of water is relatively shallow but sufficient for most surface navigation</skos:definition>
    <skos:inScheme rdf:resource="http://www.geonames.org/ontology#H"/>
    <skos:prefLabel xml:lang="en">bank(s)</skos:prefLabel>
  </gn:Code>

  <gn:Code rdf:about="http://www.geonames.org/ontology#H.BNKR">
    <skos:definition xml:lang="en">a sloping margin of a stream channel which normally confines the stream to its channel on land</skos:definition>
    <skos:inScheme rdf:resource="http://www.geonames.org/ontology#H"/>
    <skos:prefLabel xml:lang="en">stream bank</skos:prefLabel>
  </gn:Code>

  <gn:Code rdf:about="http://www.geonames.org/ontology#H.BNKX">
    <skos:definition xml:lang="en">_</skos:definition>
    <skos:inScheme rdf:resource="http://www.geonames.org/ontology#H"/>
    <skos:prefLabel xml:lang="en">section of bank</skos:prefLabel>
  </gn:Code>

  <gn:Code rdf:about="http://www.geonames.org/ontology#H.BOG">
    <skos:definition xml:lang="en">a wetland characterized by peat forming sphagnum moss, sedge, and other acid-water plants</skos:definition>
    <skos:inScheme rdf:resource="http://www.geonames.org/ontology#H"/>
    <skos:prefLabel xml:lang="en">bog(s)</skos:prefLabel>
  </gn:Code>

  <gn:Code rdf:about="http://www.geonames.org/ontology#H.CAPG">
    <skos:definition xml:lang="en">a dome-shaped mass of glacial ice covering an area of mountain summits or other high lands; smaller than an ice sheet</skos:definition>
    <skos:inScheme rdf:resource="http://www.geonames.org/ontology#H"/>
    <skos:prefLabel xml:lang="en">icecap</skos:prefLabel>
  </gn:Code>

  <gn:Code rdf:about="http://www.geonames.org/ontology#H.CHN">
    <skos:definition xml:lang="en">the deepest part of a stream, bay, lagoon, or strait, through which the main current flows</skos:definition>
    <skos:inScheme rdf:resource="http://www.geonames.org/ontology#H"/>
    <skos:prefLabel xml:lang="en">channel</skos:prefLabel>
  </gn:Code>

  <gn:Code rdf:about="http://www.geonames.org/ontology#H.CHNL">
    <skos:definition xml:lang="en">that part of a lake having water deep enough for navigation between islands, shoals, etc.</skos:definition>
    <skos:inScheme rdf:resource="http://www.geonames.org/ontology#H"/>
    <skos:prefLabel xml:lang="en">lake channel(s)</skos:prefLabel>
  </gn:Code>

  <gn:Code rdf:about="http://www.geonames.org/ontology#H.CHNM">
    <skos:definition xml:lang="en">that part of a body of water deep enough for navigation through an area otherwise not suitable</skos:definition>
    <skos:inScheme rdf:resource="http://www.geonames.org/ontology#H"/>
    <skos:prefLabel xml:lang="en">marine channel</skos:prefLabel>
  </gn:Code>

  <gn:Code rdf:about="http://www.geonames.org/ontology#H.CHNN">
    <skos:definition xml:lang="en">a buoyed channel of sufficient depth for the safe navigation of vessels</skos:definition>
    <skos:inScheme rdf:resource="http://www.geonames.org/ontology#H"/>
    <skos:prefLabel xml:lang="en">navigation channel</skos:prefLabel>
  </gn:Code>

  <gn:Code rdf:about="http://www.geonames.org/ontology#H.CNFL">
    <skos:definition xml:lang="en">a place where two or more streams or intermittent streams flow together</skos:definition>
    <skos:inScheme rdf:resource="http://www.geonames.org/ontology#H"/>
    <skos:prefLabel xml:lang="en">confluence</skos:prefLabel>
  </gn:Code>

  <gn:Code rdf:about="http://www.geonames.org/ontology#H.CNL">
    <skos:definition xml:lang="en">an artificial watercourse</skos:definition>
    <skos:inScheme rdf:resource="http://www.geonames.org/ontology#H"/>
    <skos:prefLabel xml:lang="en">canal</skos:prefLabel>
  </gn:Code>

  <gn:Code rdf:about="http://www.geonames.org/ontology#H.CNLA">
    <skos:definition xml:lang="en">a conduit used to carry water</skos:definition>
    <skos:inScheme rdf:resource="http://www.geonames.org/ontology#H"/>
    <skos:prefLabel xml:lang="en">aqueduct</skos:prefLabel>
  </gn:Code>

  <gn:Code rdf:about="http://www.geonames.org/ontology#H.CNLB">
    <skos:definition xml:lang="en">a conspicuously curved or bent section of a canal</skos:definition>
    <skos:inScheme rdf:resource="http://www.geonames.org/ontology#H"/>
    <skos:prefLabel xml:lang="en">canal bend</skos:prefLabel>
  </gn:Code>

  <gn:Code rdf:about="http://www.geonames.org/ontology#H.CNLD">
    <skos:definition xml:lang="en">an artificial waterway carrying water away from a wetland or from drainage ditches</skos:definition>
    <skos:inScheme rdf:resource="http://www.geonames.org/ontology#H"/>
    <skos:prefLabel xml:lang="en">drainage canal</skos:prefLabel>
  </gn:Code>

  <gn:Code rdf:about="http://www.geonames.org/ontology#H.CNLI">
    <skos:definition xml:lang="en">a canal which serves as a main conduit for irrigation water</skos:definition>
    <skos:inScheme rdf:resource="http://www.geonames.org/ontology#H"/>
    <skos:prefLabel xml:lang="en">irrigation canal</skos:prefLabel>
  </gn:Code>

  <gn:Code rdf:about="http://www.geonames.org/ontology#H.CNLN">
    <skos:definition xml:lang="en">a watercourse constructed for navigation of vessels</skos:definition>
    <skos:inScheme rdf:resource="http://www.geonames.org/ontology#H"/>
    <skos:prefLabel xml:lang="en">navigation canal(s)</skos:prefLabel>
  </gn:Code>

  <gn:Code rdf:about="http://www.geonames.org/ontology#H.CNLQ">
    <skos:definition xml:lang="en">_</skos:definition>
    <skos:inScheme rdf:resource="http://www.geonames.org/ontology#H"/>
    <skos:prefLabel xml:lang="en">abandoned canal</skos:prefLabel>
  </gn:Code>

  <gn:Code rdf:about="http://www.geonames.org/ontology#H.CNLSB">
    <skos:definition xml:lang="en">a gently inclined underground tunnel bringing water for irrigation from aquifers</skos:definition>
    <skos:inScheme rdf:resource="http://www.geonames.org/ontology#H"/>
    <skos:prefLabel xml:lang="en">underground irrigation canal(s)</skos:prefLabel>
  </gn:Code>

  <gn:Code rdf:about="http://www.geonames.org/ontology#H.CNLX">
    <skos:definition xml:lang="en">_</skos:definition>
    <skos:inScheme rdf:resource="http://www.geonames.org/ontology#H"/>
    <skos:prefLabel xml:lang="en">section of canal</skos:prefLabel>
  </gn:Code>

  <gn:Code rdf:about="http://www.geonames.org/ontology#H.COVE">
    <skos:definition xml:lang="en">a small coastal indentation, smaller than a bay</skos:definition>
    <skos:inScheme rdf:resource="http://www.geonames.org/ontology#H"/>
    <skos:prefLabel xml:lang="en">cove(s)</skos:prefLabel>
  </gn:Code>

  <gn:Code rdf:about="http://www.geonames.org/ontology#H.CRKT">
    <skos:definition xml:lang="en">a meandering channel in a coastal wetland subject to bi-directional tidal currents</skos:definition>
    <skos:inScheme rdf:resource="http://www.geonames.org/ontology#H"/>
    <skos:prefLabel xml:lang="en">tidal creek(s)</skos:prefLabel>
  </gn:Code>

  <gn:Code rdf:about="http://www.geonames.org/ontology#H.CRNT">
    <skos:definition xml:lang="en">a horizontal flow of water in a given direction with uniform velocity</skos:definition>
    <skos:inScheme rdf:resource="http://www.geonames.org/ontology#H"/>
    <skos:prefLabel xml:lang="en">current</skos:prefLabel>
  </gn:Code>

  <gn:Code rdf:about="http://www.geonames.org/ontology#H.CUTF">
    <skos:definition xml:lang="en">a channel formed as a result of a stream cutting through a meander neck</skos:definition>
    <skos:inScheme rdf:resource="http://www.geonames.org/ontology#H"/>
    <skos:prefLabel xml:lang="en">cutoff</skos:prefLabel>
  </gn:Code>

  <gn:Code rdf:about="http://www.geonames.org/ontology#H.DCK">
    <skos:definition xml:lang="en">a waterway between two piers, or cut into the land for the berthing of ships</skos:definition>
    <skos:inScheme rdf:resource="http://www.geonames.org/ontology#H"/>
    <skos:prefLabel xml:lang="en">dock(s)</skos:prefLabel>
  </gn:Code>

  <gn:Code rdf:about="http://www.geonames.org/ontology#H.DCKB">
    <skos:definition xml:lang="en">a part of a harbor where ships dock</skos:definition>
    <skos:inScheme rdf:resource="http://www.geonames.org/ontology#H"/>
    <skos:prefLabel xml:lang="en">docking basin</skos:prefLabel>
  </gn:Code>

  <gn:Code rdf:about="http://www.geonames.org/ontology#H.DOMG">
    <skos:definition xml:lang="en">a comparatively elevated area on an icecap</skos:definition>
    <skos:inScheme rdf:resource="http://www.geonames.org/ontology#H"/>
    <skos:prefLabel xml:lang="en">icecap dome</skos:prefLabel>
  </gn:Code>

  <gn:Code rdf:about="http://www.geonames.org/ontology#H.DPRG">
    <skos:definition xml:lang="en">a comparatively depressed area on an icecap</skos:definition>
    <skos:inScheme rdf:resource="http://www.geonames.org/ontology#H"/>
    <skos:prefLabel xml:lang="en">icecap depression</skos:prefLabel>
  </gn:Code>

  <gn:Code rdf:about="http://www.geonames.org/ontology#H.DTCH">
    <skos:definition xml:lang="en">a small artificial watercourse dug for draining or irrigating the land</skos:definition>
    <skos:inScheme rdf:resource="http://www.geonames.org/ontology#H"/>
    <skos:prefLabel xml:lang="en">ditch</skos:prefLabel>
  </gn:Code>

  <gn:Code rdf:about="http://www.geonames.org/ontology#H.DTCHD">
    <skos:definition xml:lang="en">a ditch which serves to drain the land</skos:definition>
    <skos:inScheme rdf:resource="http://www.geonames.org/ontology#H"/>
    <skos:prefLabel xml:lang="en">drainage ditch</skos:prefLabel>
  </gn:Code>

  <gn:Code rdf:about="http://www.geonames.org/ontology#H.DTCHI">
    <skos:definition xml:lang="en">a ditch which serves to distribute irrigation water</skos:definition>
    <skos:inScheme rdf:resource="http://www.geonames.org/ontology#H"/>
    <skos:prefLabel xml:lang="en">irrigation ditch</skos:prefLabel>
  </gn:Code>

  <gn:Code rdf:about="http://www.geonames.org/ontology#H.DTCHM">
    <skos:definition xml:lang="en">an area where a drainage ditch enters a lagoon, lake or bay</skos:definition>
    <skos:inScheme rdf:resource="http://www.geonames.org/ontology#H"/>
    <skos:prefLabel xml:lang="en">ditch mouth(s)</skos:prefLabel>
  </gn:Code>

  <gn:Code rdf:about="http://www.geonames.org/ontology#H.ESTY">
    <skos:definition xml:lang="en">a funnel-shaped stream mouth or embayment where fresh water mixes with sea water under tidal influences</skos:definition>
    <skos:inScheme rdf:resource="http://www.geonames.org/ontology#H"/>
    <skos:prefLabel xml:lang="en">estuary</skos:prefLabel>
  </gn:Code>

  <gn:Code rdf:about="http://www.geonames.org/ontology#H.FISH">
    <skos:definition xml:lang="en">a fishing ground, bank or area where fishermen go to catch fish</skos:definition>
    <skos:inScheme rdf:resource="http://www.geonames.org/ontology#H"/>
    <skos:prefLabel xml:lang="en">fishing area</skos:prefLabel>
  </gn:Code>

  <gn:Code rdf:about="http://www.geonames.org/ontology#H.FJD">
    <skos:definition xml:lang="en">a long, narrow, steep-walled, deep-water arm of the sea at high latitudes, usually along mountainous coasts</skos:definition>
    <skos:inScheme rdf:resource="http://www.geonames.org/ontology#H"/>
    <skos:prefLabel xml:lang="en">fjord</skos:prefLabel>
  </gn:Code>

  <gn:Code rdf:about="http://www.geonames.org/ontology#H.FJDS">
    <skos:definition xml:lang="en">long, narrow, steep-walled, deep-water arms of the sea at high latitudes, usually along mountainous coasts</skos:definition>
    <skos:inScheme rdf:resource="http://www.geonames.org/ontology#H"/>
    <skos:prefLabel xml:lang="en">fjords</skos:prefLabel>
  </gn:Code>

  <gn:Code rdf:about="http://www.geonames.org/ontology#H.FLLS">
    <skos:definition xml:lang="en">a perpendicular or very steep descent of the water of a stream</skos:definition>
    <skos:inScheme rdf:resource="http://www.geonames.org/ontology#H"/>
    <skos:prefLabel xml:lang="en">waterfall(s)</skos:prefLabel>
  </gn:Code>

  <gn:Code rdf:about="http://www.geonames.org/ontology#H.FLLSX">
    <skos:definition xml:lang="en">_</skos:definition>
    <skos:inScheme rdf:resource="http://www.geonames.org/ontology#H"/>
    <skos:prefLabel xml:lang="en">section of waterfall(s)</skos:prefLabel>
  </gn:Code>

  <gn:Code rdf:about="http://www.geonames.org/ontology#H.FLTM">
    <skos:definition xml:lang="en">a relatively level area of mud either between high and low tide lines, or subject to flooding</skos:definition>
    <skos:inScheme rdf:resource="http://www.geonames.org/ontology#H"/>
    <skos:prefLabel xml:lang="en">mud flat(s)</skos:prefLabel>
  </gn:Code>

  <gn:Code rdf:about="http://www.geonames.org/ontology#H.FLTT">
    <skos:definition xml:lang="en">a large flat area of mud or sand attached to the shore and alternately covered and uncovered by the tide</skos:definition>
    <skos:inScheme rdf:resource="http://www.geonames.org/ontology#H"/>
    <skos:prefLabel xml:lang="en">tidal flat(s)</skos:prefLabel>
  </gn:Code>

  <gn:Code rdf:about="http://www.geonames.org/ontology#H.GLCR">
    <skos:definition xml:lang="en">a mass of ice, usually at high latitudes or high elevations, with sufficient thickness to flow away from the source area in lobes, tongues, or masses</skos:definition>
    <skos:inScheme rdf:resource="http://www.geonames.org/ontology#H"/>
    <skos:prefLabel xml:lang="en">glacier(s)</skos:prefLabel>
  </gn:Code>

  <gn:Code rdf:about="http://www.geonames.org/ontology#H.GULF">
    <skos:definition xml:lang="en">a large recess in the coastline, larger than a bay</skos:definition>
    <skos:inScheme rdf:resource="http://www.geonames.org/ontology#H"/>
    <skos:prefLabel xml:lang="en">gulf</skos:prefLabel>
  </gn:Code>

  <gn:Code rdf:about="http://www.geonames.org/ontology#H.GYSR">
    <skos:definition xml:lang="en">a type of hot spring with intermittent eruptions of jets of hot water and steam</skos:definition>
    <skos:inScheme rdf:resource="http://www.geonames.org/ontology#H"/>
    <skos:prefLabel xml:lang="en">geyser</skos:prefLabel>
  </gn:Code>

  <gn:Code rdf:about="http://www.geonames.org/ontology#H.HBR">
    <skos:definition xml:lang="en">a haven or space of deep water so sheltered by the adjacent land as to afford a safe anchorage for ships</skos:definition>
    <skos:inScheme rdf:resource="http://www.geonames.org/ontology#H"/>
    <skos:prefLabel xml:lang="en">harbor(s)</skos:prefLabel>
  </gn:Code>

  <gn:Code rdf:about="http://www.geonames.org/ontology#H.HBRX">
    <skos:definition xml:lang="en">_</skos:definition>
    <skos:inScheme rdf:resource="http://www.geonames.org/ontology#H"/>
    <skos:prefLabel xml:lang="en">section of harbor</skos:prefLabel>
  </gn:Code>

  <gn:Code rdf:about="http://www.geonames.org/ontology#H.INLT">
    <skos:definition xml:lang="en">a narrow waterway extending into the land, or connecting a bay or lagoon with a larger body of water</skos:definition>
    <skos:inScheme rdf:resource="http://www.geonames.org/ontology#H"/>
    <skos:prefLabel xml:lang="en">inlet</skos:prefLabel>
  </gn:Code>

  <gn:Code rdf:about="http://www.geonames.org/ontology#H.INLTQ">
    <skos:definition xml:lang="en">an inlet which has been filled in, or blocked by deposits</skos:definition>
    <skos:inScheme rdf:resource="http://www.geonames.org/ontology#H"/>
    <skos:prefLabel xml:lang="en">former inlet</skos:prefLabel>
  </gn:Code>

  <gn:Code rdf:about="http://www.geonames.org/ontology#H.LBED">
    <skos:definition xml:lang="en">a dried up or drained area of a former lake</skos:definition>
    <skos:inScheme rdf:resource="http://www.geonames.org/ontology#H"/>
    <skos:prefLabel xml:lang="en">lake bed(s)</skos:prefLabel>
  </gn:Code>

  <gn:Code rdf:about="http://www.geonames.org/ontology#H.LGN">
    <skos:definition xml:lang="en">a shallow coastal waterbody, completely or partly separated from a larger body of water by a barrier island, coral reef or other depositional feature</skos:definition>
    <skos:inScheme rdf:resource="http://www.geonames.org/ontology#H"/>
    <skos:prefLabel xml:lang="en">lagoon</skos:prefLabel>
  </gn:Code>

  <gn:Code rdf:about="http://www.geonames.org/ontology#H.LGNS">
    <skos:definition xml:lang="en">shallow coastal waterbodies, completely or partly separated from a larger body of water by a barrier island, coral reef or other depositional feature</skos:definition>
    <skos:inScheme rdf:resource="http://www.geonames.org/ontology#H"/>
    <skos:prefLabel xml:lang="en">lagoons</skos:prefLabel>
  </gn:Code>

  <gn:Code rdf:about="http://www.geonames.org/ontology#H.LGNX">
    <skos:definition xml:lang="en">_</skos:definition>
    <skos:inScheme rdf:resource="http://www.geonames.org/ontology#H"/>
    <skos:prefLabel xml:lang="en">section of lagoon</skos:prefLabel>
  </gn:Code>

  <gn:Code rdf:about="http://www.geonames.org/ontology#H.LK">
    <skos:definition xml:lang="en">a large inland body of standing water</skos:definition>
    <skos:inScheme rdf:resource="http://www.geonames.org/ontology#H"/>
    <skos:prefLabel xml:lang="en">lake</skos:prefLabel>
  </gn:Code>

  <gn:Code rdf:about="http://www.geonames.org/ontology#H.LKC">
    <skos:definition xml:lang="en">a lake in a crater or caldera</skos:definition>
    <skos:inScheme rdf:resource="http://www.geonames.org/ontology#H"/>
    <skos:prefLabel xml:lang="en">crater lake</skos:prefLabel>
  </gn:Code>

  <gn:Code rdf:about="http://www.geonames.org/ontology#H.LKI">
    <skos:definition xml:lang="en">_</skos:definition>
    <skos:inScheme rdf:resource="http://www.geonames.org/ontology#H"/>
    <skos:prefLabel xml:lang="en">intermittent lake</skos:prefLabel>
  </gn:Code>

  <gn:Code rdf:about="http://www.geonames.org/ontology#H.LKN">
    <skos:definition xml:lang="en">an inland body of salt water with no outlet</skos:definition>
    <skos:inScheme rdf:resource="http://www.geonames.org/ontology#H"/>
    <skos:prefLabel xml:lang="en">salt lake</skos:prefLabel>
  </gn:Code>

  <gn:Code rdf:about="http://www.geonames.org/ontology#H.LKNI">
    <skos:definition xml:lang="en">_</skos:definition>
    <skos:inScheme rdf:resource="http://www.geonames.org/ontology#H"/>
    <skos:prefLabel xml:lang="en">intermittent salt lake</skos:prefLabel>
  </gn:Code>

  <gn:Code rdf:about="http://www.geonames.org/ontology#H.LKO">
    <skos:definition xml:lang="en">a crescent-shaped lake commonly found adjacent to meandering streams</skos:definition>
    <skos:inScheme rdf:resource="http://www.geonames.org/ontology#H"/>
    <skos:prefLabel xml:lang="en">oxbow lake</skos:prefLabel>
  </gn:Code>

  <gn:Code rdf:about="http://www.geonames.org/ontology#H.LKOI">
    <skos:definition xml:lang="en">_</skos:definition>
    <skos:inScheme rdf:resource="http://www.geonames.org/ontology#H"/>
    <skos:prefLabel xml:lang="en">intermittent oxbow lake</skos:prefLabel>
  </gn:Code>

  <gn:Code rdf:about="http://www.geonames.org/ontology#H.LKS">
    <skos:definition xml:lang="en">large inland bodies of standing water</skos:definition>
    <skos:inScheme rdf:resource="http://www.geonames.org/ontology#H"/>
    <skos:prefLabel xml:lang="en">lakes</skos:prefLabel>
  </gn:Code>

  <gn:Code rdf:about="http://www.geonames.org/ontology#H.LKSB">
    <skos:definition xml:lang="en">a standing body of water in a cave</skos:definition>
    <skos:inScheme rdf:resource="http://www.geonames.org/ontology#H"/>
    <skos:prefLabel xml:lang="en">underground lake</skos:prefLabel>
  </gn:Code>

  <gn:Code rdf:about="http://www.geonames.org/ontology#H.LKSC">
    <skos:definition xml:lang="en">lakes in a crater or caldera</skos:definition>
    <skos:inScheme rdf:resource="http://www.geonames.org/ontology#H"/>
    <skos:prefLabel xml:lang="en">crater lakes</skos:prefLabel>
  </gn:Code>

  <gn:Code rdf:about="http://www.geonames.org/ontology#H.LKSI">
    <skos:definition xml:lang="en">_</skos:definition>
    <skos:inScheme rdf:resource="http://www.geonames.org/ontology#H"/>
    <skos:prefLabel xml:lang="en">intermittent lakes</skos:prefLabel>
  </gn:Code>

  <gn:Code rdf:about="http://www.geonames.org/ontology#H.LKSN">
    <skos:definition xml:lang="en">inland bodies of salt water with no outlet</skos:definition>
    <skos:inScheme rdf:resource="http://www.geonames.org/ontology#H"/>
    <skos:prefLabel xml:lang="en">salt lakes</skos:prefLabel>
  </gn:Code>

  <gn:Code rdf:about="http://www.geonames.org/ontology#H.LKSNI">
    <skos:definition xml:lang="en">_</skos:definition>
    <skos:inScheme rdf:resource="http://www.geonames.org/ontology#H"/>
    <skos:prefLabel xml:lang="en">intermittent salt lakes</skos:prefLabel>
  </gn:Code>

  <gn:Code rdf:about="http://www.geonames.org/ontology#H.LKX">
    <skos:definition xml:lang="en">_</skos:definition>
    <skos:inScheme rdf:resource="http://www.geonames.org/ontology#H"/>
    <skos:prefLabel xml:lang="en">section of lake</skos:prefLabel>
  </gn:Code>

  <gn:Code rdf:about="http://www.geonames.org/ontology#H.MFGN">
    <skos:definition xml:lang="en">diked salt ponds used in the production of solar evaporated salt</skos:definition>
    <skos:inScheme rdf:resource="http://www.geonames.org/ontology#H"/>
    <skos:prefLabel xml:lang="en">salt evaporation ponds</skos:prefLabel>
  </gn:Code>

  <gn:Code rdf:about="http://www.geonames.org/ontology#H.MGV">
    <skos:definition xml:lang="en">a tropical tidal mud flat characterized by mangrove vegetation</skos:definition>
    <skos:inScheme rdf:resource="http://www.geonames.org/ontology#H"/>
    <skos:prefLabel xml:lang="en">mangrove swamp</skos:prefLabel>
  </gn:Code>

  <gn:Code rdf:about="http://www.geonames.org/ontology#H.MOOR">
    <skos:definition xml:lang="en">an area of open ground overlaid with wet peaty soils</skos:definition>
    <skos:inScheme rdf:resource="http://www.geonames.org/ontology#H"/>
    <skos:prefLabel xml:lang="en">moor(s)</skos:prefLabel>
  </gn:Code>

  <gn:Code rdf:about="http://www.geonames.org/ontology#H.MRSH">
    <skos:definition xml:lang="en">a wetland dominated by grass-like vegetation</skos:definition>
    <skos:inScheme rdf:resource="http://www.geonames.org/ontology#H"/>
    <skos:prefLabel xml:lang="en">marsh(es)</skos:prefLabel>
  </gn:Code>

  <gn:Code rdf:about="http://www.geonames.org/ontology#H.MRSHN">
    <skos:definition xml:lang="en">a flat area, subject to periodic salt water inundation, dominated by grassy salt-tolerant plants</skos:definition>
    <skos:inScheme rdf:resource="http://www.geonames.org/ontology#H"/>
    <skos:prefLabel xml:lang="en">salt marsh</skos:prefLabel>
  </gn:Code>

  <gn:Code rdf:about="http://www.geonames.org/ontology#H.NRWS">
    <skos:definition xml:lang="en">a navigable narrow part of a bay, strait, river, etc.</skos:definition>
    <skos:inScheme rdf:resource="http://www.geonames.org/ontology#H"/>
    <skos:prefLabel xml:lang="en">narrows</skos:prefLabel>
  </gn:Code>

  <gn:Code rdf:about="http://www.geonames.org/ontology#H.OCN">
    <skos:definition xml:lang="en">one of the major divisions of the vast expanse of salt water covering part of the earth</skos:definition>
    <skos:inScheme rdf:resource="http://www.geonames.org/ontology#H"/>
    <skos:prefLabel xml:lang="en">ocean</skos:prefLabel>
  </gn:Code>

  <gn:Code rdf:about="http://www.geonames.org/ontology#H.OVF">
    <skos:definition xml:lang="en">an area of breaking waves caused by the meeting of currents or by waves moving against the current</skos:definition>
    <skos:inScheme rdf:resource="http://www.geonames.org/ontology#H"/>
    <skos:prefLabel xml:lang="en">overfalls</skos:prefLabel>
  </gn:Code>

  <gn:Code rdf:about="http://www.geonames.org/ontology#H.PND">
    <skos:definition xml:lang="en">a small standing waterbody</skos:definition>
    <skos:inScheme rdf:resource="http://www.geonames.org/ontology#H"/>
    <skos:prefLabel xml:lang="en">pond</skos:prefLabel>
  </gn:Code>

  <gn:Code rdf:about="http://www.geonames.org/ontology#H.PNDI">
    <skos:definition xml:lang="en">_</skos:definition>
    <skos:inScheme rdf:resource="http://www.geonames.org/ontology#H"/>
    <skos:prefLabel xml:lang="en">intermittent pond</skos:prefLabel>
  </gn:Code>

  <gn:Code rdf:about="http://www.geonames.org/ontology#H.PNDN">
    <skos:definition xml:lang="en">a small standing body of salt water often in a marsh or swamp, usually along a seacoast</skos:definition>
    <skos:inScheme rdf:resource="http://www.geonames.org/ontology#H"/>
    <skos:prefLabel xml:lang="en">salt pond</skos:prefLabel>
  </gn:Code>

  <gn:Code rdf:about="http://www.geonames.org/ontology#H.PNDNI">
    <skos:definition xml:lang="en">_</skos:definition>
    <skos:inScheme rdf:resource="http://www.geonames.org/ontology#H"/>
    <skos:prefLabel xml:lang="en">intermittent salt pond(s)</skos:prefLabel>
  </gn:Code>

  <gn:Code rdf:about="http://www.geonames.org/ontology#H.PNDS">
    <skos:definition xml:lang="en">small standing waterbodies</skos:definition>
    <skos:inScheme rdf:resource="http://www.geonames.org/ontology#H"/>
    <skos:prefLabel xml:lang="en">ponds</skos:prefLabel>
  </gn:Code>

  <gn:Code rdf:about="http://www.geonames.org/ontology#H.PNDSF">
    <skos:definition xml:lang="en">ponds or enclosures in which fish are kept or raised</skos:definition>
    <skos:inScheme rdf:resource="http://www.geonames.org/ontology#H"/>
    <skos:prefLabel xml:lang="en">fishponds</skos:prefLabel>
  </gn:Code>

  <gn:Code rdf:about="http://www.geonames.org/ontology#H.PNDSI">
    <skos:definition xml:lang="en">_</skos:definition>
    <skos:inScheme rdf:resource="http://www.geonames.org/ontology#H"/>
    <skos:prefLabel xml:lang="en">intermittent ponds</skos:prefLabel>
  </gn:Code>

  <gn:Code rdf:about="http://www.geonames.org/ontology#H.PNDSN">
    <skos:definition xml:lang="en">small standing bodies of salt water often in a marsh or swamp, usually along a seacoast</skos:definition>
    <skos:inScheme rdf:resource="http://www.geonames.org/ontology#H"/>
    <skos:prefLabel xml:lang="en">salt ponds</skos:prefLabel>
  </gn:Code>

  <gn:Code rdf:about="http://www.geonames.org/ontology#H.POOL">
    <skos:definition xml:lang="en">a small and comparatively still, deep part of a larger body of water such as a stream or harbor; or a small body of standing water</skos:definition>
    <skos:inScheme rdf:resource="http://www.geonames.org/ontology#H"/>
    <skos:prefLabel xml:lang="en">pool(s)</skos:prefLabel>
  </gn:Code>

  <gn:Code rdf:about="http://www.geonames.org/ontology#H.POOLI">
    <skos:definition xml:lang="en">_</skos:definition>
    <skos:inScheme rdf:resource="http://www.geonames.org/ontology#H"/>
    <skos:prefLabel xml:lang="en">intermittent pool</skos:prefLabel>
  </gn:Code>

  <gn:Code rdf:about="http://www.geonames.org/ontology#H.RCH">
    <skos:definition xml:lang="en">a straight section of a navigable stream or channel between two bends</skos:definition>
    <skos:inScheme rdf:resource="http://www.geonames.org/ontology#H"/>
    <skos:prefLabel xml:lang="en">reach</skos:prefLabel>
  </gn:Code>

  <gn:Code rdf:about="http://www.geonames.org/ontology#H.RDGG">
    <skos:definition xml:lang="en">a linear elevation on an icecap</skos:definition>
    <skos:inScheme rdf:resource="http://www.geonames.org/ontology#H"/>
    <skos:prefLabel xml:lang="en">icecap ridge</skos:prefLabel>
  </gn:Code>

  <gn:Code rdf:about="http://www.geonames.org/ontology#H.RDST">
    <skos:definition xml:lang="en">an open anchorage affording less protection than a harbor</skos:definition>
    <skos:inScheme rdf:resource="http://www.geonames.org/ontology#H"/>
    <skos:prefLabel xml:lang="en">roadstead</skos:prefLabel>
  </gn:Code>

  <gn:Code rdf:about="http://www.geonames.org/ontology#H.RF">
    <skos:definition xml:lang="en">a surface-navigation hazard composed of consolidated material</skos:definition>
    <skos:inScheme rdf:resource="http://www.geonames.org/ontology#H"/>
    <skos:prefLabel xml:lang="en">reef(s)</skos:prefLabel>
  </gn:Code>

  <gn:Code rdf:about="http://www.geonames.org/ontology#H.RFC">
    <skos:definition xml:lang="en">a surface-navigation hazard composed of coral</skos:definition>
    <skos:inScheme rdf:resource="http://www.geonames.org/ontology#H"/>
    <skos:prefLabel xml:lang="en">coral reef(s)</skos:prefLabel>
  </gn:Code>

  <gn:Code rdf:about="http://www.geonames.org/ontology#H.RFX">
    <skos:definition xml:lang="en">_</skos:definition>
    <skos:inScheme rdf:resource="http://www.geonames.org/ontology#H"/>
    <skos:prefLabel xml:lang="en">section of reef</skos:prefLabel>
  </gn:Code>

  <gn:Code rdf:about="http://www.geonames.org/ontology#H.RPDS">
    <skos:definition xml:lang="en">a turbulent section of a stream associated with a steep, irregular stream bed</skos:definition>
    <skos:inScheme rdf:resource="http://www.geonames.org/ontology#H"/>
    <skos:prefLabel xml:lang="en">rapids</skos:prefLabel>
  </gn:Code>

  <gn:Code rdf:about="http://www.geonames.org/ontology#H.RSV">
    <skos:definition xml:lang="en">an artificial pond or lake</skos:definition>
    <skos:inScheme rdf:resource="http://www.geonames.org/ontology#H"/>
    <skos:prefLabel xml:lang="en">reservoir(s)</skos:prefLabel>
  </gn:Code>

  <gn:Code rdf:about="http://www.geonames.org/ontology#H.RSVI">
    <skos:definition xml:lang="en">_</skos:definition>
    <skos:inScheme rdf:resource="http://www.geonames.org/ontology#H"/>
    <skos:prefLabel xml:lang="en">intermittent reservoir</skos:prefLabel>
  </gn:Code>

  <gn:Code rdf:about="http://www.geonames.org/ontology#H.RSVT">
    <skos:definition xml:lang="en">a contained pool or tank of water at, below, or above ground level</skos:definition>
    <skos:inScheme rdf:resource="http://www.geonames.org/ontology#H"/>
    <skos:prefLabel xml:lang="en">water tank</skos:prefLabel>
  </gn:Code>

  <gn:Code rdf:about="http://www.geonames.org/ontology#H.RVN">
    <skos:definition xml:lang="en">a small, narrow, deep, steep-sided stream channel, smaller than a gorge</skos:definition>
    <skos:inScheme rdf:resource="http://www.geonames.org/ontology#H"/>
    <skos:prefLabel xml:lang="en">ravine(s)</skos:prefLabel>
  </gn:Code>

  <gn:Code rdf:about="http://www.geonames.org/ontology#H.SBKH">
    <skos:definition xml:lang="en">a salt flat or salt encrusted plain subject to periodic inundation from flooding or high tides</skos:definition>
    <skos:inScheme rdf:resource="http://www.geonames.org/ontology#H"/>
    <skos:prefLabel xml:lang="en">sabkha(s)</skos:prefLabel>
  </gn:Code>

  <gn:Code rdf:about="http://www.geonames.org/ontology#H.SD">
    <skos:definition xml:lang="en">a long arm of the sea forming a channel between the mainland and an island or islands; or connecting two larger bodies of water</skos:definition>
    <skos:inScheme rdf:resource="http://www.geonames.org/ontology#H"/>
    <skos:prefLabel xml:lang="en">sound</skos:prefLabel>
  </gn:Code>

  <gn:Code rdf:about="http://www.geonames.org/ontology#H.SEA">
    <skos:definition xml:lang="en">a large body of salt water more or less confined by continuous land or chains of islands forming a subdivision of an ocean</skos:definition>
    <skos:inScheme rdf:resource="http://www.geonames.org/ontology#H"/>
    <skos:prefLabel xml:lang="en">sea</skos:prefLabel>
  </gn:Code>

  <gn:Code rdf:about="http://www.geonames.org/ontology#H.SHOL">
    <skos:definition xml:lang="en">a surface-navigation hazard composed of unconsolidated material</skos:definition>
    <skos:inScheme rdf:resource="http://www.geonames.org/ontology#H"/>
    <skos:prefLabel xml:lang="en">shoal(s)</skos:prefLabel>
  </gn:Code>

  <gn:Code rdf:about="http://www.geonames.org/ontology#H.SILL">
    <skos:definition xml:lang="en">the low part of an underwater gap or saddle separating basins, including a similar feature at the mouth of a fjord</skos:definition>
    <skos:inScheme rdf:resource="http://www.geonames.org/ontology#H"/>
    <skos:prefLabel xml:lang="en">sill</skos:prefLabel>
  </gn:Code>

  <gn:Code rdf:about="http://www.geonames.org/ontology#H.SPNG">
    <skos:definition xml:lang="en">a place where ground water flows naturally out of the ground</skos:definition>
    <skos:inScheme rdf:resource="http://www.geonames.org/ontology#H"/>
    <skos:prefLabel xml:lang="en">spring(s)</skos:prefLabel>
  </gn:Code>

  <gn:Code rdf:about="http://www.geonames.org/ontology#H.SPNS">
    <skos:definition xml:lang="en">a place where sulphur ground water flows naturally out of the ground</skos:definition>
    <skos:inScheme rdf:resource="http://www.geonames.org/ontology#H"/>
    <skos:prefLabel xml:lang="en">sulphur spring(s)</skos:prefLabel>
  </gn:Code>

  <gn:Code rdf:about="http://www.geonames.org/ontology#H.SPNT">
    <skos:definition xml:lang="en">a place where hot ground water flows naturally out of the ground</skos:definition>
    <skos:inScheme rdf:resource="http://www.geonames.org/ontology#H"/>
    <skos:prefLabel xml:lang="en">hot spring(s)</skos:prefLabel>
  </gn:Code>

  <gn:Code rdf:about="http://www.geonames.org/ontology#H.STM">
    <skos:definition xml:lang="en">a body of running water moving to a lower level in a channel on land</skos:definition>
    <skos:inScheme rdf:resource="http://www.geonames.org/ontology#H"/>
    <skos:prefLabel xml:lang="en">stream</skos:prefLabel>
  </gn:Code>

  <gn:Code rdf:about="http://www.geonames.org/ontology#H.STMA">
    <skos:definition xml:lang="en">a diverging branch flowing out of a main stream and rejoining it downstream</skos:definition>
    <skos:inScheme rdf:resource="http://www.geonames.org/ontology#H"/>
    <skos:prefLabel xml:lang="en">anabranch</skos:prefLabel>
  </gn:Code>

  <gn:Code rdf:about="http://www.geonames.org/ontology#H.STMB">
    <skos:definition xml:lang="en">a conspicuously curved or bent segment of a stream</skos:definition>
    <skos:inScheme rdf:resource="http://www.geonames.org/ontology#H"/>
    <skos:prefLabel xml:lang="en">stream bend</skos:prefLabel>
  </gn:Code>

  <gn:Code rdf:about="http://www.geonames.org/ontology#H.STMC">
    <skos:definition xml:lang="en">a stream that has been substantially ditched, diked, or straightened</skos:definition>
    <skos:inScheme rdf:resource="http://www.geonames.org/ontology#H"/>
    <skos:prefLabel xml:lang="en">canalized stream</skos:prefLabel>
  </gn:Code>

  <gn:Code rdf:about="http://www.geonames.org/ontology#H.STMD">
    <skos:definition xml:lang="en">a branch which flows away from the main stream, as in a delta or irrigation canal</skos:definition>
    <skos:inScheme rdf:resource="http://www.geonames.org/ontology#H"/>
    <skos:prefLabel xml:lang="en">distributary(-ies)</skos:prefLabel>
  </gn:Code>

  <gn:Code rdf:about="http://www.geonames.org/ontology#H.STMH">
    <skos:definition xml:lang="en">the source and upper part of a stream, including the upper drainage basin</skos:definition>
    <skos:inScheme rdf:resource="http://www.geonames.org/ontology#H"/>
    <skos:prefLabel xml:lang="en">headwaters</skos:prefLabel>
  </gn:Code>

  <gn:Code rdf:about="http://www.geonames.org/ontology#H.STMI">
    <skos:definition xml:lang="en">_</skos:definition>
    <skos:inScheme rdf:resource="http://www.geonames.org/ontology#H"/>
    <skos:prefLabel xml:lang="en">intermittent stream</skos:prefLabel>
  </gn:Code>

  <gn:Code rdf:about="http://www.geonames.org/ontology#H.STMIX">
    <skos:definition xml:lang="en">_</skos:definition>
    <skos:inScheme rdf:resource="http://www.geonames.org/ontology#H"/>
    <skos:prefLabel xml:lang="en">section of intermittent stream</skos:prefLabel>
  </gn:Code>

  <gn:Code rdf:about="http://www.geonames.org/ontology#H.STMM">
    <skos:definition xml:lang="en">a place where a stream discharges into a lagoon, lake, or the sea</skos:definition>
    <skos:inScheme rdf:resource="http://www.geonames.org/ontology#H"/>
    <skos:prefLabel xml:lang="en">stream mouth(s)</skos:prefLabel>
  </gn:Code>

  <gn:Code rdf:about="http://www.geonames.org/ontology#H.STMQ">
    <skos:definition xml:lang="en">a former stream or distributary no longer carrying flowing water, but still evident due to lakes, wetland, topographic or vegetation patterns</skos:definition>
    <skos:inScheme rdf:resource="http://www.geonames.org/ontology#H"/>
    <skos:prefLabel xml:lang="en">abandoned watercourse</skos:prefLabel>
  </gn:Code>

  <gn:Code rdf:about="http://www.geonames.org/ontology#H.STMS">
    <skos:definition xml:lang="en">bodies of running water moving to a lower level in a channel on land</skos:definition>
    <skos:inScheme rdf:resource="http://www.geonames.org/ontology#H"/>
    <skos:prefLabel xml:lang="en">streams</skos:prefLabel>
  </gn:Code>

  <gn:Code rdf:about="http://www.geonames.org/ontology#H.STMSB">
    <skos:definition xml:lang="en">a surface stream that disappears into an underground channel, or dries up in an arid area</skos:definition>
    <skos:inScheme rdf:resource="http://www.geonames.org/ontology#H"/>
    <skos:prefLabel xml:lang="en">lost river</skos:prefLabel>
  </gn:Code>

  <gn:Code rdf:about="http://www.geonames.org/ontology#H.STMX">
    <skos:definition xml:lang="en">_</skos:definition>
    <skos:inScheme rdf:resource="http://www.geonames.org/ontology#H"/>
    <skos:prefLabel xml:lang="en">section of stream</skos:prefLabel>
  </gn:Code>

  <gn:Code rdf:about="http://www.geonames.org/ontology#H.STRT">
    <skos:definition xml:lang="en">a relatively narrow waterway, usually narrower and less extensive than a sound, connecting two larger bodies of water</skos:definition>
    <skos:inScheme rdf:resource="http://www.geonames.org/ontology#H"/>
    <skos:prefLabel xml:lang="en">strait</skos:prefLabel>
  </gn:Code>

  <gn:Code rdf:about="http://www.geonames.org/ontology#H.SWMP">
    <skos:definition xml:lang="en">a wetland dominated by tree vegetation</skos:definition>
    <skos:inScheme rdf:resource="http://www.geonames.org/ontology#H"/>
    <skos:prefLabel xml:lang="en">swamp</skos:prefLabel>
  </gn:Code>

  <gn:Code rdf:about="http://www.geonames.org/ontology#H.SYSI">
    <skos:definition xml:lang="en">a network of ditches and one or more of the following elements: water supply, reservoir, canal, pump, well, drain, etc.</skos:definition>
    <skos:inScheme rdf:resource="http://www.geonames.org/ontology#H"/>
    <skos:prefLabel xml:lang="en">irrigation system</skos:prefLabel>
  </gn:Code>

  <gn:Code rdf:about="http://www.geonames.org/ontology#H.TNLC">
    <skos:definition xml:lang="en">a tunnel through which a canal passes</skos:definition>
    <skos:inScheme rdf:resource="http://www.geonames.org/ontology#H"/>
    <skos:prefLabel xml:lang="en">canal tunnel</skos:prefLabel>
  </gn:Code>

  <gn:Code rdf:about="http://www.geonames.org/ontology#H.WAD">
    <skos:definition xml:lang="en">a valley or ravine, bounded by relatively steep banks, which in the rainy season becomes a watercourse; found primarily in North Africa and the Middle East</skos:definition>
    <skos:inScheme rdf:resource="http://www.geonames.org/ontology#H"/>
    <skos:prefLabel xml:lang="en">wadi</skos:prefLabel>
  </gn:Code>

  <gn:Code rdf:about="http://www.geonames.org/ontology#H.WADB">
    <skos:definition xml:lang="en">a conspicuously curved or bent segment of a wadi</skos:definition>
    <skos:inScheme rdf:resource="http://www.geonames.org/ontology#H"/>
    <skos:prefLabel xml:lang="en">wadi bend</skos:prefLabel>
  </gn:Code>

  <gn:Code rdf:about="http://www.geonames.org/ontology#H.WADJ">
    <skos:definition xml:lang="en">a place where two or more wadies join</skos:definition>
    <skos:inScheme rdf:resource="http://www.geonames.org/ontology#H"/>
    <skos:prefLabel xml:lang="en">wadi junction</skos:prefLabel>
  </gn:Code>

  <gn:Code rdf:about="http://www.geonames.org/ontology#H.WADM">
    <skos:definition xml:lang="en">the lower terminus of a wadi where it widens into an adjoining floodplain, depression, or waterbody</skos:definition>
    <skos:inScheme rdf:resource="http://www.geonames.org/ontology#H"/>
    <skos:prefLabel xml:lang="en">wadi mouth</skos:prefLabel>
  </gn:Code>

  <gn:Code rdf:about="http://www.geonames.org/ontology#H.WADS">
    <skos:definition xml:lang="en">valleys or ravines, bounded by relatively steep banks, which in the rainy season become watercourses; found primarily in North Africa and the Middle East</skos:definition>
    <skos:inScheme rdf:resource="http://www.geonames.org/ontology#H"/>
    <skos:prefLabel xml:lang="en">wadies</skos:prefLabel>
  </gn:Code>

  <gn:Code rdf:about="http://www.geonames.org/ontology#H.WADX">
    <skos:definition xml:lang="en">_</skos:definition>
    <skos:inScheme rdf:resource="http://www.geonames.org/ontology#H"/>
    <skos:prefLabel xml:lang="en">section of wadi</skos:prefLabel>
  </gn:Code>

  <gn:Code rdf:about="http://www.geonames.org/ontology#H.WHRL">
    <skos:definition xml:lang="en">a turbulent, rotating movement of water in a stream</skos:definition>
    <skos:inScheme rdf:resource="http://www.geonames.org/ontology#H"/>
    <skos:prefLabel xml:lang="en">whirlpool</skos:prefLabel>
  </gn:Code>

  <gn:Code rdf:about="http://www.geonames.org/ontology#H.WLL">
    <skos:definition xml:lang="en">a cylindrical hole, pit, or tunnel drilled or dug down to a depth from which water, oil, or gas can be pumped or brought to the surface</skos:definition>
    <skos:inScheme rdf:resource="http://www.geonames.org/ontology#H"/>
    <skos:prefLabel xml:lang="en">well</skos:prefLabel>
  </gn:Code>

  <gn:Code rdf:about="http://www.geonames.org/ontology#H.WLLQ">
    <skos:definition xml:lang="en">_</skos:definition>
    <skos:inScheme rdf:resource="http://www.geonames.org/ontology#H"/>
    <skos:prefLabel xml:lang="en">abandoned well</skos:prefLabel>
  </gn:Code>

  <gn:Code rdf:about="http://www.geonames.org/ontology#H.WLLS">
    <skos:definition xml:lang="en">cylindrical holes, pits, or tunnels drilled or dug down to a depth from which water, oil, or gas can be pumped or brought to the surface</skos:definition>
    <skos:inScheme rdf:resource="http://www.geonames.org/ontology#H"/>
    <skos:prefLabel xml:lang="en">wells</skos:prefLabel>
  </gn:Code>

  <gn:Code rdf:about="http://www.geonames.org/ontology#H.WTLD">
    <skos:definition xml:lang="en">an area subject to inundation, usually characterized by bog, marsh, or swamp vegetation</skos:definition>
    <skos:inScheme rdf:resource="http://www.geonames.org/ontology#H"/>
    <skos:prefLabel xml:lang="en">wetland</skos:prefLabel>
  </gn:Code>

  <gn:Code rdf:about="http://www.geonames.org/ontology#H.WTLDI">
    <skos:definition xml:lang="en">_</skos:definition>
    <skos:inScheme rdf:resource="http://www.geonames.org/ontology#H"/>
    <skos:prefLabel xml:lang="en">intermittent wetland</skos:prefLabel>
  </gn:Code>

  <gn:Code rdf:about="http://www.geonames.org/ontology#H.WTRC">
    <skos:definition xml:lang="en">a natural, well-defined channel produced by flowing water, or an artificial channel designed to carry flowing water</skos:definition>
    <skos:inScheme rdf:resource="http://www.geonames.org/ontology#H"/>
    <skos:prefLabel xml:lang="en">watercourse</skos:prefLabel>
  </gn:Code>

  <gn:Code rdf:about="http://www.geonames.org/ontology#H.WTRH">
    <skos:definition xml:lang="en">a natural hole, hollow, or small depression that contains water, used by man and animals, especially in arid areas</skos:definition>
    <skos:inScheme rdf:resource="http://www.geonames.org/ontology#H"/>
    <skos:prefLabel xml:lang="en">waterhole(s)</skos:prefLabel>
  </gn:Code>

  <gn:Class rdf:about="http://www.geonames.org/ontology#L">
    <rdfs:comment xml:lang="en">parks,area, ...</rdfs:comment>
  </gn:Class>

  <gn:Code rdf:about="http://www.geonames.org/ontology#L.AGRC">
    <skos:definition xml:lang="en">a tract of land set aside for agricultural settlement</skos:definition>
    <skos:inScheme rdf:resource="http://www.geonames.org/ontology#L"/>
    <skos:prefLabel xml:lang="en">agricultural colony</skos:prefLabel>
  </gn:Code>

  <gn:Code rdf:about="http://www.geonames.org/ontology#L.AMUS">
    <skos:definition xml:lang="en">Amusement Park are theme parks, adventure parks offering entertainment, similar to funfairs but with a fix location</skos:definition>
    <skos:inScheme rdf:resource="http://www.geonames.org/ontology#L"/>
    <skos:prefLabel xml:lang="en">amusement park</skos:prefLabel>
  </gn:Code>

  <gn:Code rdf:about="http://www.geonames.org/ontology#L.AREA">
    <skos:definition xml:lang="en">a tract of land without homogeneous character or boundaries</skos:definition>
    <skos:inScheme rdf:resource="http://www.geonames.org/ontology#L"/>
    <skos:prefLabel xml:lang="en">area</skos:prefLabel>
  </gn:Code>

  <gn:Code rdf:about="http://www.geonames.org/ontology#L.BSND">
    <skos:definition xml:lang="en">an area drained by a stream</skos:definition>
    <skos:inScheme rdf:resource="http://www.geonames.org/ontology#L"/>
    <skos:prefLabel xml:lang="en">drainage basin</skos:prefLabel>
  </gn:Code>

  <gn:Code rdf:about="http://www.geonames.org/ontology#L.BSNP">
    <skos:definition xml:lang="en">an area underlain by an oil-rich structural basin</skos:definition>
    <skos:inScheme rdf:resource="http://www.geonames.org/ontology#L"/>
    <skos:prefLabel xml:lang="en">petroleum basin</skos:prefLabel>
  </gn:Code>

  <gn:Code rdf:about="http://www.geonames.org/ontology#L.BTL">
    <skos:definition xml:lang="en">a site of a land battle of historical importance</skos:definition>
    <skos:inScheme rdf:resource="http://www.geonames.org/ontology#L"/>
    <skos:prefLabel xml:lang="en">battlefield</skos:prefLabel>
  </gn:Code>

  <gn:Code rdf:about="http://www.geonames.org/ontology#L.CLG">
    <skos:definition xml:lang="en">an area in a forest with trees removed</skos:definition>
    <skos:inScheme rdf:resource="http://www.geonames.org/ontology#L"/>
    <skos:prefLabel xml:lang="en">clearing</skos:prefLabel>
  </gn:Code>

  <gn:Code rdf:about="http://www.geonames.org/ontology#L.CMN">
    <skos:definition xml:lang="en">a park or pasture for community use</skos:definition>
    <skos:inScheme rdf:resource="http://www.geonames.org/ontology#L"/>
    <skos:prefLabel xml:lang="en">common</skos:prefLabel>
  </gn:Code>

  <gn:Code rdf:about="http://www.geonames.org/ontology#L.CNS">
    <skos:definition xml:lang="en">a lease of land by a government for economic development, e.g., mining, forestry</skos:definition>
    <skos:inScheme rdf:resource="http://www.geonames.org/ontology#L"/>
    <skos:prefLabel xml:lang="en">concession area</skos:prefLabel>
  </gn:Code>

  <gn:Code rdf:about="http://www.geonames.org/ontology#L.COLF">
    <skos:definition xml:lang="en">a region in which coal deposits of possible economic value occur</skos:definition>
    <skos:inScheme rdf:resource="http://www.geonames.org/ontology#L"/>
    <skos:prefLabel xml:lang="en">coalfield</skos:prefLabel>
  </gn:Code>

  <gn:Code rdf:about="http://www.geonames.org/ontology#L.CONT">
    <skos:definition xml:lang="en">continent : Europe, Africa, Asia, North America, South America, Oceania,Antarctica</skos:definition>
    <skos:inScheme rdf:resource="http://www.geonames.org/ontology#L"/>
    <skos:prefLabel xml:lang="en">continent</skos:prefLabel>
  </gn:Code>

  <gn:Code rdf:about="http://www.geonames.org/ontology#L.CST">
    <skos:definition xml:lang="en">a zone of variable width straddling the shoreline</skos:definition>
    <skos:inScheme rdf:resource="http://www.geonames.org/ontology#L"/>
    <skos:prefLabel xml:lang="en">coast</skos:prefLabel>
  </gn:Code>

  <gn:Code rdf:about="http://www.geonames.org/ontology#L.CTRB">
    <skos:definition xml:lang="en">a place where a number of businesses are located</skos:definition>
    <skos:inScheme rdf:resource="http://www.geonames.org/ontology#L"/>
    <skos:prefLabel xml:lang="en">business center</skos:prefLabel>
  </gn:Code>

  <gn:Code rdf:about="http://www.geonames.org/ontology#L.DEVH">
    <skos:definition xml:lang="en">a tract of land on which many houses of similar design are built according to a development plan</skos:definition>
    <skos:inScheme rdf:resource="http://www.geonames.org/ontology#L"/>
    <skos:prefLabel xml:lang="en">housing development</skos:prefLabel>
  </gn:Code>

  <gn:Code rdf:about="http://www.geonames.org/ontology#L.FLD">
    <skos:definition xml:lang="en">an open as opposed to wooded area</skos:definition>
    <skos:inScheme rdf:resource="http://www.geonames.org/ontology#L"/>
    <skos:prefLabel xml:lang="en">field(s)</skos:prefLabel>
  </gn:Code>

  <gn:Code rdf:about="http://www.geonames.org/ontology#L.FLDI">
    <skos:definition xml:lang="en">a tract of level or terraced land which is irrigated</skos:definition>
    <skos:inScheme rdf:resource="http://www.geonames.org/ontology#L"/>
    <skos:prefLabel xml:lang="en">irrigated field(s)</skos:prefLabel>
  </gn:Code>

  <gn:Code rdf:about="http://www.geonames.org/ontology#L.GASF">
    <skos:definition xml:lang="en">an area containing a subterranean store of natural gas of economic value</skos:definition>
    <skos:inScheme rdf:resource="http://www.geonames.org/ontology#L"/>
    <skos:prefLabel xml:lang="en">gasfield</skos:prefLabel>
  </gn:Code>

  <gn:Code rdf:about="http://www.geonames.org/ontology#L.GRAZ">
    <skos:definition xml:lang="en">an area of grasses and shrubs used for grazing</skos:definition>
    <skos:inScheme rdf:resource="http://www.geonames.org/ontology#L"/>
    <skos:prefLabel xml:lang="en">grazing area</skos:prefLabel>
  </gn:Code>

  <gn:Code rdf:about="http://www.geonames.org/ontology#L.GVL">
    <skos:definition xml:lang="en">an area covered with gravel</skos:definition>
    <skos:inScheme rdf:resource="http://www.geonames.org/ontology#L"/>
    <skos:prefLabel xml:lang="en">gravel area</skos:prefLabel>
  </gn:Code>

  <gn:Code rdf:about="http://www.geonames.org/ontology#L.INDS">
    <skos:definition xml:lang="en">an area characterized by industrial activity</skos:definition>
    <skos:inScheme rdf:resource="http://www.geonames.org/ontology#L"/>
    <skos:prefLabel xml:lang="en">industrial area</skos:prefLabel>
  </gn:Code>

  <gn:Code rdf:about="http://www.geonames.org/ontology#L.LAND">
    <skos:definition xml:lang="en">a tract of land in the Arctic</skos:definition>
    <skos:inScheme rdf:resource="http://www.geonames.org/ontology#L"/>
    <skos:prefLabel xml:lang="en">arctic land</skos:prefLabel>
  </gn:Code>

  <gn:Code rdf:about="http://www.geonames.org/ontology#L.LCTY">
    <skos:definition xml:lang="en">a minor area or place of unspecified or mixed character and indefinite boundaries</skos:definition>
    <skos:inScheme rdf:resource="http://www.geonames.org/ontology#L"/>
    <skos:prefLabel xml:lang="en">locality</skos:prefLabel>
  </gn:Code>

  <gn:Code rdf:about="http://www.geonames.org/ontology#L.MILB">
    <skos:definition xml:lang="en">a place used by an army or other armed service for storing arms and supplies, and for accommodating and training troops, a base from which operations can be initiated</skos:definition>
    <skos:inScheme rdf:resource="http://www.geonames.org/ontology#L"/>
    <skos:prefLabel xml:lang="en">military base</skos:prefLabel>
  </gn:Code>

  <gn:Code rdf:about="http://www.geonames.org/ontology#L.MNA">
    <skos:definition xml:lang="en">an area of mine sites where minerals and ores are extracted</skos:definition>
    <skos:inScheme rdf:resource="http://www.geonames.org/ontology#L"/>
    <skos:prefLabel xml:lang="en">mining area</skos:prefLabel>
  </gn:Code>

  <gn:Code rdf:about="http://www.geonames.org/ontology#L.MVA">
    <skos:definition xml:lang="en">a tract of land where military field exercises are carried out</skos:definition>
    <skos:inScheme rdf:resource="http://www.geonames.org/ontology#L"/>
    <skos:prefLabel xml:lang="en">maneuver area</skos:prefLabel>
  </gn:Code>

  <gn:Code rdf:about="http://www.geonames.org/ontology#L.NVB">
    <skos:definition xml:lang="en">an area used to store supplies, provide barracks for troops and naval personnel, a port for naval vessels, and from which operations are initiated</skos:definition>
    <skos:inScheme rdf:resource="http://www.geonames.org/ontology#L"/>
    <skos:prefLabel xml:lang="en">naval base</skos:prefLabel>
  </gn:Code>

  <gn:Code rdf:about="http://www.geonames.org/ontology#L.OAS">
    <skos:definition xml:lang="en">an area in a desert made productive by the availability of water</skos:definition>
    <skos:inScheme rdf:resource="http://www.geonames.org/ontology#L"/>
    <skos:prefLabel xml:lang="en">oasis(-es)</skos:prefLabel>
  </gn:Code>

  <gn:Code rdf:about="http://www.geonames.org/ontology#L.OILF">
    <skos:definition xml:lang="en">an area containing a subterranean store of petroleum of economic value</skos:definition>
    <skos:inScheme rdf:resource="http://www.geonames.org/ontology#L"/>
    <skos:prefLabel xml:lang="en">oilfield</skos:prefLabel>
  </gn:Code>

  <gn:Code rdf:about="http://www.geonames.org/ontology#L.PEAT">
    <skos:definition xml:lang="en">an area where peat is harvested</skos:definition>
    <skos:inScheme rdf:resource="http://www.geonames.org/ontology#L"/>
    <skos:prefLabel xml:lang="en">peat cutting area</skos:prefLabel>
  </gn:Code>

  <gn:Code rdf:about="http://www.geonames.org/ontology#L.PRK">
    <skos:definition xml:lang="en">an area, often of forested land, maintained as a place of beauty, or for recreation</skos:definition>
    <skos:inScheme rdf:resource="http://www.geonames.org/ontology#L"/>
    <skos:prefLabel xml:lang="en">park</skos:prefLabel>
  </gn:Code>

  <gn:Code rdf:about="http://www.geonames.org/ontology#L.PRT">
    <skos:definition xml:lang="en">a place provided with terminal and transfer facilities for loading and discharging waterborne cargo or passengers, usually located in a harbor</skos:definition>
    <skos:inScheme rdf:resource="http://www.geonames.org/ontology#L"/>
    <skos:prefLabel xml:lang="en">port</skos:prefLabel>
  </gn:Code>

  <gn:Code rdf:about="http://www.geonames.org/ontology#L.QCKS">
    <skos:definition xml:lang="en">an area where loose sand with water moving through it may become unstable when heavy objects are placed at the surface, causing them to sink</skos:definition>
    <skos:inScheme rdf:resource="http://www.geonames.org/ontology#L"/>
    <skos:prefLabel xml:lang="en">quicksand</skos:prefLabel>
  </gn:Code>

  <gn:Code rdf:about="http://www.geonames.org/ontology#L.REP">
    <skos:definition xml:lang="en">_</skos:definition>
    <skos:inScheme rdf:resource="http://www.geonames.org/ontology#L"/>
    <skos:prefLabel xml:lang="en">republic</skos:prefLabel>
  </gn:Code>

  <gn:Code rdf:about="http://www.geonames.org/ontology#L.RES">
    <skos:definition xml:lang="en">a tract of public land reserved for future use or restricted as to use</skos:definition>
    <skos:inScheme rdf:resource="http://www.geonames.org/ontology#L"/>
    <skos:prefLabel xml:lang="en">reserve</skos:prefLabel>
  </gn:Code>

  <gn:Code rdf:about="http://www.geonames.org/ontology#L.RESA">
    <skos:definition xml:lang="en">a tract of land reserved for agricultural reclamation and/or development</skos:definition>
    <skos:inScheme rdf:resource="http://www.geonames.org/ontology#L"/>
    <skos:prefLabel xml:lang="en">agricultural reserve</skos:prefLabel>
  </gn:Code>

  <gn:Code rdf:about="http://www.geonames.org/ontology#L.RESF">
    <skos:definition xml:lang="en">a forested area set aside for preservation or controlled use</skos:definition>
    <skos:inScheme rdf:resource="http://www.geonames.org/ontology#L"/>
    <skos:prefLabel xml:lang="en">forest reserve</skos:prefLabel>
  </gn:Code>

  <gn:Code rdf:about="http://www.geonames.org/ontology#L.RESH">
    <skos:definition xml:lang="en">a tract of land used primarily for hunting</skos:definition>
    <skos:inScheme rdf:resource="http://www.geonames.org/ontology#L"/>
    <skos:prefLabel xml:lang="en">hunting reserve</skos:prefLabel>
  </gn:Code>

  <gn:Code rdf:about="http://www.geonames.org/ontology#L.RESN">
    <skos:definition xml:lang="en">an area reserved for the maintenance of a natural habitat</skos:definition>
    <skos:inScheme rdf:resource="http://www.geonames.org/ontology#L"/>
    <skos:prefLabel xml:lang="en">nature reserve</skos:prefLabel>
  </gn:Code>

  <gn:Code rdf:about="http://www.geonames.org/ontology#L.RESP">
    <skos:definition xml:lang="en">an area of palm trees where use is controlled</skos:definition>
    <skos:inScheme rdf:resource="http://www.geonames.org/ontology#L"/>
    <skos:prefLabel xml:lang="en">palm tree reserve</skos:prefLabel>
  </gn:Code>

  <gn:Code rdf:about="http://www.geonames.org/ontology#L.RESV">
    <skos:definition xml:lang="en">a tract of land set aside for aboriginal, tribal, or native populations</skos:definition>
    <skos:inScheme rdf:resource="http://www.geonames.org/ontology#L"/>
    <skos:prefLabel xml:lang="en">reservation</skos:prefLabel>
  </gn:Code>

  <gn:Code rdf:about="http://www.geonames.org/ontology#L.RESW">
    <skos:definition xml:lang="en">a tract of public land reserved for the preservation of wildlife</skos:definition>
    <skos:inScheme rdf:resource="http://www.geonames.org/ontology#L"/>
    <skos:prefLabel xml:lang="en">wildlife reserve</skos:prefLabel>
  </gn:Code>

  <gn:Code rdf:about="http://www.geonames.org/ontology#L.RGN">
    <skos:definition xml:lang="en">an area distinguished by one or more observable physical or cultural characteristics</skos:definition>
    <skos:inScheme rdf:resource="http://www.geonames.org/ontology#L"/>
    <skos:prefLabel xml:lang="en">region</skos:prefLabel>
  </gn:Code>

  <gn:Code rdf:about="http://www.geonames.org/ontology#L.RGNE">
    <skos:definition xml:lang="en">a region of a country established for economic development or for statistical purposes</skos:definition>
    <skos:inScheme rdf:resource="http://www.geonames.org/ontology#L"/>
    <skos:prefLabel xml:lang="en">economic region</skos:prefLabel>
  </gn:Code>

  <gn:Code rdf:about="http://www.geonames.org/ontology#L.RGNL">
    <skos:definition xml:lang="en">a tract of land distinguished by numerous lakes</skos:definition>
    <skos:inScheme rdf:resource="http://www.geonames.org/ontology#L"/>
    <skos:prefLabel xml:lang="en">lake region</skos:prefLabel>
  </gn:Code>

  <gn:Code rdf:about="http://www.geonames.org/ontology#L.RNGA">
    <skos:definition xml:lang="en">a tract of land used for artillery firing practice</skos:definition>
    <skos:inScheme rdf:resource="http://www.geonames.org/ontology#L"/>
    <skos:prefLabel xml:lang="en">artillery range</skos:prefLabel>
  </gn:Code>

  <gn:Code rdf:about="http://www.geonames.org/ontology#L.SALT">
    <skos:definition xml:lang="en">a shallow basin or flat where salt accumulates after periodic inundation</skos:definition>
    <skos:inScheme rdf:resource="http://www.geonames.org/ontology#L"/>
    <skos:prefLabel xml:lang="en">salt area</skos:prefLabel>
  </gn:Code>

  <gn:Code rdf:about="http://www.geonames.org/ontology#L.SNOW">
    <skos:definition xml:lang="en">an area of permanent snow and ice forming the accumulation area of a glacier</skos:definition>
    <skos:inScheme rdf:resource="http://www.geonames.org/ontology#L"/>
    <skos:prefLabel xml:lang="en">snowfield</skos:prefLabel>
  </gn:Code>

  <gn:Code rdf:about="http://www.geonames.org/ontology#L.TRB">
    <skos:definition xml:lang="en">a tract of land used by nomadic or other tribes</skos:definition>
    <skos:inScheme rdf:resource="http://www.geonames.org/ontology#L"/>
    <skos:prefLabel xml:lang="en">tribal area</skos:prefLabel>
  </gn:Code>

  <gn:Code rdf:about="http://www.geonames.org/ontology#L.ZZZZZ">
    <skos:definition xml:lang="en">_</skos:definition>
    <skos:inScheme rdf:resource="http://www.geonames.org/ontology#L"/>
    <skos:prefLabel xml:lang="en">master source holdings list</skos:prefLabel>
  </gn:Code>

  <gn:Class rdf:about="http://www.geonames.org/ontology#P">
    <rdfs:comment xml:lang="en">city, village,...</rdfs:comment>
  </gn:Class>

  <gn:Code rdf:about="http://www.geonames.org/ontology#P.PPL">
    <skos:definition xml:lang="en">a city, town, village, or other agglomeration of buildings where people live and work</skos:definition>
    <skos:inScheme rdf:resource="http://www.geonames.org/ontology#P"/>
    <skos:prefLabel xml:lang="en">populated place</skos:prefLabel>
  </gn:Code>

  <gn:Code rdf:about="http://www.geonames.org/ontology#P.PPLA">
    <skos:definition xml:lang="en">seat of a first-order administrative division (PPLC takes precedence over PPLA)</skos:definition>
    <skos:inScheme rdf:resource="http://www.geonames.org/ontology#P"/>
    <skos:prefLabel xml:lang="en">seat of a first-order administrative division</skos:prefLabel>
  </gn:Code>

  <gn:Code rdf:about="http://www.geonames.org/ontology#P.PPLA2">
    <skos:definition xml:lang="en">_</skos:definition>
    <skos:inScheme rdf:resource="http://www.geonames.org/ontology#P"/>
    <skos:prefLabel xml:lang="en">seat of a second-order administrative division</skos:prefLabel>
  </gn:Code>

  <gn:Code rdf:about="http://www.geonames.org/ontology#P.PPLA3">
    <skos:definition xml:lang="en">_</skos:definition>
    <skos:inScheme rdf:resource="http://www.geonames.org/ontology#P"/>
    <skos:prefLabel xml:lang="en">seat of a third-order administrative division</skos:prefLabel>
  </gn:Code>

  <gn:Code rdf:about="http://www.geonames.org/ontology#P.PPLA4">
    <skos:definition xml:lang="en">_</skos:definition>
    <skos:inScheme rdf:resource="http://www.geonames.org/ontology#P"/>
    <skos:prefLabel xml:lang="en">seat of a fourth-order administrative division</skos:prefLabel>
  </gn:Code>

  <gn:Code rdf:about="http://www.geonames.org/ontology#P.PPLC">
    <skos:definition xml:lang="en">_</skos:definition>
    <skos:inScheme rdf:resource="http://www.geonames.org/ontology#P"/>
    <skos:prefLabel xml:lang="en">capital of a political entity</skos:prefLabel>
  </gn:Code>

  <gn:Code rdf:about="http://www.geonames.org/ontology#P.PPLF">
    <skos:definition xml:lang="en">a populated place where the population is largely engaged in agricultural activities</skos:definition>
    <skos:inScheme rdf:resource="http://www.geonames.org/ontology#P"/>
    <skos:prefLabel xml:lang="en">farm village</skos:prefLabel>
  </gn:Code>

  <gn:Code rdf:about="http://www.geonames.org/ontology#P.PPLG">
    <skos:definition xml:lang="en">_</skos:definition>
    <skos:inScheme rdf:resource="http://www.geonames.org/ontology#P"/>
    <skos:prefLabel xml:lang="en">seat of government of a political entity</skos:prefLabel>
  </gn:Code>

  <gn:Code rdf:about="http://www.geonames.org/ontology#P.PPLL">
    <skos:definition xml:lang="en">an area similar to a locality but with a small group of dwellings or other buildings</skos:definition>
    <skos:inScheme rdf:resource="http://www.geonames.org/ontology#P"/>
    <skos:prefLabel xml:lang="en">populated locality</skos:prefLabel>
  </gn:Code>

  <gn:Code rdf:about="http://www.geonames.org/ontology#P.PPLQ">
    <skos:definition xml:lang="en">_</skos:definition>
    <skos:inScheme rdf:resource="http://www.geonames.org/ontology#P"/>
    <skos:prefLabel xml:lang="en">abandoned populated place</skos:prefLabel>
  </gn:Code>

  <gn:Code rdf:about="http://www.geonames.org/ontology#P.PPLR">
    <skos:definition xml:lang="en">a populated place whose population is largely engaged in religious occupations</skos:definition>
    <skos:inScheme rdf:resource="http://www.geonames.org/ontology#P"/>
    <skos:prefLabel xml:lang="en">religious populated place</skos:prefLabel>
  </gn:Code>

  <gn:Code rdf:about="http://www.geonames.org/ontology#P.PPLS">
    <skos:definition xml:lang="en">cities, towns, villages, or other agglomerations of buildings where people live and work</skos:definition>
    <skos:inScheme rdf:resource="http://www.geonames.org/ontology#P"/>
    <skos:prefLabel xml:lang="en">populated places</skos:prefLabel>
  </gn:Code>

  <gn:Code rdf:about="http://www.geonames.org/ontology#P.PPLW">
    <skos:definition xml:lang="en">a village, town or city destroyed by a natural disaster, or by war</skos:definition>
    <skos:inScheme rdf:resource="http://www.geonames.org/ontology#P"/>
    <skos:prefLabel xml:lang="en">destroyed populated place</skos:prefLabel>
  </gn:Code>

  <gn:Code rdf:about="http://www.geonames.org/ontology#P.PPLX">
    <skos:definition xml:lang="en">_</skos:definition>
    <skos:inScheme rdf:resource="http://www.geonames.org/ontology#P"/>
    <skos:prefLabel xml:lang="en">section of populated place</skos:prefLabel>
  </gn:Code>

  <gn:Code rdf:about="http://www.geonames.org/ontology#P.STLMT">
    <skos:definition xml:lang="en">_</skos:definition>
    <skos:inScheme rdf:resource="http://www.geonames.org/ontology#P"/>
    <skos:prefLabel xml:lang="en">israeli settlement</skos:prefLabel>
  </gn:Code>

  <gn:Class rdf:about="http://www.geonames.org/ontology#R">
    <rdfs:comment xml:lang="en">road, railroad, ...</rdfs:comment>
  </gn:Class>

  <gn:Code rdf:about="http://www.geonames.org/ontology#R.CSWY">
    <skos:definition xml:lang="en">a raised roadway across wet ground or shallow water</skos:definition>
    <skos:inScheme rdf:resource="http://www.geonames.org/ontology#R"/>
    <skos:prefLabel xml:lang="en">causeway</skos:prefLabel>
  </gn:Code>

  <gn:Code rdf:about="http://www.geonames.org/ontology#R.CSWYQ">
    <skos:definition xml:lang="en">a causeway no longer used for transportation</skos:definition>
    <skos:inScheme rdf:resource="http://www.geonames.org/ontology#R"/>
    <skos:prefLabel xml:lang="en">former causeway</skos:prefLabel>
  </gn:Code>

  <gn:Code rdf:about="http://www.geonames.org/ontology#R.OILP">
    <skos:definition xml:lang="en">a pipeline used for transporting oil</skos:definition>
    <skos:inScheme rdf:resource="http://www.geonames.org/ontology#R"/>
    <skos:prefLabel xml:lang="en">oil pipeline</skos:prefLabel>
  </gn:Code>

  <gn:Code rdf:about="http://www.geonames.org/ontology#R.PRMN">
    <skos:definition xml:lang="en">a place for public walking, usually along a beach front</skos:definition>
    <skos:inScheme rdf:resource="http://www.geonames.org/ontology#R"/>
    <skos:prefLabel xml:lang="en">promenade</skos:prefLabel>
  </gn:Code>

  <gn:Code rdf:about="http://www.geonames.org/ontology#R.PTGE">
    <skos:definition xml:lang="en">a place where boats, goods, etc., are carried overland between navigable waters</skos:definition>
    <skos:inScheme rdf:resource="http://www.geonames.org/ontology#R"/>
    <skos:prefLabel xml:lang="en">portage</skos:prefLabel>
  </gn:Code>

  <gn:Code rdf:about="http://www.geonames.org/ontology#R.RD">
    <skos:definition xml:lang="en">an open way with improved surface for transportation of animals, people and vehicles</skos:definition>
    <skos:inScheme rdf:resource="http://www.geonames.org/ontology#R"/>
    <skos:prefLabel xml:lang="en">road</skos:prefLabel>
  </gn:Code>

  <gn:Code rdf:about="http://www.geonames.org/ontology#R.RDA">
    <skos:definition xml:lang="en">the remains of a road used by ancient cultures</skos:definition>
    <skos:inScheme rdf:resource="http://www.geonames.org/ontology#R"/>
    <skos:prefLabel xml:lang="en">ancient road</skos:prefLabel>
  </gn:Code>

  <gn:Code rdf:about="http://www.geonames.org/ontology#R.RDB">
    <skos:definition xml:lang="en">a conspicuously curved or bent section of a road</skos:definition>
    <skos:inScheme rdf:resource="http://www.geonames.org/ontology#R"/>
    <skos:prefLabel xml:lang="en">road bend</skos:prefLabel>
  </gn:Code>

  <gn:Code rdf:about="http://www.geonames.org/ontology#R.RDCUT">
    <skos:definition xml:lang="en">an excavation cut through a hill or ridge for a road</skos:definition>
    <skos:inScheme rdf:resource="http://www.geonames.org/ontology#R"/>
    <skos:prefLabel xml:lang="en">road cut</skos:prefLabel>
  </gn:Code>

  <gn:Code rdf:about="http://www.geonames.org/ontology#R.RDJCT">
    <skos:definition xml:lang="en">a place where two or more roads join</skos:definition>
    <skos:inScheme rdf:resource="http://www.geonames.org/ontology#R"/>
    <skos:prefLabel xml:lang="en">road junction</skos:prefLabel>
  </gn:Code>

  <gn:Code rdf:about="http://www.geonames.org/ontology#R.RJCT">
    <skos:definition xml:lang="en">a place where two or more railroad tracks join</skos:definition>
    <skos:inScheme rdf:resource="http://www.geonames.org/ontology#R"/>
    <skos:prefLabel xml:lang="en">railroad junction</skos:prefLabel>
  </gn:Code>

  <gn:Code rdf:about="http://www.geonames.org/ontology#R.RR">
    <skos:definition xml:lang="en">a permanent twin steel-rail track on which freight and passenger cars move long distances</skos:definition>
    <skos:inScheme rdf:resource="http://www.geonames.org/ontology#R"/>
    <skos:prefLabel xml:lang="en">railroad</skos:prefLabel>
  </gn:Code>

  <gn:Code rdf:about="http://www.geonames.org/ontology#R.RRQ">
    <skos:definition xml:lang="en">_</skos:definition>
    <skos:inScheme rdf:resource="http://www.geonames.org/ontology#R"/>
    <skos:prefLabel xml:lang="en">abandoned railroad</skos:prefLabel>
  </gn:Code>

  <gn:Code rdf:about="http://www.geonames.org/ontology#R.RTE">
    <skos:definition xml:lang="en">the route taken by caravans</skos:definition>
    <skos:inScheme rdf:resource="http://www.geonames.org/ontology#R"/>
    <skos:prefLabel xml:lang="en">caravan route</skos:prefLabel>
  </gn:Code>

  <gn:Code rdf:about="http://www.geonames.org/ontology#R.RYD">
    <skos:definition xml:lang="en">a system of tracks used for the making up of trains, and switching and storing freight cars</skos:definition>
    <skos:inScheme rdf:resource="http://www.geonames.org/ontology#R"/>
    <skos:prefLabel xml:lang="en">railroad yard</skos:prefLabel>
  </gn:Code>

  <gn:Code rdf:about="http://www.geonames.org/ontology#R.ST">
    <skos:definition xml:lang="en">a paved urban thoroughfare</skos:definition>
    <skos:inScheme rdf:resource="http://www.geonames.org/ontology#R"/>
    <skos:prefLabel xml:lang="en">street</skos:prefLabel>
  </gn:Code>

  <gn:Code rdf:about="http://www.geonames.org/ontology#R.STKR">
    <skos:definition xml:lang="en">a route taken by livestock herds</skos:definition>
    <skos:inScheme rdf:resource="http://www.geonames.org/ontology#R"/>
    <skos:prefLabel xml:lang="en">stock route</skos:prefLabel>
  </gn:Code>

  <gn:Code rdf:about="http://www.geonames.org/ontology#R.TNL">
    <skos:definition xml:lang="en">a subterranean passageway for transportation</skos:definition>
    <skos:inScheme rdf:resource="http://www.geonames.org/ontology#R"/>
    <skos:prefLabel xml:lang="en">tunnel</skos:prefLabel>
  </gn:Code>

  <gn:Code rdf:about="http://www.geonames.org/ontology#R.TNLN">
    <skos:definition xml:lang="en">a cave that is open at both ends</skos:definition>
    <skos:inScheme rdf:resource="http://www.geonames.org/ontology#R"/>
    <skos:prefLabel xml:lang="en">natural tunnel</skos:prefLabel>
  </gn:Code>

  <gn:Code rdf:about="http://www.geonames.org/ontology#R.TNLRD">
    <skos:definition xml:lang="en">a tunnel through which a road passes</skos:definition>
    <skos:inScheme rdf:resource="http://www.geonames.org/ontology#R"/>
    <skos:prefLabel xml:lang="en">road tunnel</skos:prefLabel>
  </gn:Code>

  <gn:Code rdf:about="http://www.geonames.org/ontology#R.TNLRR">
    <skos:definition xml:lang="en">a tunnel through which a railroad passes</skos:definition>
    <skos:inScheme rdf:resource="http://www.geonames.org/ontology#R"/>
    <skos:prefLabel xml:lang="en">railroad tunnel</skos:prefLabel>
  </gn:Code>

  <gn:Code rdf:about="http://www.geonames.org/ontology#R.TNLS">
    <skos:definition xml:lang="en">subterranean passageways for transportation</skos:definition>
    <skos:inScheme rdf:resource="http://www.geonames.org/ontology#R"/>
    <skos:prefLabel xml:lang="en">tunnels</skos:prefLabel>
  </gn:Code>

  <gn:Code rdf:about="http://www.geonames.org/ontology#R.TRL">
    <skos:definition xml:lang="en">a path, track, or route used by pedestrians, animals, or off-road vehicles</skos:definition>
    <skos:inScheme rdf:resource="http://www.geonames.org/ontology#R"/>
    <skos:prefLabel xml:lang="en">trail</skos:prefLabel>
  </gn:Code>

  <gn:Class rdf:about="http://www.geonames.org/ontology#S">
    <rdfs:comment xml:lang="en">spot, building, farm, ...</rdfs:comment>
  </gn:Class>

  <gn:Code rdf:about="http://www.geonames.org/ontology#S.ADMF">
    <skos:definition xml:lang="en">a government building</skos:definition>
    <skos:inScheme rdf:resource="http://www.geonames.org/ontology#S"/>
    <skos:prefLabel xml:lang="en">administrative facility</skos:prefLabel>
  </gn:Code>

  <gn:Code rdf:about="http://www.geonames.org/ontology#S.AGRF">
    <skos:definition xml:lang="en">a building and/or tract of land used for improving agriculture</skos:definition>
    <skos:inScheme rdf:resource="http://www.geonames.org/ontology#S"/>
    <skos:prefLabel xml:lang="en">agricultural facility</skos:prefLabel>
  </gn:Code>

  <gn:Code rdf:about="http://www.geonames.org/ontology#S.AIRB">
    <skos:definition xml:lang="en">an area used to store supplies, provide barracks for air force personnel, hangars and runways for aircraft, and from which operations are initiated</skos:definition>
    <skos:inScheme rdf:resource="http://www.geonames.org/ontology#S"/>
    <skos:prefLabel xml:lang="en">airbase</skos:prefLabel>
  </gn:Code>

  <gn:Code rdf:about="http://www.geonames.org/ontology#S.AIRF">
    <skos:definition xml:lang="en">a place on land where aircraft land and take off; no facilities provided for the commercial handling of passengers and cargo</skos:definition>
    <skos:inScheme rdf:resource="http://www.geonames.org/ontology#S"/>
    <skos:prefLabel xml:lang="en">airfield</skos:prefLabel>
  </gn:Code>

  <gn:Code rdf:about="http://www.geonames.org/ontology#S.AIRH">
    <skos:definition xml:lang="en">a place where helicopters land and take off</skos:definition>
    <skos:inScheme rdf:resource="http://www.geonames.org/ontology#S"/>
    <skos:prefLabel xml:lang="en">heliport</skos:prefLabel>
  </gn:Code>

  <gn:Code rdf:about="http://www.geonames.org/ontology#S.AIRP">
    <skos:definition xml:lang="en">a place where aircraft regularly land and take off, with runways, navigational aids, and major facilities for the commercial handling of passengers and cargo</skos:definition>
    <skos:inScheme rdf:resource="http://www.geonames.org/ontology#S"/>
    <skos:prefLabel xml:lang="en">airport</skos:prefLabel>
  </gn:Code>

  <gn:Code rdf:about="http://www.geonames.org/ontology#S.AIRQ">
    <skos:definition xml:lang="en">_</skos:definition>
    <skos:inScheme rdf:resource="http://www.geonames.org/ontology#S"/>
    <skos:prefLabel xml:lang="en">abandoned airfield</skos:prefLabel>
  </gn:Code>

  <gn:Code rdf:about="http://www.geonames.org/ontology#S.AMTH">
    <skos:definition xml:lang="en">an oval or circular structure with rising tiers of seats about a stage or open space</skos:definition>
    <skos:inScheme rdf:resource="http://www.geonames.org/ontology#S"/>
    <skos:prefLabel xml:lang="en">amphitheater</skos:prefLabel>
  </gn:Code>

  <gn:Code rdf:about="http://www.geonames.org/ontology#S.ANS">
    <skos:definition xml:lang="en">a place where archeological remains, old structures, or cultural artifacts are located</skos:definition>
    <skos:inScheme rdf:resource="http://www.geonames.org/ontology#S"/>
    <skos:prefLabel xml:lang="en">ancient site</skos:prefLabel>
  </gn:Code>

  <gn:Code rdf:about="http://www.geonames.org/ontology#S.ARCH">
    <skos:definition xml:lang="en">a natural or man-made structure in the form of an arch</skos:definition>
    <skos:inScheme rdf:resource="http://www.geonames.org/ontology#S"/>
    <skos:prefLabel xml:lang="en">arch</skos:prefLabel>
  </gn:Code>

  <gn:Code rdf:about="http://www.geonames.org/ontology#S.ASTR">
    <skos:definition xml:lang="en">a point on the earth whose position has been determined by observations of celestial bodies</skos:definition>
    <skos:inScheme rdf:resource="http://www.geonames.org/ontology#S"/>
    <skos:prefLabel xml:lang="en">astronomical station</skos:prefLabel>
  </gn:Code>

  <gn:Code rdf:about="http://www.geonames.org/ontology#S.ASYL">
    <skos:definition xml:lang="en">a facility where the insane are cared for and protected</skos:definition>
    <skos:inScheme rdf:resource="http://www.geonames.org/ontology#S"/>
    <skos:prefLabel xml:lang="en">asylum</skos:prefLabel>
  </gn:Code>

  <gn:Code rdf:about="http://www.geonames.org/ontology#S.ATHF">
    <skos:definition xml:lang="en">a tract of land used for playing team sports, and athletic track and field events</skos:definition>
    <skos:inScheme rdf:resource="http://www.geonames.org/ontology#S"/>
    <skos:prefLabel xml:lang="en">athletic field</skos:prefLabel>
  </gn:Code>

  <gn:Code rdf:about="http://www.geonames.org/ontology#S.ATM">
    <skos:definition xml:lang="en">An unattended electronic machine in a public place, connected to a data system and related equipment and activated by a bank customer to obtain cash withdrawals and other banking services.</skos:definition>
    <skos:inScheme rdf:resource="http://www.geonames.org/ontology#S"/>
    <skos:prefLabel xml:lang="en">automatic teller machine</skos:prefLabel>
  </gn:Code>

  <gn:Code rdf:about="http://www.geonames.org/ontology#S.BANK">
    <skos:definition xml:lang="en">A business establishment in which money is kept for saving or commercial purposes or is invested, supplied for loans, or exchanged.</skos:definition>
    <skos:inScheme rdf:resource="http://www.geonames.org/ontology#S"/>
    <skos:prefLabel xml:lang="en">bank</skos:prefLabel>
  </gn:Code>

  <gn:Code rdf:about="http://www.geonames.org/ontology#S.BCN">
    <skos:definition xml:lang="en">a fixed artificial navigation mark</skos:definition>
    <skos:inScheme rdf:resource="http://www.geonames.org/ontology#S"/>
    <skos:prefLabel xml:lang="en">beacon</skos:prefLabel>
  </gn:Code>

  <gn:Code rdf:about="http://www.geonames.org/ontology#S.BDG">
    <skos:definition xml:lang="en">a structure erected across an obstacle such as a stream, road, etc., in order to carry roads, railroads, and pedestrians across</skos:definition>
    <skos:inScheme rdf:resource="http://www.geonames.org/ontology#S"/>
    <skos:prefLabel xml:lang="en">bridge</skos:prefLabel>
  </gn:Code>

  <gn:Code rdf:about="http://www.geonames.org/ontology#S.BDGQ">
    <skos:definition xml:lang="en">a destroyed or decayed bridge which is no longer functional</skos:definition>
    <skos:inScheme rdf:resource="http://www.geonames.org/ontology#S"/>
    <skos:prefLabel xml:lang="en">ruined bridge</skos:prefLabel>
  </gn:Code>

  <gn:Code rdf:about="http://www.geonames.org/ontology#S.BLDG">
    <skos:definition xml:lang="en">a structure built for permanent use, as a house, factory, etc.</skos:definition>
    <skos:inScheme rdf:resource="http://www.geonames.org/ontology#S"/>
    <skos:prefLabel xml:lang="en">building(s)</skos:prefLabel>
  </gn:Code>

  <gn:Code rdf:about="http://www.geonames.org/ontology#S.BP">
    <skos:definition xml:lang="en">a fixture marking a point along a boundary</skos:definition>
    <skos:inScheme rdf:resource="http://www.geonames.org/ontology#S"/>
    <skos:prefLabel xml:lang="en">boundary marker</skos:prefLabel>
  </gn:Code>

  <gn:Code rdf:about="http://www.geonames.org/ontology#S.BRKS">
    <skos:definition xml:lang="en">a building for lodging military personnel</skos:definition>
    <skos:inScheme rdf:resource="http://www.geonames.org/ontology#S"/>
    <skos:prefLabel xml:lang="en">barracks</skos:prefLabel>
  </gn:Code>

  <gn:Code rdf:about="http://www.geonames.org/ontology#S.BRKW">
    <skos:definition xml:lang="en">a structure erected to break the force of waves at the entrance to a harbor or port</skos:definition>
    <skos:inScheme rdf:resource="http://www.geonames.org/ontology#S"/>
    <skos:prefLabel xml:lang="en">breakwater</skos:prefLabel>
  </gn:Code>

  <gn:Code rdf:about="http://www.geonames.org/ontology#S.BSTN">
    <skos:definition xml:lang="en">a facility for baling agricultural products</skos:definition>
    <skos:inScheme rdf:resource="http://www.geonames.org/ontology#S"/>
    <skos:prefLabel xml:lang="en">baling station</skos:prefLabel>
  </gn:Code>

  <gn:Code rdf:about="http://www.geonames.org/ontology#S.BTYD">
    <skos:definition xml:lang="en">a waterside facility for servicing, repairing, and building small vessels</skos:definition>
    <skos:inScheme rdf:resource="http://www.geonames.org/ontology#S"/>
    <skos:prefLabel xml:lang="en">boatyard</skos:prefLabel>
  </gn:Code>

  <gn:Code rdf:about="http://www.geonames.org/ontology#S.BUR">
    <skos:definition xml:lang="en">a cave used for human burials</skos:definition>
    <skos:inScheme rdf:resource="http://www.geonames.org/ontology#S"/>
    <skos:prefLabel xml:lang="en">burial cave(s)</skos:prefLabel>
  </gn:Code>

  <gn:Code rdf:about="http://www.geonames.org/ontology#S.BUSTN">
    <skos:definition xml:lang="en">a facility comprising ticket office, platforms, etc. for loading and unloading passengers</skos:definition>
    <skos:inScheme rdf:resource="http://www.geonames.org/ontology#S"/>
    <skos:prefLabel xml:lang="en">Bus Station</skos:prefLabel>
  </gn:Code>

  <gn:Code rdf:about="http://www.geonames.org/ontology#S.BUSTP">
    <skos:definition xml:lang="en">a place lacking station facilities</skos:definition>
    <skos:inScheme rdf:resource="http://www.geonames.org/ontology#S"/>
    <skos:prefLabel xml:lang="en">Bus Stop</skos:prefLabel>
  </gn:Code>

  <gn:Code rdf:about="http://www.geonames.org/ontology#S.CARN">
    <skos:definition xml:lang="en">a heap of stones erected as a landmark or for other purposes</skos:definition>
    <skos:inScheme rdf:resource="http://www.geonames.org/ontology#S"/>
    <skos:prefLabel xml:lang="en">cairn</skos:prefLabel>
  </gn:Code>

  <gn:Code rdf:about="http://www.geonames.org/ontology#S.CAVE">
    <skos:definition xml:lang="en">an underground passageway or chamber, or cavity on the side of a cliff</skos:definition>
    <skos:inScheme rdf:resource="http://www.geonames.org/ontology#S"/>
    <skos:prefLabel xml:lang="en">cave(s)</skos:prefLabel>
  </gn:Code>

  <gn:Code rdf:about="http://www.geonames.org/ontology#S.CCL">
    <skos:definition xml:lang="en">Centres for Continuous Learning</skos:definition>
    <skos:inScheme rdf:resource="http://www.geonames.org/ontology#S"/>
    <skos:prefLabel xml:lang="en">Centre Continuous Learning</skos:prefLabel>
  </gn:Code>

  <gn:Code rdf:about="http://www.geonames.org/ontology#S.CH">
    <skos:definition xml:lang="en">a building for public Christian worship</skos:definition>
    <skos:inScheme rdf:resource="http://www.geonames.org/ontology#S"/>
    <skos:prefLabel xml:lang="en">church</skos:prefLabel>
  </gn:Code>

  <gn:Code rdf:about="http://www.geonames.org/ontology#S.CMP">
    <skos:definition xml:lang="en">a site occupied by tents, huts, or other shelters for temporary use</skos:definition>
    <skos:inScheme rdf:resource="http://www.geonames.org/ontology#S"/>
    <skos:prefLabel xml:lang="en">camp(s)</skos:prefLabel>
  </gn:Code>

  <gn:Code rdf:about="http://www.geonames.org/ontology#S.CMPL">
    <skos:definition xml:lang="en">a camp used by loggers</skos:definition>
    <skos:inScheme rdf:resource="http://www.geonames.org/ontology#S"/>
    <skos:prefLabel xml:lang="en">logging camp</skos:prefLabel>
  </gn:Code>

  <gn:Code rdf:about="http://www.geonames.org/ontology#S.CMPLA">
    <skos:definition xml:lang="en">a camp used by migrant or temporary laborers</skos:definition>
    <skos:inScheme rdf:resource="http://www.geonames.org/ontology#S"/>
    <skos:prefLabel xml:lang="en">labor camp</skos:prefLabel>
  </gn:Code>

  <gn:Code rdf:about="http://www.geonames.org/ontology#S.CMPMN">
    <skos:definition xml:lang="en">a camp used by miners</skos:definition>
    <skos:inScheme rdf:resource="http://www.geonames.org/ontology#S"/>
    <skos:prefLabel xml:lang="en">mining camp</skos:prefLabel>
  </gn:Code>

  <gn:Code rdf:about="http://www.geonames.org/ontology#S.CMPO">
    <skos:definition xml:lang="en">a camp used by oilfield workers</skos:definition>
    <skos:inScheme rdf:resource="http://www.geonames.org/ontology#S"/>
    <skos:prefLabel xml:lang="en">oil camp</skos:prefLabel>
  </gn:Code>

  <gn:Code rdf:about="http://www.geonames.org/ontology#S.CMPQ">
    <skos:definition xml:lang="en">_</skos:definition>
    <skos:inScheme rdf:resource="http://www.geonames.org/ontology#S"/>
    <skos:prefLabel xml:lang="en">abandoned camp</skos:prefLabel>
  </gn:Code>

  <gn:Code rdf:about="http://www.geonames.org/ontology#S.CMPRF">
    <skos:definition xml:lang="en">a camp used by refugees</skos:definition>
    <skos:inScheme rdf:resource="http://www.geonames.org/ontology#S"/>
    <skos:prefLabel xml:lang="en">refugee camp</skos:prefLabel>
  </gn:Code>

  <gn:Code rdf:about="http://www.geonames.org/ontology#S.CMTY">
    <skos:definition xml:lang="en">a burial place or ground</skos:definition>
    <skos:inScheme rdf:resource="http://www.geonames.org/ontology#S"/>
    <skos:prefLabel xml:lang="en">cemetery</skos:prefLabel>
  </gn:Code>

  <gn:Code rdf:about="http://www.geonames.org/ontology#S.COMC">
    <skos:definition xml:lang="en">a facility, including buildings, antennae, towers and electronic equipment for receiving and transmitting information</skos:definition>
    <skos:inScheme rdf:resource="http://www.geonames.org/ontology#S"/>
    <skos:prefLabel xml:lang="en">communication center</skos:prefLabel>
  </gn:Code>

  <gn:Code rdf:about="http://www.geonames.org/ontology#S.CRRL">
    <skos:definition xml:lang="en">a pen or enclosure for confining or capturing animals</skos:definition>
    <skos:inScheme rdf:resource="http://www.geonames.org/ontology#S"/>
    <skos:prefLabel xml:lang="en">corral(s)</skos:prefLabel>
  </gn:Code>

  <gn:Code rdf:about="http://www.geonames.org/ontology#S.CSNO">
    <skos:definition xml:lang="en">a building used for entertainment, especially gambling</skos:definition>
    <skos:inScheme rdf:resource="http://www.geonames.org/ontology#S"/>
    <skos:prefLabel xml:lang="en">casino</skos:prefLabel>
  </gn:Code>

  <gn:Code rdf:about="http://www.geonames.org/ontology#S.CSTL">
    <skos:definition xml:lang="en">a large fortified building or set of buildings</skos:definition>
    <skos:inScheme rdf:resource="http://www.geonames.org/ontology#S"/>
    <skos:prefLabel xml:lang="en">castle</skos:prefLabel>
  </gn:Code>

  <gn:Code rdf:about="http://www.geonames.org/ontology#S.CSTM">
    <skos:definition xml:lang="en">a building in a port where customs and duties are paid, and where vessels are entered and cleared</skos:definition>
    <skos:inScheme rdf:resource="http://www.geonames.org/ontology#S"/>
    <skos:prefLabel xml:lang="en">customs house</skos:prefLabel>
  </gn:Code>

  <gn:Code rdf:about="http://www.geonames.org/ontology#S.CTHSE">
    <skos:definition xml:lang="en">a building in which courts of law are held</skos:definition>
    <skos:inScheme rdf:resource="http://www.geonames.org/ontology#S"/>
    <skos:prefLabel xml:lang="en">courthouse</skos:prefLabel>
  </gn:Code>

  <gn:Code rdf:about="http://www.geonames.org/ontology#S.CTRA">
    <skos:definition xml:lang="en">a facility where atomic research is carried out</skos:definition>
    <skos:inScheme rdf:resource="http://www.geonames.org/ontology#S"/>
    <skos:prefLabel xml:lang="en">atomic center</skos:prefLabel>
  </gn:Code>

  <gn:Code rdf:about="http://www.geonames.org/ontology#S.CTRCM">
    <skos:definition xml:lang="en">a facility for community recreation and other activities</skos:definition>
    <skos:inScheme rdf:resource="http://www.geonames.org/ontology#S"/>
    <skos:prefLabel xml:lang="en">community center</skos:prefLabel>
  </gn:Code>

  <gn:Code rdf:about="http://www.geonames.org/ontology#S.CTRF">
    <skos:definition xml:lang="en">a place where more than one facility is situated</skos:definition>
    <skos:inScheme rdf:resource="http://www.geonames.org/ontology#S"/>
    <skos:prefLabel xml:lang="en">facility center</skos:prefLabel>
  </gn:Code>

  <gn:Code rdf:about="http://www.geonames.org/ontology#S.CTRM">
    <skos:definition xml:lang="en">a complex of health care buildings including two or more of the following: hospital, medical school, clinic, pharmacy, doctor's offices, etc.</skos:definition>
    <skos:inScheme rdf:resource="http://www.geonames.org/ontology#S"/>
    <skos:prefLabel xml:lang="en">medical center</skos:prefLabel>
  </gn:Code>

  <gn:Code rdf:about="http://www.geonames.org/ontology#S.CTRR">
    <skos:definition xml:lang="en">a facility where more than one religious activity is carried out, e.g., retreat, school, monastery, worship</skos:definition>
    <skos:inScheme rdf:resource="http://www.geonames.org/ontology#S"/>
    <skos:prefLabel xml:lang="en">religious center</skos:prefLabel>
  </gn:Code>

  <gn:Code rdf:about="http://www.geonames.org/ontology#S.CTRS">
    <skos:definition xml:lang="en">a facility for launching, tracking, or controlling satellites and space vehicles</skos:definition>
    <skos:inScheme rdf:resource="http://www.geonames.org/ontology#S"/>
    <skos:prefLabel xml:lang="en">space center</skos:prefLabel>
  </gn:Code>

  <gn:Code rdf:about="http://www.geonames.org/ontology#S.CVNT">
    <skos:definition xml:lang="en">a building where a community of nuns lives in seclusion</skos:definition>
    <skos:inScheme rdf:resource="http://www.geonames.org/ontology#S"/>
    <skos:prefLabel xml:lang="en">convent</skos:prefLabel>
  </gn:Code>

  <gn:Code rdf:about="http://www.geonames.org/ontology#S.DAM">
    <skos:definition xml:lang="en">a barrier constructed across a stream to impound water</skos:definition>
    <skos:inScheme rdf:resource="http://www.geonames.org/ontology#S"/>
    <skos:prefLabel xml:lang="en">dam</skos:prefLabel>
  </gn:Code>

  <gn:Code rdf:about="http://www.geonames.org/ontology#S.DAMQ">
    <skos:definition xml:lang="en">a destroyed or decayed dam which is no longer functional</skos:definition>
    <skos:inScheme rdf:resource="http://www.geonames.org/ontology#S"/>
    <skos:prefLabel xml:lang="en">ruined dam</skos:prefLabel>
  </gn:Code>

  <gn:Code rdf:about="http://www.geonames.org/ontology#S.DAMSB">
    <skos:definition xml:lang="en">a dam put down to bedrock in a sand river</skos:definition>
    <skos:inScheme rdf:resource="http://www.geonames.org/ontology#S"/>
    <skos:prefLabel xml:lang="en">sub-surface dam</skos:prefLabel>
  </gn:Code>

  <gn:Code rdf:about="http://www.geonames.org/ontology#S.DARY">
    <skos:definition xml:lang="en">a facility for the processing, sale and distribution of milk or milk products</skos:definition>
    <skos:inScheme rdf:resource="http://www.geonames.org/ontology#S"/>
    <skos:prefLabel xml:lang="en">dairy</skos:prefLabel>
  </gn:Code>

  <gn:Code rdf:about="http://www.geonames.org/ontology#S.DCKD">
    <skos:definition xml:lang="en">a dock providing support for a vessel, and means for removing the water so that the bottom of the vessel can be exposed</skos:definition>
    <skos:inScheme rdf:resource="http://www.geonames.org/ontology#S"/>
    <skos:prefLabel xml:lang="en">dry dock</skos:prefLabel>
  </gn:Code>

  <gn:Code rdf:about="http://www.geonames.org/ontology#S.DCKY">
    <skos:definition xml:lang="en">a facility for servicing, building, or repairing ships</skos:definition>
    <skos:inScheme rdf:resource="http://www.geonames.org/ontology#S"/>
    <skos:prefLabel xml:lang="en">dockyard</skos:prefLabel>
  </gn:Code>

  <gn:Code rdf:about="http://www.geonames.org/ontology#S.DIKE">
    <skos:definition xml:lang="en">an earth or stone embankment usually constructed for flood or stream control</skos:definition>
    <skos:inScheme rdf:resource="http://www.geonames.org/ontology#S"/>
    <skos:prefLabel xml:lang="en">dike</skos:prefLabel>
  </gn:Code>

  <gn:Code rdf:about="http://www.geonames.org/ontology#S.DPOF">
    <skos:definition xml:lang="en">an area where fuel is stored</skos:definition>
    <skos:inScheme rdf:resource="http://www.geonames.org/ontology#S"/>
    <skos:prefLabel xml:lang="en">fuel depot</skos:prefLabel>
  </gn:Code>

  <gn:Code rdf:about="http://www.geonames.org/ontology#S.EST">
    <skos:definition xml:lang="en">a large commercialized agricultural landholding with associated buildings and other facilities</skos:definition>
    <skos:inScheme rdf:resource="http://www.geonames.org/ontology#S"/>
    <skos:prefLabel xml:lang="en">estate(s)</skos:prefLabel>
  </gn:Code>

  <gn:Code rdf:about="http://www.geonames.org/ontology#S.ESTB">
    <skos:definition xml:lang="en">an estate that specializes in the growing of bananas</skos:definition>
    <skos:inScheme rdf:resource="http://www.geonames.org/ontology#S"/>
    <skos:prefLabel xml:lang="en">banana plantation</skos:prefLabel>
  </gn:Code>

  <gn:Code rdf:about="http://www.geonames.org/ontology#S.ESTC">
    <skos:definition xml:lang="en">an estate specializing in the cultivation of cotton</skos:definition>
    <skos:inScheme rdf:resource="http://www.geonames.org/ontology#S"/>
    <skos:prefLabel xml:lang="en">cotton plantation</skos:prefLabel>
  </gn:Code>

  <gn:Code rdf:about="http://www.geonames.org/ontology#S.ESTO">
    <skos:definition xml:lang="en">an estate specializing in the cultivation of oil palm trees</skos:definition>
    <skos:inScheme rdf:resource="http://www.geonames.org/ontology#S"/>
    <skos:prefLabel xml:lang="en">oil palm plantation</skos:prefLabel>
  </gn:Code>

  <gn:Code rdf:about="http://www.geonames.org/ontology#S.ESTR">
    <skos:definition xml:lang="en">an estate which specializes in growing and tapping rubber trees</skos:definition>
    <skos:inScheme rdf:resource="http://www.geonames.org/ontology#S"/>
    <skos:prefLabel xml:lang="en">rubber plantation</skos:prefLabel>
  </gn:Code>

  <gn:Code rdf:about="http://www.geonames.org/ontology#S.ESTSG">
    <skos:definition xml:lang="en">an estate that specializes in growing sugar cane</skos:definition>
    <skos:inScheme rdf:resource="http://www.geonames.org/ontology#S"/>
    <skos:prefLabel xml:lang="en">sugar plantation</skos:prefLabel>
  </gn:Code>

  <gn:Code rdf:about="http://www.geonames.org/ontology#S.ESTSL">
    <skos:definition xml:lang="en">an estate that specializes in growing sisal</skos:definition>
    <skos:inScheme rdf:resource="http://www.geonames.org/ontology#S"/>
    <skos:prefLabel xml:lang="en">sisal plantation</skos:prefLabel>
  </gn:Code>

  <gn:Code rdf:about="http://www.geonames.org/ontology#S.ESTT">
    <skos:definition xml:lang="en">an estate which specializes in growing tea bushes</skos:definition>
    <skos:inScheme rdf:resource="http://www.geonames.org/ontology#S"/>
    <skos:prefLabel xml:lang="en">tea plantation</skos:prefLabel>
  </gn:Code>

  <gn:Code rdf:about="http://www.geonames.org/ontology#S.ESTX">
    <skos:definition xml:lang="en">_</skos:definition>
    <skos:inScheme rdf:resource="http://www.geonames.org/ontology#S"/>
    <skos:prefLabel xml:lang="en">section of estate</skos:prefLabel>
  </gn:Code>

  <gn:Code rdf:about="http://www.geonames.org/ontology#S.FCL">
    <skos:definition xml:lang="en">a building or buildings housing a center, institute, foundation, hospital, prison, mission, courthouse, etc.</skos:definition>
    <skos:inScheme rdf:resource="http://www.geonames.org/ontology#S"/>
    <skos:prefLabel xml:lang="en">facility</skos:prefLabel>
  </gn:Code>

  <gn:Code rdf:about="http://www.geonames.org/ontology#S.FNDY">
    <skos:definition xml:lang="en">a building or works where metal casting is carried out</skos:definition>
    <skos:inScheme rdf:resource="http://www.geonames.org/ontology#S"/>
    <skos:prefLabel xml:lang="en">foundry</skos:prefLabel>
  </gn:Code>

  <gn:Code rdf:about="http://www.geonames.org/ontology#S.FRM">
    <skos:definition xml:lang="en">a tract of land with associated buildings devoted to agriculture</skos:definition>
    <skos:inScheme rdf:resource="http://www.geonames.org/ontology#S"/>
    <skos:prefLabel xml:lang="en">farm</skos:prefLabel>
  </gn:Code>

  <gn:Code rdf:about="http://www.geonames.org/ontology#S.FRMQ">
    <skos:definition xml:lang="en">_</skos:definition>
    <skos:inScheme rdf:resource="http://www.geonames.org/ontology#S"/>
    <skos:prefLabel xml:lang="en">abandoned farm</skos:prefLabel>
  </gn:Code>

  <gn:Code rdf:about="http://www.geonames.org/ontology#S.FRMS">
    <skos:definition xml:lang="en">tracts of land with associated buildings devoted to agriculture</skos:definition>
    <skos:inScheme rdf:resource="http://www.geonames.org/ontology#S"/>
    <skos:prefLabel xml:lang="en">farms</skos:prefLabel>
  </gn:Code>

  <gn:Code rdf:about="http://www.geonames.org/ontology#S.FRMT">
    <skos:definition xml:lang="en">the buildings and adjacent service areas of a farm</skos:definition>
    <skos:inScheme rdf:resource="http://www.geonames.org/ontology#S"/>
    <skos:prefLabel xml:lang="en">farmstead</skos:prefLabel>
  </gn:Code>

  <gn:Code rdf:about="http://www.geonames.org/ontology#S.FT">
    <skos:definition xml:lang="en">a defensive structure or earthworks</skos:definition>
    <skos:inScheme rdf:resource="http://www.geonames.org/ontology#S"/>
    <skos:prefLabel xml:lang="en">fort</skos:prefLabel>
  </gn:Code>

  <gn:Code rdf:about="http://www.geonames.org/ontology#S.FY">
    <skos:definition xml:lang="en">a boat or other floating conveyance and terminal facilities regularly used to transport people and vehicles across a waterbody</skos:definition>
    <skos:inScheme rdf:resource="http://www.geonames.org/ontology#S"/>
    <skos:prefLabel xml:lang="en">ferry</skos:prefLabel>
  </gn:Code>

  <gn:Code rdf:about="http://www.geonames.org/ontology#S.GATE">
    <skos:definition xml:lang="en">a controlled access entrance or exit</skos:definition>
    <skos:inScheme rdf:resource="http://www.geonames.org/ontology#S"/>
    <skos:prefLabel xml:lang="en">gate</skos:prefLabel>
  </gn:Code>

  <gn:Code rdf:about="http://www.geonames.org/ontology#S.GDN">
    <skos:definition xml:lang="en">an enclosure for displaying selected plant or animal life</skos:definition>
    <skos:inScheme rdf:resource="http://www.geonames.org/ontology#S"/>
    <skos:prefLabel xml:lang="en">garden(s)</skos:prefLabel>
  </gn:Code>

  <gn:Code rdf:about="http://www.geonames.org/ontology#S.GHSE">
    <skos:definition xml:lang="en">a house used to provide lodging for paying guests</skos:definition>
    <skos:inScheme rdf:resource="http://www.geonames.org/ontology#S"/>
    <skos:prefLabel xml:lang="en">guest house</skos:prefLabel>
  </gn:Code>

  <gn:Code rdf:about="http://www.geonames.org/ontology#S.GOSP">
    <skos:definition xml:lang="en">a facility for separating gas from oil</skos:definition>
    <skos:inScheme rdf:resource="http://www.geonames.org/ontology#S"/>
    <skos:prefLabel xml:lang="en">gas-oil separator plant</skos:prefLabel>
  </gn:Code>

  <gn:Code rdf:about="http://www.geonames.org/ontology#S.GRVE">
    <skos:definition xml:lang="en">a burial site</skos:definition>
    <skos:inScheme rdf:resource="http://www.geonames.org/ontology#S"/>
    <skos:prefLabel xml:lang="en">grave</skos:prefLabel>
  </gn:Code>

  <gn:Code rdf:about="http://www.geonames.org/ontology#S.HERM">
    <skos:definition xml:lang="en">a secluded residence, usually for religious sects</skos:definition>
    <skos:inScheme rdf:resource="http://www.geonames.org/ontology#S"/>
    <skos:prefLabel xml:lang="en">hermitage</skos:prefLabel>
  </gn:Code>

  <gn:Code rdf:about="http://www.geonames.org/ontology#S.HLT">
    <skos:definition xml:lang="en">a place where caravans stop for rest</skos:definition>
    <skos:inScheme rdf:resource="http://www.geonames.org/ontology#S"/>
    <skos:prefLabel xml:lang="en">halting place</skos:prefLabel>
  </gn:Code>

  <gn:Code rdf:about="http://www.geonames.org/ontology#S.HSE">
    <skos:definition xml:lang="en">a building used as a human habitation</skos:definition>
    <skos:inScheme rdf:resource="http://www.geonames.org/ontology#S"/>
    <skos:prefLabel xml:lang="en">house(s)</skos:prefLabel>
  </gn:Code>

  <gn:Code rdf:about="http://www.geonames.org/ontology#S.HSEC">
    <skos:definition xml:lang="en">a large house, mansion, or chateau, on a large estate</skos:definition>
    <skos:inScheme rdf:resource="http://www.geonames.org/ontology#S"/>
    <skos:prefLabel xml:lang="en">country house</skos:prefLabel>
  </gn:Code>

  <gn:Code rdf:about="http://www.geonames.org/ontology#S.HSP">
    <skos:definition xml:lang="en">a building in which sick or injured, especially those confined to bed, are medically treated</skos:definition>
    <skos:inScheme rdf:resource="http://www.geonames.org/ontology#S"/>
    <skos:prefLabel xml:lang="en">hospital</skos:prefLabel>
  </gn:Code>

  <gn:Code rdf:about="http://www.geonames.org/ontology#S.HSPC">
    <skos:definition xml:lang="en">a medical facility associated with a hospital for outpatients</skos:definition>
    <skos:inScheme rdf:resource="http://www.geonames.org/ontology#S"/>
    <skos:prefLabel xml:lang="en">clinic</skos:prefLabel>
  </gn:Code>

  <gn:Code rdf:about="http://www.geonames.org/ontology#S.HSPD">
    <skos:definition xml:lang="en">a building where medical or dental aid is dispensed</skos:definition>
    <skos:inScheme rdf:resource="http://www.geonames.org/ontology#S"/>
    <skos:prefLabel xml:lang="en">dispensary</skos:prefLabel>
  </gn:Code>

  <gn:Code rdf:about="http://www.geonames.org/ontology#S.HSPL">
    <skos:definition xml:lang="en">an asylum or hospital for lepers</skos:definition>
    <skos:inScheme rdf:resource="http://www.geonames.org/ontology#S"/>
    <skos:prefLabel xml:lang="en">leprosarium</skos:prefLabel>
  </gn:Code>

  <gn:Code rdf:about="http://www.geonames.org/ontology#S.HSTS">
    <skos:definition xml:lang="en">a place of historical importance</skos:definition>
    <skos:inScheme rdf:resource="http://www.geonames.org/ontology#S"/>
    <skos:prefLabel xml:lang="en">historical site</skos:prefLabel>
  </gn:Code>

  <gn:Code rdf:about="http://www.geonames.org/ontology#S.HTL">
    <skos:definition xml:lang="en">a building providing lodging and/or meals for the public</skos:definition>
    <skos:inScheme rdf:resource="http://www.geonames.org/ontology#S"/>
    <skos:prefLabel xml:lang="en">hotel</skos:prefLabel>
  </gn:Code>

  <gn:Code rdf:about="http://www.geonames.org/ontology#S.HUT">
    <skos:definition xml:lang="en">a small primitive house</skos:definition>
    <skos:inScheme rdf:resource="http://www.geonames.org/ontology#S"/>
    <skos:prefLabel xml:lang="en">hut</skos:prefLabel>
  </gn:Code>

  <gn:Code rdf:about="http://www.geonames.org/ontology#S.HUTS">
    <skos:definition xml:lang="en">small primitive houses</skos:definition>
    <skos:inScheme rdf:resource="http://www.geonames.org/ontology#S"/>
    <skos:prefLabel xml:lang="en">huts</skos:prefLabel>
  </gn:Code>

  <gn:Code rdf:about="http://www.geonames.org/ontology#S.INSM">
    <skos:definition xml:lang="en">a facility for use of and control by armed forces</skos:definition>
    <skos:inScheme rdf:resource="http://www.geonames.org/ontology#S"/>
    <skos:prefLabel xml:lang="en">military installation</skos:prefLabel>
  </gn:Code>

  <gn:Code rdf:about="http://www.geonames.org/ontology#S.ITTR">
    <skos:definition xml:lang="en">a facility where research is carried out</skos:definition>
    <skos:inScheme rdf:resource="http://www.geonames.org/ontology#S"/>
    <skos:prefLabel xml:lang="en">research institute</skos:prefLabel>
  </gn:Code>

  <gn:Code rdf:about="http://www.geonames.org/ontology#S.JTY">
    <skos:definition xml:lang="en">a structure built out into the water at a river mouth or harbor entrance to regulate currents and silting</skos:definition>
    <skos:inScheme rdf:resource="http://www.geonames.org/ontology#S"/>
    <skos:prefLabel xml:lang="en">jetty</skos:prefLabel>
  </gn:Code>

  <gn:Code rdf:about="http://www.geonames.org/ontology#S.LDNG">
    <skos:definition xml:lang="en">a place where boats receive or discharge passengers and freight, but lacking most port facilities</skos:definition>
    <skos:inScheme rdf:resource="http://www.geonames.org/ontology#S"/>
    <skos:prefLabel xml:lang="en">landing</skos:prefLabel>
  </gn:Code>

  <gn:Code rdf:about="http://www.geonames.org/ontology#S.LEPC">
    <skos:definition xml:lang="en">a settled area inhabited by lepers in relative isolation</skos:definition>
    <skos:inScheme rdf:resource="http://www.geonames.org/ontology#S"/>
    <skos:prefLabel xml:lang="en">leper colony</skos:prefLabel>
  </gn:Code>

  <gn:Code rdf:about="http://www.geonames.org/ontology#S.LIBR">
    <skos:definition xml:lang="en">A place in which information resources such as books are kept for reading, reference, or lending.</skos:definition>
    <skos:inScheme rdf:resource="http://www.geonames.org/ontology#S"/>
    <skos:prefLabel xml:lang="en">library</skos:prefLabel>
  </gn:Code>

  <gn:Code rdf:about="http://www.geonames.org/ontology#S.LNDF">
    <skos:definition xml:lang="en">a place for trash and garbage disposal in which the waste is buried between layers of earth to build up low-lying land</skos:definition>
    <skos:inScheme rdf:resource="http://www.geonames.org/ontology#S"/>
    <skos:prefLabel xml:lang="en">landfill</skos:prefLabel>
  </gn:Code>

  <gn:Code rdf:about="http://www.geonames.org/ontology#S.LOCK">
    <skos:definition xml:lang="en">a basin in a waterway with gates at each end by means of which vessels are passed from one water level to another</skos:definition>
    <skos:inScheme rdf:resource="http://www.geonames.org/ontology#S"/>
    <skos:prefLabel xml:lang="en">lock(s)</skos:prefLabel>
  </gn:Code>

  <gn:Code rdf:about="http://www.geonames.org/ontology#S.LTHSE">
    <skos:definition xml:lang="en">a distinctive structure exhibiting a major navigation light</skos:definition>
    <skos:inScheme rdf:resource="http://www.geonames.org/ontology#S"/>
    <skos:prefLabel xml:lang="en">lighthouse</skos:prefLabel>
  </gn:Code>

  <gn:Code rdf:about="http://www.geonames.org/ontology#S.MALL">
    <skos:definition xml:lang="en">A large, often enclosed shopping complex containing various stores, businesses, and restaurants usually accessible by common passageways.</skos:definition>
    <skos:inScheme rdf:resource="http://www.geonames.org/ontology#S"/>
    <skos:prefLabel xml:lang="en">mall</skos:prefLabel>
  </gn:Code>

  <gn:Code rdf:about="http://www.geonames.org/ontology#S.MAR">
    <skos:definition xml:lang="en">a harbor facility for small boats, yachts, etc.</skos:definition>
    <skos:inScheme rdf:resource="http://www.geonames.org/ontology#S"/>
    <skos:prefLabel xml:lang="en">marina</skos:prefLabel>
  </gn:Code>

  <gn:Code rdf:about="http://www.geonames.org/ontology#S.MFG">
    <skos:definition xml:lang="en">one or more buildings where goods are manufactured, processed or fabricated</skos:definition>
    <skos:inScheme rdf:resource="http://www.geonames.org/ontology#S"/>
    <skos:prefLabel xml:lang="en">factory</skos:prefLabel>
  </gn:Code>

  <gn:Code rdf:about="http://www.geonames.org/ontology#S.MFGB">
    <skos:definition xml:lang="en">one or more buildings where beer is brewed</skos:definition>
    <skos:inScheme rdf:resource="http://www.geonames.org/ontology#S"/>
    <skos:prefLabel xml:lang="en">brewery</skos:prefLabel>
  </gn:Code>

  <gn:Code rdf:about="http://www.geonames.org/ontology#S.MFGC">
    <skos:definition xml:lang="en">a building where food items are canned</skos:definition>
    <skos:inScheme rdf:resource="http://www.geonames.org/ontology#S"/>
    <skos:prefLabel xml:lang="en">cannery</skos:prefLabel>
  </gn:Code>

  <gn:Code rdf:about="http://www.geonames.org/ontology#S.MFGCU">
    <skos:definition xml:lang="en">a facility for processing copper ore</skos:definition>
    <skos:inScheme rdf:resource="http://www.geonames.org/ontology#S"/>
    <skos:prefLabel xml:lang="en">copper works</skos:prefLabel>
  </gn:Code>

  <gn:Code rdf:about="http://www.geonames.org/ontology#S.MFGLM">
    <skos:definition xml:lang="en">a furnace in which limestone is reduced to lime</skos:definition>
    <skos:inScheme rdf:resource="http://www.geonames.org/ontology#S"/>
    <skos:prefLabel xml:lang="en">limekiln</skos:prefLabel>
  </gn:Code>

  <gn:Code rdf:about="http://www.geonames.org/ontology#S.MFGM">
    <skos:definition xml:lang="en">a factory where ammunition is made</skos:definition>
    <skos:inScheme rdf:resource="http://www.geonames.org/ontology#S"/>
    <skos:prefLabel xml:lang="en">munitions plant</skos:prefLabel>
  </gn:Code>

  <gn:Code rdf:about="http://www.geonames.org/ontology#S.MFGPH">
    <skos:definition xml:lang="en">a facility for producing fertilizer</skos:definition>
    <skos:inScheme rdf:resource="http://www.geonames.org/ontology#S"/>
    <skos:prefLabel xml:lang="en">phosphate works</skos:prefLabel>
  </gn:Code>

  <gn:Code rdf:about="http://www.geonames.org/ontology#S.MFGQ">
    <skos:definition xml:lang="en">_</skos:definition>
    <skos:inScheme rdf:resource="http://www.geonames.org/ontology#S"/>
    <skos:prefLabel xml:lang="en">abandoned factory</skos:prefLabel>
  </gn:Code>

  <gn:Code rdf:about="http://www.geonames.org/ontology#S.MFGSG">
    <skos:definition xml:lang="en">a facility for converting raw sugar into refined sugar</skos:definition>
    <skos:inScheme rdf:resource="http://www.geonames.org/ontology#S"/>
    <skos:prefLabel xml:lang="en">sugar refinery</skos:prefLabel>
  </gn:Code>

  <gn:Code rdf:about="http://www.geonames.org/ontology#S.MKT">
    <skos:definition xml:lang="en">a place where goods are bought and sold at regular intervals</skos:definition>
    <skos:inScheme rdf:resource="http://www.geonames.org/ontology#S"/>
    <skos:prefLabel xml:lang="en">market</skos:prefLabel>
  </gn:Code>

  <gn:Code rdf:about="http://www.geonames.org/ontology#S.ML">
    <skos:definition xml:lang="en">a building housing machines for transforming, shaping, finishing, grinding, or extracting products</skos:definition>
    <skos:inScheme rdf:resource="http://www.geonames.org/ontology#S"/>
    <skos:prefLabel xml:lang="en">mill(s)</skos:prefLabel>
  </gn:Code>

  <gn:Code rdf:about="http://www.geonames.org/ontology#S.MLM">
    <skos:definition xml:lang="en">a facility for improving the metal content of ore by concentration</skos:definition>
    <skos:inScheme rdf:resource="http://www.geonames.org/ontology#S"/>
    <skos:prefLabel xml:lang="en">ore treatment plant</skos:prefLabel>
  </gn:Code>

  <gn:Code rdf:about="http://www.geonames.org/ontology#S.MLO">
    <skos:definition xml:lang="en">a mill where oil is extracted from olives</skos:definition>
    <skos:inScheme rdf:resource="http://www.geonames.org/ontology#S"/>
    <skos:prefLabel xml:lang="en">olive oil mill</skos:prefLabel>
  </gn:Code>

  <gn:Code rdf:about="http://www.geonames.org/ontology#S.MLSG">
    <skos:definition xml:lang="en">a facility where sugar cane is processed into raw sugar</skos:definition>
    <skos:inScheme rdf:resource="http://www.geonames.org/ontology#S"/>
    <skos:prefLabel xml:lang="en">sugar mill</skos:prefLabel>
  </gn:Code>

  <gn:Code rdf:about="http://www.geonames.org/ontology#S.MLSGQ">
    <skos:definition xml:lang="en">a sugar mill no longer used as a sugar mill</skos:definition>
    <skos:inScheme rdf:resource="http://www.geonames.org/ontology#S"/>
    <skos:prefLabel xml:lang="en">former sugar mill</skos:prefLabel>
  </gn:Code>

  <gn:Code rdf:about="http://www.geonames.org/ontology#S.MLSW">
    <skos:definition xml:lang="en">a mill where logs or lumber are sawn to specified shapes and sizes</skos:definition>
    <skos:inScheme rdf:resource="http://www.geonames.org/ontology#S"/>
    <skos:prefLabel xml:lang="en">sawmill</skos:prefLabel>
  </gn:Code>

  <gn:Code rdf:about="http://www.geonames.org/ontology#S.MLWND">
    <skos:definition xml:lang="en">a mill or water pump powered by wind</skos:definition>
    <skos:inScheme rdf:resource="http://www.geonames.org/ontology#S"/>
    <skos:prefLabel xml:lang="en">windmill</skos:prefLabel>
  </gn:Code>

  <gn:Code rdf:about="http://www.geonames.org/ontology#S.MLWTR">
    <skos:definition xml:lang="en">a mill powered by running water</skos:definition>
    <skos:inScheme rdf:resource="http://www.geonames.org/ontology#S"/>
    <skos:prefLabel xml:lang="en">water mill</skos:prefLabel>
  </gn:Code>

  <gn:Code rdf:about="http://www.geonames.org/ontology#S.MN">
    <skos:definition xml:lang="en">a site where mineral ores are extracted from the ground by excavating surface pits and subterranean passages</skos:definition>
    <skos:inScheme rdf:resource="http://www.geonames.org/ontology#S"/>
    <skos:prefLabel xml:lang="en">mine(s)</skos:prefLabel>
  </gn:Code>

  <gn:Code rdf:about="http://www.geonames.org/ontology#S.MNAU">
    <skos:definition xml:lang="en">a mine where gold ore, or alluvial gold is extracted</skos:definition>
    <skos:inScheme rdf:resource="http://www.geonames.org/ontology#S"/>
    <skos:prefLabel xml:lang="en">gold mine(s)</skos:prefLabel>
  </gn:Code>

  <gn:Code rdf:about="http://www.geonames.org/ontology#S.MNC">
    <skos:definition xml:lang="en">a mine where coal is extracted</skos:definition>
    <skos:inScheme rdf:resource="http://www.geonames.org/ontology#S"/>
    <skos:prefLabel xml:lang="en">coal mine(s)</skos:prefLabel>
  </gn:Code>

  <gn:Code rdf:about="http://www.geonames.org/ontology#S.MNCR">
    <skos:definition xml:lang="en">a mine where chrome ore is extracted</skos:definition>
    <skos:inScheme rdf:resource="http://www.geonames.org/ontology#S"/>
    <skos:prefLabel xml:lang="en">chrome mine(s)</skos:prefLabel>
  </gn:Code>

  <gn:Code rdf:about="http://www.geonames.org/ontology#S.MNCU">
    <skos:definition xml:lang="en">a mine where copper ore is extracted</skos:definition>
    <skos:inScheme rdf:resource="http://www.geonames.org/ontology#S"/>
    <skos:prefLabel xml:lang="en">copper mine(s)</skos:prefLabel>
  </gn:Code>

  <gn:Code rdf:about="http://www.geonames.org/ontology#S.MNDT">
    <skos:definition xml:lang="en">a place where diatomaceous earth is extracted</skos:definition>
    <skos:inScheme rdf:resource="http://www.geonames.org/ontology#S"/>
    <skos:prefLabel xml:lang="en">diatomite mine(s)</skos:prefLabel>
  </gn:Code>

  <gn:Code rdf:about="http://www.geonames.org/ontology#S.MNFE">
    <skos:definition xml:lang="en">a mine where iron ore is extracted</skos:definition>
    <skos:inScheme rdf:resource="http://www.geonames.org/ontology#S"/>
    <skos:prefLabel xml:lang="en">iron mine(s)</skos:prefLabel>
  </gn:Code>

  <gn:Code rdf:about="http://www.geonames.org/ontology#S.MNMT">
    <skos:definition xml:lang="en">a commemorative structure or statue</skos:definition>
    <skos:inScheme rdf:resource="http://www.geonames.org/ontology#S"/>
    <skos:prefLabel xml:lang="en">monument</skos:prefLabel>
  </gn:Code>

  <gn:Code rdf:about="http://www.geonames.org/ontology#S.MNN">
    <skos:definition xml:lang="en">a mine from which salt is extracted</skos:definition>
    <skos:inScheme rdf:resource="http://www.geonames.org/ontology#S"/>
    <skos:prefLabel xml:lang="en">salt mine(s)</skos:prefLabel>
  </gn:Code>

  <gn:Code rdf:about="http://www.geonames.org/ontology#S.MNNI">
    <skos:definition xml:lang="en">a mine where nickel ore is extracted</skos:definition>
    <skos:inScheme rdf:resource="http://www.geonames.org/ontology#S"/>
    <skos:prefLabel xml:lang="en">nickel mine(s)</skos:prefLabel>
  </gn:Code>

  <gn:Code rdf:about="http://www.geonames.org/ontology#S.MNPB">
    <skos:definition xml:lang="en">a mine where lead ore is extracted</skos:definition>
    <skos:inScheme rdf:resource="http://www.geonames.org/ontology#S"/>
    <skos:prefLabel xml:lang="en">lead mine(s)</skos:prefLabel>
  </gn:Code>

  <gn:Code rdf:about="http://www.geonames.org/ontology#S.MNPL">
    <skos:definition xml:lang="en">a place where heavy metals are concentrated and running water is used to extract them from unconsolidated sediments</skos:definition>
    <skos:inScheme rdf:resource="http://www.geonames.org/ontology#S"/>
    <skos:prefLabel xml:lang="en">placer mine(s)</skos:prefLabel>
  </gn:Code>

  <gn:Code rdf:about="http://www.geonames.org/ontology#S.MNQ">
    <skos:definition xml:lang="en">_</skos:definition>
    <skos:inScheme rdf:resource="http://www.geonames.org/ontology#S"/>
    <skos:prefLabel xml:lang="en">abandoned mine</skos:prefLabel>
  </gn:Code>

  <gn:Code rdf:about="http://www.geonames.org/ontology#S.MNQR">
    <skos:definition xml:lang="en">a surface mine where building stone or gravel and sand, etc. are extracted</skos:definition>
    <skos:inScheme rdf:resource="http://www.geonames.org/ontology#S"/>
    <skos:prefLabel xml:lang="en">quarry(-ies)</skos:prefLabel>
  </gn:Code>

  <gn:Code rdf:about="http://www.geonames.org/ontology#S.MNSN">
    <skos:definition xml:lang="en">a mine where tin ore is extracted</skos:definition>
    <skos:inScheme rdf:resource="http://www.geonames.org/ontology#S"/>
    <skos:prefLabel xml:lang="en">tin mine(s)</skos:prefLabel>
  </gn:Code>

  <gn:Code rdf:about="http://www.geonames.org/ontology#S.MOLE">
    <skos:definition xml:lang="en">a massive structure of masonry or large stones serving as a pier or breakwater</skos:definition>
    <skos:inScheme rdf:resource="http://www.geonames.org/ontology#S"/>
    <skos:prefLabel xml:lang="en">mole</skos:prefLabel>
  </gn:Code>

  <gn:Code rdf:about="http://www.geonames.org/ontology#S.MSQE">
    <skos:definition xml:lang="en">a building for public Islamic worship</skos:definition>
    <skos:inScheme rdf:resource="http://www.geonames.org/ontology#S"/>
    <skos:prefLabel xml:lang="en">mosque</skos:prefLabel>
  </gn:Code>

  <gn:Code rdf:about="http://www.geonames.org/ontology#S.MSSN">
    <skos:definition xml:lang="en">a place characterized by dwellings, school, church, hospital and other facilities operated by a religious group for the purpose of providing charitable services and to propagate religion</skos:definition>
    <skos:inScheme rdf:resource="http://www.geonames.org/ontology#S"/>
    <skos:prefLabel xml:lang="en">mission</skos:prefLabel>
  </gn:Code>

  <gn:Code rdf:about="http://www.geonames.org/ontology#S.MSSNQ">
    <skos:definition xml:lang="en">_</skos:definition>
    <skos:inScheme rdf:resource="http://www.geonames.org/ontology#S"/>
    <skos:prefLabel xml:lang="en">abandoned mission</skos:prefLabel>
  </gn:Code>

  <gn:Code rdf:about="http://www.geonames.org/ontology#S.MSTY">
    <skos:definition xml:lang="en">a building and grounds where a community of monks lives in seclusion</skos:definition>
    <skos:inScheme rdf:resource="http://www.geonames.org/ontology#S"/>
    <skos:prefLabel xml:lang="en">monastery</skos:prefLabel>
  </gn:Code>

  <gn:Code rdf:about="http://www.geonames.org/ontology#S.MTRO">
    <skos:definition xml:lang="en">metro station (Underground, Tube, or Métro)</skos:definition>
    <skos:inScheme rdf:resource="http://www.geonames.org/ontology#S"/>
    <skos:prefLabel xml:lang="en">metro station</skos:prefLabel>
  </gn:Code>

  <gn:Code rdf:about="http://www.geonames.org/ontology#S.MUS">
    <skos:definition xml:lang="en">a building where objects of permanent interest in one or more of the arts and sciences are preserved and exhibited</skos:definition>
    <skos:inScheme rdf:resource="http://www.geonames.org/ontology#S"/>
    <skos:prefLabel xml:lang="en">museum</skos:prefLabel>
  </gn:Code>

  <gn:Code rdf:about="http://www.geonames.org/ontology#S.NOV">
    <skos:definition xml:lang="en">a religious house or school where novices are trained</skos:definition>
    <skos:inScheme rdf:resource="http://www.geonames.org/ontology#S"/>
    <skos:prefLabel xml:lang="en">novitiate</skos:prefLabel>
  </gn:Code>

  <gn:Code rdf:about="http://www.geonames.org/ontology#S.NSY">
    <skos:definition xml:lang="en">a place where plants are propagated for transplanting or grafting</skos:definition>
    <skos:inScheme rdf:resource="http://www.geonames.org/ontology#S"/>
    <skos:prefLabel xml:lang="en">nursery(-ies)</skos:prefLabel>
  </gn:Code>

  <gn:Code rdf:about="http://www.geonames.org/ontology#S.OBPT">
    <skos:definition xml:lang="en">a wildlife or scenic observation point</skos:definition>
    <skos:inScheme rdf:resource="http://www.geonames.org/ontology#S"/>
    <skos:prefLabel xml:lang="en">observation point</skos:prefLabel>
  </gn:Code>

  <gn:Code rdf:about="http://www.geonames.org/ontology#S.OBS">
    <skos:definition xml:lang="en">a facility equipped for observation of atmospheric or space phenomena</skos:definition>
    <skos:inScheme rdf:resource="http://www.geonames.org/ontology#S"/>
    <skos:prefLabel xml:lang="en">observatory</skos:prefLabel>
  </gn:Code>

  <gn:Code rdf:about="http://www.geonames.org/ontology#S.OBSR">
    <skos:definition xml:lang="en">a facility equipped with an array of antennae for receiving radio waves from space</skos:definition>
    <skos:inScheme rdf:resource="http://www.geonames.org/ontology#S"/>
    <skos:prefLabel xml:lang="en">radio observatory</skos:prefLabel>
  </gn:Code>

  <gn:Code rdf:about="http://www.geonames.org/ontology#S.OILJ">
    <skos:definition xml:lang="en">a section of an oil pipeline where two or more pipes join together</skos:definition>
    <skos:inScheme rdf:resource="http://www.geonames.org/ontology#S"/>
    <skos:prefLabel xml:lang="en">oil pipeline junction</skos:prefLabel>
  </gn:Code>

  <gn:Code rdf:about="http://www.geonames.org/ontology#S.OILQ">
    <skos:definition xml:lang="en">_</skos:definition>
    <skos:inScheme rdf:resource="http://www.geonames.org/ontology#S"/>
    <skos:prefLabel xml:lang="en">abandoned oil well</skos:prefLabel>
  </gn:Code>

  <gn:Code rdf:about="http://www.geonames.org/ontology#S.OILR">
    <skos:definition xml:lang="en">a facility for converting crude oil into refined petroleum products</skos:definition>
    <skos:inScheme rdf:resource="http://www.geonames.org/ontology#S"/>
    <skos:prefLabel xml:lang="en">oil refinery</skos:prefLabel>
  </gn:Code>

  <gn:Code rdf:about="http://www.geonames.org/ontology#S.OILT">
    <skos:definition xml:lang="en">a tract of land occupied by large, cylindrical, metal tanks in which oil or liquid petrochemicals are stored</skos:definition>
    <skos:inScheme rdf:resource="http://www.geonames.org/ontology#S"/>
    <skos:prefLabel xml:lang="en">tank farm</skos:prefLabel>
  </gn:Code>

  <gn:Code rdf:about="http://www.geonames.org/ontology#S.OILW">
    <skos:definition xml:lang="en">a well from which oil may be pumped</skos:definition>
    <skos:inScheme rdf:resource="http://www.geonames.org/ontology#S"/>
    <skos:prefLabel xml:lang="en">oil well</skos:prefLabel>
  </gn:Code>

  <gn:Code rdf:about="http://www.geonames.org/ontology#S.OPRA">
    <skos:definition xml:lang="en">A theater designed chiefly for the performance of operas.</skos:definition>
    <skos:inScheme rdf:resource="http://www.geonames.org/ontology#S"/>
    <skos:prefLabel xml:lang="en">opera house</skos:prefLabel>
  </gn:Code>

  <gn:Code rdf:about="http://www.geonames.org/ontology#S.PAL">
    <skos:definition xml:lang="en">a large stately house, often a royal or presidential residence</skos:definition>
    <skos:inScheme rdf:resource="http://www.geonames.org/ontology#S"/>
    <skos:prefLabel xml:lang="en">palace</skos:prefLabel>
  </gn:Code>

  <gn:Code rdf:about="http://www.geonames.org/ontology#S.PGDA">
    <skos:definition xml:lang="en">a tower-like storied structure, usually a Buddhist shrine</skos:definition>
    <skos:inScheme rdf:resource="http://www.geonames.org/ontology#S"/>
    <skos:prefLabel xml:lang="en">pagoda</skos:prefLabel>
  </gn:Code>

  <gn:Code rdf:about="http://www.geonames.org/ontology#S.PIER">
    <skos:definition xml:lang="en">a structure built out into navigable water on piles providing berthing for ships and recreation</skos:definition>
    <skos:inScheme rdf:resource="http://www.geonames.org/ontology#S"/>
    <skos:prefLabel xml:lang="en">pier</skos:prefLabel>
  </gn:Code>

  <gn:Code rdf:about="http://www.geonames.org/ontology#S.PKLT">
    <skos:definition xml:lang="en">an area used for parking vehicles</skos:definition>
    <skos:inScheme rdf:resource="http://www.geonames.org/ontology#S"/>
    <skos:prefLabel xml:lang="en">parking lot</skos:prefLabel>
  </gn:Code>

  <gn:Code rdf:about="http://www.geonames.org/ontology#S.PMPO">
    <skos:definition xml:lang="en">a facility for pumping oil through a pipeline</skos:definition>
    <skos:inScheme rdf:resource="http://www.geonames.org/ontology#S"/>
    <skos:prefLabel xml:lang="en">oil pumping station</skos:prefLabel>
  </gn:Code>

  <gn:Code rdf:about="http://www.geonames.org/ontology#S.PMPW">
    <skos:definition xml:lang="en">a facility for pumping water from a major well or through a pipeline</skos:definition>
    <skos:inScheme rdf:resource="http://www.geonames.org/ontology#S"/>
    <skos:prefLabel xml:lang="en">water pumping station</skos:prefLabel>
  </gn:Code>

  <gn:Code rdf:about="http://www.geonames.org/ontology#S.PO">
    <skos:definition xml:lang="en">a public building in which mail is received, sorted and distributed</skos:definition>
    <skos:inScheme rdf:resource="http://www.geonames.org/ontology#S"/>
    <skos:prefLabel xml:lang="en">post office</skos:prefLabel>
  </gn:Code>

  <gn:Code rdf:about="http://www.geonames.org/ontology#S.PP">
    <skos:definition xml:lang="en">a building in which police are stationed</skos:definition>
    <skos:inScheme rdf:resource="http://www.geonames.org/ontology#S"/>
    <skos:prefLabel xml:lang="en">police post</skos:prefLabel>
  </gn:Code>

  <gn:Code rdf:about="http://www.geonames.org/ontology#S.PPQ">
    <skos:definition xml:lang="en">_</skos:definition>
    <skos:inScheme rdf:resource="http://www.geonames.org/ontology#S"/>
    <skos:prefLabel xml:lang="en">abandoned police post</skos:prefLabel>
  </gn:Code>

  <gn:Code rdf:about="http://www.geonames.org/ontology#S.PRKGT">
    <skos:definition xml:lang="en">a controlled access to a park</skos:definition>
    <skos:inScheme rdf:resource="http://www.geonames.org/ontology#S"/>
    <skos:prefLabel xml:lang="en">park gate</skos:prefLabel>
  </gn:Code>

  <gn:Code rdf:about="http://www.geonames.org/ontology#S.PRKHQ">
    <skos:definition xml:lang="en">a park administrative facility</skos:definition>
    <skos:inScheme rdf:resource="http://www.geonames.org/ontology#S"/>
    <skos:prefLabel xml:lang="en">park headquarters</skos:prefLabel>
  </gn:Code>

  <gn:Code rdf:about="http://www.geonames.org/ontology#S.PRN">
    <skos:definition xml:lang="en">a facility for confining prisoners</skos:definition>
    <skos:inScheme rdf:resource="http://www.geonames.org/ontology#S"/>
    <skos:prefLabel xml:lang="en">prison</skos:prefLabel>
  </gn:Code>

  <gn:Code rdf:about="http://www.geonames.org/ontology#S.PRNJ">
    <skos:definition xml:lang="en">a facility for confining, training, and reforming young law offenders</skos:definition>
    <skos:inScheme rdf:resource="http://www.geonames.org/ontology#S"/>
    <skos:prefLabel xml:lang="en">reformatory</skos:prefLabel>
  </gn:Code>

  <gn:Code rdf:about="http://www.geonames.org/ontology#S.PRNQ">
    <skos:definition xml:lang="en">_</skos:definition>
    <skos:inScheme rdf:resource="http://www.geonames.org/ontology#S"/>
    <skos:prefLabel xml:lang="en">abandoned prison</skos:prefLabel>
  </gn:Code>

  <gn:Code rdf:about="http://www.geonames.org/ontology#S.PS">
    <skos:definition xml:lang="en">a facility for generating electric power</skos:definition>
    <skos:inScheme rdf:resource="http://www.geonames.org/ontology#S"/>
    <skos:prefLabel xml:lang="en">power station</skos:prefLabel>
  </gn:Code>

  <gn:Code rdf:about="http://www.geonames.org/ontology#S.PSH">
    <skos:definition xml:lang="en">a building where electricity is generated from water power</skos:definition>
    <skos:inScheme rdf:resource="http://www.geonames.org/ontology#S"/>
    <skos:prefLabel xml:lang="en">hydroelectric power station</skos:prefLabel>
  </gn:Code>

  <gn:Code rdf:about="http://www.geonames.org/ontology#S.PSTB">
    <skos:definition xml:lang="en">a post or station at an international boundary for the regulation of movement of people and goods</skos:definition>
    <skos:inScheme rdf:resource="http://www.geonames.org/ontology#S"/>
    <skos:prefLabel xml:lang="en">border post</skos:prefLabel>
  </gn:Code>

  <gn:Code rdf:about="http://www.geonames.org/ontology#S.PSTC">
    <skos:definition xml:lang="en">a building at an international boundary where customs and duties are paid on goods</skos:definition>
    <skos:inScheme rdf:resource="http://www.geonames.org/ontology#S"/>
    <skos:prefLabel xml:lang="en">customs post</skos:prefLabel>
  </gn:Code>

  <gn:Code rdf:about="http://www.geonames.org/ontology#S.PSTP">
    <skos:definition xml:lang="en">a post from which patrols are sent out</skos:definition>
    <skos:inScheme rdf:resource="http://www.geonames.org/ontology#S"/>
    <skos:prefLabel xml:lang="en">patrol post</skos:prefLabel>
  </gn:Code>

  <gn:Code rdf:about="http://www.geonames.org/ontology#S.PYR">
    <skos:definition xml:lang="en">an ancient massive structure of square ground plan with four triangular faces meeting at a point and used for enclosing tombs</skos:definition>
    <skos:inScheme rdf:resource="http://www.geonames.org/ontology#S"/>
    <skos:prefLabel xml:lang="en">pyramid</skos:prefLabel>
  </gn:Code>

  <gn:Code rdf:about="http://www.geonames.org/ontology#S.PYRS">
    <skos:definition xml:lang="en">ancient massive structures of square ground plan with four triangular faces meeting at a point and used for enclosing tombs</skos:definition>
    <skos:inScheme rdf:resource="http://www.geonames.org/ontology#S"/>
    <skos:prefLabel xml:lang="en">pyramids</skos:prefLabel>
  </gn:Code>

  <gn:Code rdf:about="http://www.geonames.org/ontology#S.QUAY">
    <skos:definition xml:lang="en">a structure of solid construction along a shore or bank which provides berthing for ships and which generally provides cargo handling facilities</skos:definition>
    <skos:inScheme rdf:resource="http://www.geonames.org/ontology#S"/>
    <skos:prefLabel xml:lang="en">quay</skos:prefLabel>
  </gn:Code>

  <gn:Code rdf:about="http://www.geonames.org/ontology#S.RECG">
    <skos:definition xml:lang="en">a recreation field where golf is played</skos:definition>
    <skos:inScheme rdf:resource="http://www.geonames.org/ontology#S"/>
    <skos:prefLabel xml:lang="en">golf course</skos:prefLabel>
  </gn:Code>

  <gn:Code rdf:about="http://www.geonames.org/ontology#S.RECR">
    <skos:definition xml:lang="en">a track where races are held</skos:definition>
    <skos:inScheme rdf:resource="http://www.geonames.org/ontology#S"/>
    <skos:prefLabel xml:lang="en">racetrack</skos:prefLabel>
  </gn:Code>

  <gn:Code rdf:about="http://www.geonames.org/ontology#S.REST">
    <skos:definition xml:lang="en">A place where meals are served to the public</skos:definition>
    <skos:inScheme rdf:resource="http://www.geonames.org/ontology#S"/>
    <skos:prefLabel xml:lang="en">restaurant</skos:prefLabel>
  </gn:Code>

  <gn:Code rdf:about="http://www.geonames.org/ontology#S.RHSE">
    <skos:definition xml:lang="en">a structure maintained for the rest and shelter of travelers</skos:definition>
    <skos:inScheme rdf:resource="http://www.geonames.org/ontology#S"/>
    <skos:prefLabel xml:lang="en">resthouse</skos:prefLabel>
  </gn:Code>

  <gn:Code rdf:about="http://www.geonames.org/ontology#S.RKRY">
    <skos:definition xml:lang="en">a breeding place of a colony of birds or seals</skos:definition>
    <skos:inScheme rdf:resource="http://www.geonames.org/ontology#S"/>
    <skos:prefLabel xml:lang="en">rookery</skos:prefLabel>
  </gn:Code>

  <gn:Code rdf:about="http://www.geonames.org/ontology#S.RLG">
    <skos:definition xml:lang="en">an ancient site of significant religious importance</skos:definition>
    <skos:inScheme rdf:resource="http://www.geonames.org/ontology#S"/>
    <skos:prefLabel xml:lang="en">religious site</skos:prefLabel>
  </gn:Code>

  <gn:Code rdf:about="http://www.geonames.org/ontology#S.RLGR">
    <skos:definition xml:lang="en">a place of temporary seclusion, especially for religious groups</skos:definition>
    <skos:inScheme rdf:resource="http://www.geonames.org/ontology#S"/>
    <skos:prefLabel xml:lang="en">retreat</skos:prefLabel>
  </gn:Code>

  <gn:Code rdf:about="http://www.geonames.org/ontology#S.RNCH">
    <skos:definition xml:lang="en">a large farm specializing in extensive grazing of livestock</skos:definition>
    <skos:inScheme rdf:resource="http://www.geonames.org/ontology#S"/>
    <skos:prefLabel xml:lang="en">ranch(es)</skos:prefLabel>
  </gn:Code>

  <gn:Code rdf:about="http://www.geonames.org/ontology#S.RSD">
    <skos:definition xml:lang="en">a short track parallel to and joining the main track</skos:definition>
    <skos:inScheme rdf:resource="http://www.geonames.org/ontology#S"/>
    <skos:prefLabel xml:lang="en">railroad siding</skos:prefLabel>
  </gn:Code>

  <gn:Code rdf:about="http://www.geonames.org/ontology#S.RSGNL">
    <skos:definition xml:lang="en">a signal at the entrance of a particular section of track governing the movement of trains</skos:definition>
    <skos:inScheme rdf:resource="http://www.geonames.org/ontology#S"/>
    <skos:prefLabel xml:lang="en">railroad signal</skos:prefLabel>
  </gn:Code>

  <gn:Code rdf:about="http://www.geonames.org/ontology#S.RSRT">
    <skos:definition xml:lang="en">a specialized facility for vacation, health, or participation sports activities</skos:definition>
    <skos:inScheme rdf:resource="http://www.geonames.org/ontology#S"/>
    <skos:prefLabel xml:lang="en">resort</skos:prefLabel>
  </gn:Code>

  <gn:Code rdf:about="http://www.geonames.org/ontology#S.RSTN">
    <skos:definition xml:lang="en">a facility comprising ticket office, platforms, etc. for loading and unloading train passengers and freight</skos:definition>
    <skos:inScheme rdf:resource="http://www.geonames.org/ontology#S"/>
    <skos:prefLabel xml:lang="en">railroad station</skos:prefLabel>
  </gn:Code>

  <gn:Code rdf:about="http://www.geonames.org/ontology#S.RSTNQ">
    <skos:definition xml:lang="en">_</skos:definition>
    <skos:inScheme rdf:resource="http://www.geonames.org/ontology#S"/>
    <skos:prefLabel xml:lang="en">abandoned railroad station</skos:prefLabel>
  </gn:Code>

  <gn:Code rdf:about="http://www.geonames.org/ontology#S.RSTP">
    <skos:definition xml:lang="en">a place lacking station facilities where trains stop to pick up and unload passengers and freight</skos:definition>
    <skos:inScheme rdf:resource="http://www.geonames.org/ontology#S"/>
    <skos:prefLabel xml:lang="en">railroad stop</skos:prefLabel>
  </gn:Code>

  <gn:Code rdf:about="http://www.geonames.org/ontology#S.RSTPQ">
    <skos:definition xml:lang="en">_</skos:definition>
    <skos:inScheme rdf:resource="http://www.geonames.org/ontology#S"/>
    <skos:prefLabel xml:lang="en">abandoned railroad stop</skos:prefLabel>
  </gn:Code>

  <gn:Code rdf:about="http://www.geonames.org/ontology#S.RUIN">
    <skos:definition xml:lang="en">a destroyed or decayed structure which is no longer functional</skos:definition>
    <skos:inScheme rdf:resource="http://www.geonames.org/ontology#S"/>
    <skos:prefLabel xml:lang="en">ruin(s)</skos:prefLabel>
  </gn:Code>

  <gn:Code rdf:about="http://www.geonames.org/ontology#S.SCH">
    <skos:definition xml:lang="en">building(s) where instruction in one or more branches of knowledge takes place</skos:definition>
    <skos:inScheme rdf:resource="http://www.geonames.org/ontology#S"/>
    <skos:prefLabel xml:lang="en">school</skos:prefLabel>
  </gn:Code>

  <gn:Code rdf:about="http://www.geonames.org/ontology#S.SCHA">
    <skos:definition xml:lang="en">a school with a curriculum focused on agriculture</skos:definition>
    <skos:inScheme rdf:resource="http://www.geonames.org/ontology#S"/>
    <skos:prefLabel xml:lang="en">agricultural school</skos:prefLabel>
  </gn:Code>

  <gn:Code rdf:about="http://www.geonames.org/ontology#S.SCHC">
    <skos:definition xml:lang="en">the grounds and buildings of an institution of higher learning</skos:definition>
    <skos:inScheme rdf:resource="http://www.geonames.org/ontology#S"/>
    <skos:prefLabel xml:lang="en">college</skos:prefLabel>
  </gn:Code>

  <gn:Code rdf:about="http://www.geonames.org/ontology#S.SCHD">
    <skos:definition xml:lang="en">Driving School</skos:definition>
    <skos:inScheme rdf:resource="http://www.geonames.org/ontology#S"/>
    <skos:prefLabel xml:lang="en">Driving School</skos:prefLabel>
  </gn:Code>

  <gn:Code rdf:about="http://www.geonames.org/ontology#S.SCHL">
    <skos:definition xml:lang="en">Language Schools &amp; Institutions</skos:definition>
    <skos:inScheme rdf:resource="http://www.geonames.org/ontology#S"/>
    <skos:prefLabel xml:lang="en">Language School</skos:prefLabel>
  </gn:Code>

  <gn:Code rdf:about="http://www.geonames.org/ontology#S.SCHM">
    <skos:definition xml:lang="en">a school at which military science forms the core of the curriculum</skos:definition>
    <skos:inScheme rdf:resource="http://www.geonames.org/ontology#S"/>
    <skos:prefLabel xml:lang="en">military school</skos:prefLabel>
  </gn:Code>

  <gn:Code rdf:about="http://www.geonames.org/ontology#S.SCHN">
    <skos:definition xml:lang="en">a school at which maritime sciences form the core of the curriculum</skos:definition>
    <skos:inScheme rdf:resource="http://www.geonames.org/ontology#S"/>
    <skos:prefLabel xml:lang="en">maritime school</skos:prefLabel>
  </gn:Code>

  <gn:Code rdf:about="http://www.geonames.org/ontology#S.SCHT">
    <skos:definition xml:lang="en">post-secondary school with a specifically technical or vocational curriculum</skos:definition>
    <skos:inScheme rdf:resource="http://www.geonames.org/ontology#S"/>
    <skos:prefLabel xml:lang="en">technical school</skos:prefLabel>
  </gn:Code>

  <gn:Code rdf:about="http://www.geonames.org/ontology#S.SECP">
    <skos:definition xml:lang="en">State Exam Preparation Centres</skos:definition>
    <skos:inScheme rdf:resource="http://www.geonames.org/ontology#S"/>
    <skos:prefLabel xml:lang="en">State Exam Prep Centre</skos:prefLabel>
  </gn:Code>

  <gn:Code rdf:about="http://www.geonames.org/ontology#S.SHPF">
    <skos:definition xml:lang="en">a fence or wall enclosure for sheep and other small herd animals</skos:definition>
    <skos:inScheme rdf:resource="http://www.geonames.org/ontology#S"/>
    <skos:prefLabel xml:lang="en">sheepfold</skos:prefLabel>
  </gn:Code>

  <gn:Code rdf:about="http://www.geonames.org/ontology#S.SHRN">
    <skos:definition xml:lang="en">a structure or place memorializing a person or religious concept</skos:definition>
    <skos:inScheme rdf:resource="http://www.geonames.org/ontology#S"/>
    <skos:prefLabel xml:lang="en">shrine</skos:prefLabel>
  </gn:Code>

  <gn:Code rdf:about="http://www.geonames.org/ontology#S.SHSE">
    <skos:definition xml:lang="en">a building for storing goods, especially provisions</skos:definition>
    <skos:inScheme rdf:resource="http://www.geonames.org/ontology#S"/>
    <skos:prefLabel xml:lang="en">storehouse</skos:prefLabel>
  </gn:Code>

  <gn:Code rdf:about="http://www.geonames.org/ontology#S.SLCE">
    <skos:definition xml:lang="en">a conduit or passage for carrying off surplus water from a waterbody, usually regulated by means of a sluice gate</skos:definition>
    <skos:inScheme rdf:resource="http://www.geonames.org/ontology#S"/>
    <skos:prefLabel xml:lang="en">sluice</skos:prefLabel>
  </gn:Code>

  <gn:Code rdf:about="http://www.geonames.org/ontology#S.SNTR">
    <skos:definition xml:lang="en">a facility where victims of physical or mental disorders are treated</skos:definition>
    <skos:inScheme rdf:resource="http://www.geonames.org/ontology#S"/>
    <skos:prefLabel xml:lang="en">sanatorium</skos:prefLabel>
  </gn:Code>

  <gn:Code rdf:about="http://www.geonames.org/ontology#S.SPA">
    <skos:definition xml:lang="en">a resort area usually developed around a medicinal spring</skos:definition>
    <skos:inScheme rdf:resource="http://www.geonames.org/ontology#S"/>
    <skos:prefLabel xml:lang="en">spa</skos:prefLabel>
  </gn:Code>

  <gn:Code rdf:about="http://www.geonames.org/ontology#S.SPLY">
    <skos:definition xml:lang="en">a passage or outlet through which surplus water flows over, around or through a dam</skos:definition>
    <skos:inScheme rdf:resource="http://www.geonames.org/ontology#S"/>
    <skos:prefLabel xml:lang="en">spillway</skos:prefLabel>
  </gn:Code>

  <gn:Code rdf:about="http://www.geonames.org/ontology#S.SQR">
    <skos:definition xml:lang="en">a broad, open, public area near the center of a town or city</skos:definition>
    <skos:inScheme rdf:resource="http://www.geonames.org/ontology#S"/>
    <skos:prefLabel xml:lang="en">square</skos:prefLabel>
  </gn:Code>

  <gn:Code rdf:about="http://www.geonames.org/ontology#S.STBL">
    <skos:definition xml:lang="en">a building for the shelter and feeding of farm animals, especially horses</skos:definition>
    <skos:inScheme rdf:resource="http://www.geonames.org/ontology#S"/>
    <skos:prefLabel xml:lang="en">stable</skos:prefLabel>
  </gn:Code>

  <gn:Code rdf:about="http://www.geonames.org/ontology#S.STDM">
    <skos:definition xml:lang="en">a structure with an enclosure for athletic games with tiers of seats for spectators</skos:definition>
    <skos:inScheme rdf:resource="http://www.geonames.org/ontology#S"/>
    <skos:prefLabel xml:lang="en">stadium</skos:prefLabel>
  </gn:Code>

  <gn:Code rdf:about="http://www.geonames.org/ontology#S.STNB">
    <skos:definition xml:lang="en">a scientific facility used as a base from which research is carried out or monitored</skos:definition>
    <skos:inScheme rdf:resource="http://www.geonames.org/ontology#S"/>
    <skos:prefLabel xml:lang="en">scientific research base</skos:prefLabel>
  </gn:Code>

  <gn:Code rdf:about="http://www.geonames.org/ontology#S.STNC">
    <skos:definition xml:lang="en">a facility from which the coast is guarded by armed vessels</skos:definition>
    <skos:inScheme rdf:resource="http://www.geonames.org/ontology#S"/>
    <skos:prefLabel xml:lang="en">coast guard station</skos:prefLabel>
  </gn:Code>

  <gn:Code rdf:about="http://www.geonames.org/ontology#S.STNE">
    <skos:definition xml:lang="en">a facility for carrying out experiments</skos:definition>
    <skos:inScheme rdf:resource="http://www.geonames.org/ontology#S"/>
    <skos:prefLabel xml:lang="en">experiment station</skos:prefLabel>
  </gn:Code>

  <gn:Code rdf:about="http://www.geonames.org/ontology#S.STNF">
    <skos:definition xml:lang="en">a collection of buildings and facilities for carrying out forest management</skos:definition>
    <skos:inScheme rdf:resource="http://www.geonames.org/ontology#S"/>
    <skos:prefLabel xml:lang="en">forest station</skos:prefLabel>
  </gn:Code>

  <gn:Code rdf:about="http://www.geonames.org/ontology#S.STNI">
    <skos:definition xml:lang="en">a station at which vehicles, goods, and people are inspected</skos:definition>
    <skos:inScheme rdf:resource="http://www.geonames.org/ontology#S"/>
    <skos:prefLabel xml:lang="en">inspection station</skos:prefLabel>
  </gn:Code>

  <gn:Code rdf:about="http://www.geonames.org/ontology#S.STNM">
    <skos:definition xml:lang="en">a station at which weather elements are recorded</skos:definition>
    <skos:inScheme rdf:resource="http://www.geonames.org/ontology#S"/>
    <skos:prefLabel xml:lang="en">meteorological station</skos:prefLabel>
  </gn:Code>

  <gn:Code rdf:about="http://www.geonames.org/ontology#S.STNR">
    <skos:definition xml:lang="en">a facility for producing and transmitting information by radio waves</skos:definition>
    <skos:inScheme rdf:resource="http://www.geonames.org/ontology#S"/>
    <skos:prefLabel xml:lang="en">radio station</skos:prefLabel>
  </gn:Code>

  <gn:Code rdf:about="http://www.geonames.org/ontology#S.STNS">
    <skos:definition xml:lang="en">a facility for tracking and communicating with orbiting satellites</skos:definition>
    <skos:inScheme rdf:resource="http://www.geonames.org/ontology#S"/>
    <skos:prefLabel xml:lang="en">satellite station</skos:prefLabel>
  </gn:Code>

  <gn:Code rdf:about="http://www.geonames.org/ontology#S.STNW">
    <skos:definition xml:lang="en">a facility for butchering whales and processing train oil</skos:definition>
    <skos:inScheme rdf:resource="http://www.geonames.org/ontology#S"/>
    <skos:prefLabel xml:lang="en">whaling station</skos:prefLabel>
  </gn:Code>

  <gn:Code rdf:about="http://www.geonames.org/ontology#S.STPS">
    <skos:definition xml:lang="en">stones or slabs placed for ease in ascending or descending a steep slope</skos:definition>
    <skos:inScheme rdf:resource="http://www.geonames.org/ontology#S"/>
    <skos:prefLabel xml:lang="en">steps</skos:prefLabel>
  </gn:Code>

  <gn:Code rdf:about="http://www.geonames.org/ontology#S.SWT">
    <skos:definition xml:lang="en">facility for the processing of sewage and/or wastewater</skos:definition>
    <skos:inScheme rdf:resource="http://www.geonames.org/ontology#S"/>
    <skos:prefLabel xml:lang="en">sewage treatment plant</skos:prefLabel>
  </gn:Code>

  <gn:Code rdf:about="http://www.geonames.org/ontology#S.THTR">
    <skos:definition xml:lang="en">A building, room, or outdoor structure for the presentation of plays, films, or other dramatic performances</skos:definition>
    <skos:inScheme rdf:resource="http://www.geonames.org/ontology#S"/>
    <skos:prefLabel xml:lang="en">theater</skos:prefLabel>
  </gn:Code>

  <gn:Code rdf:about="http://www.geonames.org/ontology#S.TMB">
    <skos:definition xml:lang="en">a structure for interring bodies</skos:definition>
    <skos:inScheme rdf:resource="http://www.geonames.org/ontology#S"/>
    <skos:prefLabel xml:lang="en">tomb(s)</skos:prefLabel>
  </gn:Code>

  <gn:Code rdf:about="http://www.geonames.org/ontology#S.TMPL">
    <skos:definition xml:lang="en">an edifice dedicated to religious worship</skos:definition>
    <skos:inScheme rdf:resource="http://www.geonames.org/ontology#S"/>
    <skos:prefLabel xml:lang="en">temple(s)</skos:prefLabel>
  </gn:Code>

  <gn:Code rdf:about="http://www.geonames.org/ontology#S.TNKD">
    <skos:definition xml:lang="en">a small artificial pond used for immersing cattle in chemically treated water for disease control</skos:definition>
    <skos:inScheme rdf:resource="http://www.geonames.org/ontology#S"/>
    <skos:prefLabel xml:lang="en">cattle dipping tank</skos:prefLabel>
  </gn:Code>

  <gn:Code rdf:about="http://www.geonames.org/ontology#S.TOWR">
    <skos:definition xml:lang="en">a high conspicuous structure, typically much higher than its diameter</skos:definition>
    <skos:inScheme rdf:resource="http://www.geonames.org/ontology#S"/>
    <skos:prefLabel xml:lang="en">tower</skos:prefLabel>
  </gn:Code>

  <gn:Code rdf:about="http://www.geonames.org/ontology#S.TRANT">
    <skos:definition xml:lang="en">facilities for the handling of vehicular freight and passengers</skos:definition>
    <skos:inScheme rdf:resource="http://www.geonames.org/ontology#S"/>
    <skos:prefLabel xml:lang="en">transit terminal</skos:prefLabel>
  </gn:Code>

  <gn:Code rdf:about="http://www.geonames.org/ontology#S.TRIG">
    <skos:definition xml:lang="en">a point on the earth whose position has been determined by triangulation</skos:definition>
    <skos:inScheme rdf:resource="http://www.geonames.org/ontology#S"/>
    <skos:prefLabel xml:lang="en">triangulation station</skos:prefLabel>
  </gn:Code>

  <gn:Code rdf:about="http://www.geonames.org/ontology#S.TRMO">
    <skos:definition xml:lang="en">a tank farm or loading facility at the end of an oil pipeline</skos:definition>
    <skos:inScheme rdf:resource="http://www.geonames.org/ontology#S"/>
    <skos:prefLabel xml:lang="en">oil pipeline terminal</skos:prefLabel>
  </gn:Code>

  <gn:Code rdf:about="http://www.geonames.org/ontology#S.TWO">
    <skos:definition xml:lang="en">Temporary Work Offices</skos:definition>
    <skos:inScheme rdf:resource="http://www.geonames.org/ontology#S"/>
    <skos:prefLabel xml:lang="en">Temp Work Office</skos:prefLabel>
  </gn:Code>

  <gn:Code rdf:about="http://www.geonames.org/ontology#S.UNIO">
    <skos:definition xml:lang="en">Post Universitary Education Institutes (post graduate studies and highly specialised master programs) &amp; MBA</skos:definition>
    <skos:inScheme rdf:resource="http://www.geonames.org/ontology#S"/>
    <skos:prefLabel xml:lang="en">postgrad &amp; MBA</skos:prefLabel>
  </gn:Code>

  <gn:Code rdf:about="http://www.geonames.org/ontology#S.UNIP">
    <skos:definition xml:lang="en">University Preparation Schools &amp; Institutions</skos:definition>
    <skos:inScheme rdf:resource="http://www.geonames.org/ontology#S"/>
    <skos:prefLabel xml:lang="en">University Prep School</skos:prefLabel>
  </gn:Code>

  <gn:Code rdf:about="http://www.geonames.org/ontology#S.UNIV">
    <skos:definition xml:lang="en">An institution for higher learning with teaching and research facilities constituting a graduate school and professional schools that award master's degrees and doctorates and an undergraduate division that awards bachelor's degrees.</skos:definition>
    <skos:inScheme rdf:resource="http://www.geonames.org/ontology#S"/>
    <skos:prefLabel xml:lang="en">university</skos:prefLabel>
  </gn:Code>

  <gn:Code rdf:about="http://www.geonames.org/ontology#S.USGE">
    <skos:definition xml:lang="en">a facility operated by the United States Government in Panama</skos:definition>
    <skos:inScheme rdf:resource="http://www.geonames.org/ontology#S"/>
    <skos:prefLabel xml:lang="en">united states government establishment</skos:prefLabel>
  </gn:Code>

  <gn:Code rdf:about="http://www.geonames.org/ontology#S.VETF">
    <skos:definition xml:lang="en">a building or camp at which veterinary services are available</skos:definition>
    <skos:inScheme rdf:resource="http://www.geonames.org/ontology#S"/>
    <skos:prefLabel xml:lang="en">veterinary facility</skos:prefLabel>
  </gn:Code>

  <gn:Code rdf:about="http://www.geonames.org/ontology#S.WALL">
    <skos:definition xml:lang="en">a thick masonry structure, usually enclosing a field or building, or forming the side of a structure</skos:definition>
    <skos:inScheme rdf:resource="http://www.geonames.org/ontology#S"/>
    <skos:prefLabel xml:lang="en">wall</skos:prefLabel>
  </gn:Code>

  <gn:Code rdf:about="http://www.geonames.org/ontology#S.WALLA">
    <skos:definition xml:lang="en">the remains of a linear defensive stone structure</skos:definition>
    <skos:inScheme rdf:resource="http://www.geonames.org/ontology#S"/>
    <skos:prefLabel xml:lang="en">ancient wall</skos:prefLabel>
  </gn:Code>

  <gn:Code rdf:about="http://www.geonames.org/ontology#S.WEIR">
    <skos:definition xml:lang="en">a small dam in a stream, designed to raise the water level or to divert stream flow through a desired channel</skos:definition>
    <skos:inScheme rdf:resource="http://www.geonames.org/ontology#S"/>
    <skos:prefLabel xml:lang="en">weir(s)</skos:prefLabel>
  </gn:Code>

  <gn:Code rdf:about="http://www.geonames.org/ontology#S.WHRF">
    <skos:definition xml:lang="en">a structure of open rather than solid construction along a shore or a bank which provides berthing for ships and cargo-handling facilities</skos:definition>
    <skos:inScheme rdf:resource="http://www.geonames.org/ontology#S"/>
    <skos:prefLabel xml:lang="en">wharf(-ves)</skos:prefLabel>
  </gn:Code>

  <gn:Code rdf:about="http://www.geonames.org/ontology#S.WRCK">
    <skos:definition xml:lang="en">the site of the remains of a wrecked vessel</skos:definition>
    <skos:inScheme rdf:resource="http://www.geonames.org/ontology#S"/>
    <skos:prefLabel xml:lang="en">wreck</skos:prefLabel>
  </gn:Code>

  <gn:Code rdf:about="http://www.geonames.org/ontology#S.WTRW">
    <skos:definition xml:lang="en">a facility for supplying potable water through a water source and a system of pumps and filtration beds</skos:definition>
    <skos:inScheme rdf:resource="http://www.geonames.org/ontology#S"/>
    <skos:prefLabel xml:lang="en">waterworks</skos:prefLabel>
  </gn:Code>

  <gn:Code rdf:about="http://www.geonames.org/ontology#S.ZNF">
    <skos:definition xml:lang="en">an area, usually a section of a port, where goods may be received and shipped free of customs duty and of most customs regulations</skos:definition>
    <skos:inScheme rdf:resource="http://www.geonames.org/ontology#S"/>
    <skos:prefLabel xml:lang="en">free trade zone</skos:prefLabel>
  </gn:Code>

  <gn:Code rdf:about="http://www.geonames.org/ontology#S.ZOO">
    <skos:definition xml:lang="en">a zoological garden or park where wild animals are kept for exhibition</skos:definition>
    <skos:inScheme rdf:resource="http://www.geonames.org/ontology#S"/>
    <skos:prefLabel xml:lang="en">zoo</skos:prefLabel>
  </gn:Code>

  <gn:Class rdf:about="http://www.geonames.org/ontology#T">
    <rdfs:comment xml:lang="en">mountain, hill, rock, ...</rdfs:comment>
  </gn:Class>

  <gn:Code rdf:about="http://www.geonames.org/ontology#T.ASPH">
    <skos:definition xml:lang="en">a small basin containing naturally occurring asphalt</skos:definition>
    <skos:inScheme rdf:resource="http://www.geonames.org/ontology#T"/>
    <skos:prefLabel xml:lang="en">asphalt lake</skos:prefLabel>
  </gn:Code>

  <gn:Code rdf:about="http://www.geonames.org/ontology#T.ATOL">
    <skos:definition xml:lang="en">a ring-shaped coral reef which has closely spaced islands on it encircling a lagoon</skos:definition>
    <skos:inScheme rdf:resource="http://www.geonames.org/ontology#T"/>
    <skos:prefLabel xml:lang="en">atoll(s)</skos:prefLabel>
  </gn:Code>

  <gn:Code rdf:about="http://www.geonames.org/ontology#T.BAR">
    <skos:definition xml:lang="en">a shallow ridge or mound of coarse unconsolidated material in a stream channel, at the mouth of a stream, estuary, or lagoon and in the wave-break zone along coasts</skos:definition>
    <skos:inScheme rdf:resource="http://www.geonames.org/ontology#T"/>
    <skos:prefLabel xml:lang="en">bar</skos:prefLabel>
  </gn:Code>

  <gn:Code rdf:about="http://www.geonames.org/ontology#T.BCH">
    <skos:definition xml:lang="en">a shore zone of coarse unconsolidated sediment that extends from the low-water line to the highest reach of storm waves</skos:definition>
    <skos:inScheme rdf:resource="http://www.geonames.org/ontology#T"/>
    <skos:prefLabel xml:lang="en">beach</skos:prefLabel>
  </gn:Code>

  <gn:Code rdf:about="http://www.geonames.org/ontology#T.BCHS">
    <skos:definition xml:lang="en">a shore zone of coarse unconsolidated sediment that extends from the low-water line to the highest reach of storm waves</skos:definition>
    <skos:inScheme rdf:resource="http://www.geonames.org/ontology#T"/>
    <skos:prefLabel xml:lang="en">beaches</skos:prefLabel>
  </gn:Code>

  <gn:Code rdf:about="http://www.geonames.org/ontology#T.BDLD">
    <skos:definition xml:lang="en">an area characterized by a maze of very closely spaced, deep, narrow, steep-sided ravines, and sharp crests and pinnacles</skos:definition>
    <skos:inScheme rdf:resource="http://www.geonames.org/ontology#T"/>
    <skos:prefLabel xml:lang="en">badlands</skos:prefLabel>
  </gn:Code>

  <gn:Code rdf:about="http://www.geonames.org/ontology#T.BLDR">
    <skos:definition xml:lang="en">a high altitude or high latitude bare, flat area covered with large angular rocks</skos:definition>
    <skos:inScheme rdf:resource="http://www.geonames.org/ontology#T"/>
    <skos:prefLabel xml:lang="en">boulder field</skos:prefLabel>
  </gn:Code>

  <gn:Code rdf:about="http://www.geonames.org/ontology#T.BLHL">
    <skos:definition xml:lang="en">a hole in coastal rock through which sea water is forced by a rising tide or waves and spurted through an outlet into the air</skos:definition>
    <skos:inScheme rdf:resource="http://www.geonames.org/ontology#T"/>
    <skos:prefLabel xml:lang="en">blowhole(s)</skos:prefLabel>
  </gn:Code>

  <gn:Code rdf:about="http://www.geonames.org/ontology#T.BLOW">
    <skos:definition xml:lang="en">a small depression in sandy terrain, caused by wind erosion</skos:definition>
    <skos:inScheme rdf:resource="http://www.geonames.org/ontology#T"/>
    <skos:prefLabel xml:lang="en">blowout(s)</skos:prefLabel>
  </gn:Code>

  <gn:Code rdf:about="http://www.geonames.org/ontology#T.BNCH">
    <skos:definition xml:lang="en">a long, narrow bedrock platform bounded by steeper slopes above and below, usually overlooking a waterbody</skos:definition>
    <skos:inScheme rdf:resource="http://www.geonames.org/ontology#T"/>
    <skos:prefLabel xml:lang="en">bench</skos:prefLabel>
  </gn:Code>

  <gn:Code rdf:about="http://www.geonames.org/ontology#T.BUTE">
    <skos:definition xml:lang="en">a small, isolated, usually flat-topped hill with steep sides</skos:definition>
    <skos:inScheme rdf:resource="http://www.geonames.org/ontology#T"/>
    <skos:prefLabel xml:lang="en">butte(s)</skos:prefLabel>
  </gn:Code>

  <gn:Code rdf:about="http://www.geonames.org/ontology#T.CAPE">
    <skos:definition xml:lang="en">a land area, more prominent than a point, projecting into the sea and marking a notable change in coastal direction</skos:definition>
    <skos:inScheme rdf:resource="http://www.geonames.org/ontology#T"/>
    <skos:prefLabel xml:lang="en">cape</skos:prefLabel>
  </gn:Code>

  <gn:Code rdf:about="http://www.geonames.org/ontology#T.CFT">
    <skos:definition xml:lang="en">a deep narrow slot, notch, or groove in a coastal cliff</skos:definition>
    <skos:inScheme rdf:resource="http://www.geonames.org/ontology#T"/>
    <skos:prefLabel xml:lang="en">cleft(s)</skos:prefLabel>
  </gn:Code>

  <gn:Code rdf:about="http://www.geonames.org/ontology#T.CLDA">
    <skos:definition xml:lang="en">a depression measuring kilometers across formed by the collapse of a volcanic mountain</skos:definition>
    <skos:inScheme rdf:resource="http://www.geonames.org/ontology#T"/>
    <skos:prefLabel xml:lang="en">caldera</skos:prefLabel>
  </gn:Code>

  <gn:Code rdf:about="http://www.geonames.org/ontology#T.CLF">
    <skos:definition xml:lang="en">a high, steep to perpendicular slope overlooking a waterbody or lower area</skos:definition>
    <skos:inScheme rdf:resource="http://www.geonames.org/ontology#T"/>
    <skos:prefLabel xml:lang="en">cliff(s)</skos:prefLabel>
  </gn:Code>

  <gn:Code rdf:about="http://www.geonames.org/ontology#T.CNYN">
    <skos:definition xml:lang="en">a deep, narrow valley with steep sides cutting into a plateau or mountainous area</skos:definition>
    <skos:inScheme rdf:resource="http://www.geonames.org/ontology#T"/>
    <skos:prefLabel xml:lang="en">canyon</skos:prefLabel>
  </gn:Code>

  <gn:Code rdf:about="http://www.geonames.org/ontology#T.CONE">
    <skos:definition xml:lang="en">a conical landform composed of mud or volcanic material</skos:definition>
    <skos:inScheme rdf:resource="http://www.geonames.org/ontology#T"/>
    <skos:prefLabel xml:lang="en">cone(s)</skos:prefLabel>
  </gn:Code>

  <gn:Code rdf:about="http://www.geonames.org/ontology#T.CRDR">
    <skos:definition xml:lang="en">a strip or area of land having significance as an access way</skos:definition>
    <skos:inScheme rdf:resource="http://www.geonames.org/ontology#T"/>
    <skos:prefLabel xml:lang="en">corridor</skos:prefLabel>
  </gn:Code>

  <gn:Code rdf:about="http://www.geonames.org/ontology#T.CRQ">
    <skos:definition xml:lang="en">a bowl-like hollow partially surrounded by cliffs or steep slopes at the head of a glaciated valley</skos:definition>
    <skos:inScheme rdf:resource="http://www.geonames.org/ontology#T"/>
    <skos:prefLabel xml:lang="en">cirque</skos:prefLabel>
  </gn:Code>

  <gn:Code rdf:about="http://www.geonames.org/ontology#T.CRQS">
    <skos:definition xml:lang="en">bowl-like hollows partially surrounded by cliffs or steep slopes at the head of a glaciated valley</skos:definition>
    <skos:inScheme rdf:resource="http://www.geonames.org/ontology#T"/>
    <skos:prefLabel xml:lang="en">cirques</skos:prefLabel>
  </gn:Code>

  <gn:Code rdf:about="http://www.geonames.org/ontology#T.CRTR">
    <skos:definition xml:lang="en">a generally circular saucer or bowl-shaped depression caused by volcanic or meteorite explosive action</skos:definition>
    <skos:inScheme rdf:resource="http://www.geonames.org/ontology#T"/>
    <skos:prefLabel xml:lang="en">crater(s)</skos:prefLabel>
  </gn:Code>

  <gn:Code rdf:about="http://www.geonames.org/ontology#T.CUET">
    <skos:definition xml:lang="en">an asymmetric ridge formed on tilted strata</skos:definition>
    <skos:inScheme rdf:resource="http://www.geonames.org/ontology#T"/>
    <skos:prefLabel xml:lang="en">cuesta(s)</skos:prefLabel>
  </gn:Code>

  <gn:Code rdf:about="http://www.geonames.org/ontology#T.DLTA">
    <skos:definition xml:lang="en">a flat plain formed by alluvial deposits at the mouth of a stream</skos:definition>
    <skos:inScheme rdf:resource="http://www.geonames.org/ontology#T"/>
    <skos:prefLabel xml:lang="en">delta</skos:prefLabel>
  </gn:Code>

  <gn:Code rdf:about="http://www.geonames.org/ontology#T.DPR">
    <skos:definition xml:lang="en">a low area surrounded by higher land and usually characterized by interior drainage</skos:definition>
    <skos:inScheme rdf:resource="http://www.geonames.org/ontology#T"/>
    <skos:prefLabel xml:lang="en">depression(s)</skos:prefLabel>
  </gn:Code>

  <gn:Code rdf:about="http://www.geonames.org/ontology#T.DSRT">
    <skos:definition xml:lang="en">a large area with little or no vegetation due to extreme environmental conditions</skos:definition>
    <skos:inScheme rdf:resource="http://www.geonames.org/ontology#T"/>
    <skos:prefLabel xml:lang="en">desert</skos:prefLabel>
  </gn:Code>

  <gn:Code rdf:about="http://www.geonames.org/ontology#T.DUNE">
    <skos:definition xml:lang="en">a wave form, ridge or star shape feature composed of sand</skos:definition>
    <skos:inScheme rdf:resource="http://www.geonames.org/ontology#T"/>
    <skos:prefLabel xml:lang="en">dune(s)</skos:prefLabel>
  </gn:Code>

  <gn:Code rdf:about="http://www.geonames.org/ontology#T.DVD">
    <skos:definition xml:lang="en">a line separating adjacent drainage basins</skos:definition>
    <skos:inScheme rdf:resource="http://www.geonames.org/ontology#T"/>
    <skos:prefLabel xml:lang="en">divide</skos:prefLabel>
  </gn:Code>

  <gn:Code rdf:about="http://www.geonames.org/ontology#T.ERG">
    <skos:definition xml:lang="en">an extensive tract of shifting sand and sand dunes</skos:definition>
    <skos:inScheme rdf:resource="http://www.geonames.org/ontology#T"/>
    <skos:prefLabel xml:lang="en">sandy desert</skos:prefLabel>
  </gn:Code>

  <gn:Code rdf:about="http://www.geonames.org/ontology#T.FAN">
    <skos:definition xml:lang="en">a fan-shaped wedge of coarse alluvium with apex merging with a mountain stream bed and the fan spreading out at a low angle slope onto an adjacent plain</skos:definition>
    <skos:inScheme rdf:resource="http://www.geonames.org/ontology#T"/>
    <skos:prefLabel xml:lang="en">fan(s)</skos:prefLabel>
  </gn:Code>

  <gn:Code rdf:about="http://www.geonames.org/ontology#T.FORD">
    <skos:definition xml:lang="en">a shallow part of a stream which can be crossed on foot or by land vehicle</skos:definition>
    <skos:inScheme rdf:resource="http://www.geonames.org/ontology#T"/>
    <skos:prefLabel xml:lang="en">ford</skos:prefLabel>
  </gn:Code>

  <gn:Code rdf:about="http://www.geonames.org/ontology#T.FSR">
    <skos:definition xml:lang="en">a crack associated with volcanism</skos:definition>
    <skos:inScheme rdf:resource="http://www.geonames.org/ontology#T"/>
    <skos:prefLabel xml:lang="en">fissure</skos:prefLabel>
  </gn:Code>

  <gn:Code rdf:about="http://www.geonames.org/ontology#T.GAP">
    <skos:definition xml:lang="en">a low place in a ridge, not used for transportation</skos:definition>
    <skos:inScheme rdf:resource="http://www.geonames.org/ontology#T"/>
    <skos:prefLabel xml:lang="en">gap</skos:prefLabel>
  </gn:Code>

  <gn:Code rdf:about="http://www.geonames.org/ontology#T.GRGE">
    <skos:definition xml:lang="en">a short, narrow, steep-sided section of a stream valley</skos:definition>
    <skos:inScheme rdf:resource="http://www.geonames.org/ontology#T"/>
    <skos:prefLabel xml:lang="en">gorge(s)</skos:prefLabel>
  </gn:Code>

  <gn:Code rdf:about="http://www.geonames.org/ontology#T.HDLD">
    <skos:definition xml:lang="en">a high projection of land extending into a large body of water beyond the line of the coast</skos:definition>
    <skos:inScheme rdf:resource="http://www.geonames.org/ontology#T"/>
    <skos:prefLabel xml:lang="en">headland</skos:prefLabel>
  </gn:Code>

  <gn:Code rdf:about="http://www.geonames.org/ontology#T.HLL">
    <skos:definition xml:lang="en">a rounded elevation of limited extent rising above the surrounding land with local relief of less than 300m</skos:definition>
    <skos:inScheme rdf:resource="http://www.geonames.org/ontology#T"/>
    <skos:prefLabel xml:lang="en">hill</skos:prefLabel>
  </gn:Code>

  <gn:Code rdf:about="http://www.geonames.org/ontology#T.HLLS">
    <skos:definition xml:lang="en">rounded elevations of limited extent rising above the surrounding land with local relief of less than 300m</skos:definition>
    <skos:inScheme rdf:resource="http://www.geonames.org/ontology#T"/>
    <skos:prefLabel xml:lang="en">hills</skos:prefLabel>
  </gn:Code>

  <gn:Code rdf:about="http://www.geonames.org/ontology#T.HMCK">
    <skos:definition xml:lang="en">a patch of ground, distinct from and slightly above the surrounding plain or wetland. Often occurs in groups</skos:definition>
    <skos:inScheme rdf:resource="http://www.geonames.org/ontology#T"/>
    <skos:prefLabel xml:lang="en">hammock(s)</skos:prefLabel>
  </gn:Code>

  <gn:Code rdf:about="http://www.geonames.org/ontology#T.HMDA">
    <skos:definition xml:lang="en">a relatively sand-free, high bedrock plateau in a hot desert, with or without a gravel veneer</skos:definition>
    <skos:inScheme rdf:resource="http://www.geonames.org/ontology#T"/>
    <skos:prefLabel xml:lang="en">rock desert</skos:prefLabel>
  </gn:Code>

  <gn:Code rdf:about="http://www.geonames.org/ontology#T.INTF">
    <skos:definition xml:lang="en">a relatively undissected upland between adjacent stream valleys</skos:definition>
    <skos:inScheme rdf:resource="http://www.geonames.org/ontology#T"/>
    <skos:prefLabel xml:lang="en">interfluve</skos:prefLabel>
  </gn:Code>

  <gn:Code rdf:about="http://www.geonames.org/ontology#T.ISL">
    <skos:definition xml:lang="en">a tract of land, smaller than a continent, surrounded by water at high water</skos:definition>
    <skos:inScheme rdf:resource="http://www.geonames.org/ontology#T"/>
    <skos:prefLabel xml:lang="en">island</skos:prefLabel>
  </gn:Code>

  <gn:Code rdf:about="http://www.geonames.org/ontology#T.ISLF">
    <skos:definition xml:lang="en">an island created by landfill or diking and filling in a wetland, bay, or lagoon</skos:definition>
    <skos:inScheme rdf:resource="http://www.geonames.org/ontology#T"/>
    <skos:prefLabel xml:lang="en">artificial island</skos:prefLabel>
  </gn:Code>

  <gn:Code rdf:about="http://www.geonames.org/ontology#T.ISLM">
    <skos:definition xml:lang="en">a mangrove swamp surrounded by a waterbody</skos:definition>
    <skos:inScheme rdf:resource="http://www.geonames.org/ontology#T"/>
    <skos:prefLabel xml:lang="en">mangrove island</skos:prefLabel>
  </gn:Code>

  <gn:Code rdf:about="http://www.geonames.org/ontology#T.ISLS">
    <skos:definition xml:lang="en">tracts of land, smaller than a continent, surrounded by water at high water</skos:definition>
    <skos:inScheme rdf:resource="http://www.geonames.org/ontology#T"/>
    <skos:prefLabel xml:lang="en">islands</skos:prefLabel>
  </gn:Code>

  <gn:Code rdf:about="http://www.geonames.org/ontology#T.ISLT">
    <skos:definition xml:lang="en">a coastal island connected to the mainland by barrier beaches, levees or dikes</skos:definition>
    <skos:inScheme rdf:resource="http://www.geonames.org/ontology#T"/>
    <skos:prefLabel xml:lang="en">land-tied island</skos:prefLabel>
  </gn:Code>

  <gn:Code rdf:about="http://www.geonames.org/ontology#T.ISLX">
    <skos:definition xml:lang="en">_</skos:definition>
    <skos:inScheme rdf:resource="http://www.geonames.org/ontology#T"/>
    <skos:prefLabel xml:lang="en">section of island</skos:prefLabel>
  </gn:Code>

  <gn:Code rdf:about="http://www.geonames.org/ontology#T.ISTH">
    <skos:definition xml:lang="en">a narrow strip of land connecting two larger land masses and bordered by water</skos:definition>
    <skos:inScheme rdf:resource="http://www.geonames.org/ontology#T"/>
    <skos:prefLabel xml:lang="en">isthmus</skos:prefLabel>
  </gn:Code>

  <gn:Code rdf:about="http://www.geonames.org/ontology#T.KRST">
    <skos:definition xml:lang="en">a distinctive landscape developed on soluble rock such as limestone characterized by sinkholes, caves, disappearing streams, and underground drainage</skos:definition>
    <skos:inScheme rdf:resource="http://www.geonames.org/ontology#T"/>
    <skos:prefLabel xml:lang="en">karst area</skos:prefLabel>
  </gn:Code>

  <gn:Code rdf:about="http://www.geonames.org/ontology#T.LAVA">
    <skos:definition xml:lang="en">an area of solidified lava</skos:definition>
    <skos:inScheme rdf:resource="http://www.geonames.org/ontology#T"/>
    <skos:prefLabel xml:lang="en">lava area</skos:prefLabel>
  </gn:Code>

  <gn:Code rdf:about="http://www.geonames.org/ontology#T.LEV">
    <skos:definition xml:lang="en">a natural low embankment bordering a distributary or meandering stream; often built up artificially to control floods</skos:definition>
    <skos:inScheme rdf:resource="http://www.geonames.org/ontology#T"/>
    <skos:prefLabel xml:lang="en">levee</skos:prefLabel>
  </gn:Code>

  <gn:Code rdf:about="http://www.geonames.org/ontology#T.MESA">
    <skos:definition xml:lang="en">a flat-topped, isolated elevation with steep slopes on all sides, less extensive than a plateau</skos:definition>
    <skos:inScheme rdf:resource="http://www.geonames.org/ontology#T"/>
    <skos:prefLabel xml:lang="en">mesa(s)</skos:prefLabel>
  </gn:Code>

  <gn:Code rdf:about="http://www.geonames.org/ontology#T.MND">
    <skos:definition xml:lang="en">a low, isolated, rounded hill</skos:definition>
    <skos:inScheme rdf:resource="http://www.geonames.org/ontology#T"/>
    <skos:prefLabel xml:lang="en">mound(s)</skos:prefLabel>
  </gn:Code>

  <gn:Code rdf:about="http://www.geonames.org/ontology#T.MRN">
    <skos:definition xml:lang="en">a mound, ridge, or other accumulation of glacial till</skos:definition>
    <skos:inScheme rdf:resource="http://www.geonames.org/ontology#T"/>
    <skos:prefLabel xml:lang="en">moraine</skos:prefLabel>
  </gn:Code>

  <gn:Code rdf:about="http://www.geonames.org/ontology#T.MT">
    <skos:definition xml:lang="en">an elevation standing high above the surrounding area with small summit area, steep slopes and local relief of 300m or more</skos:definition>
    <skos:inScheme rdf:resource="http://www.geonames.org/ontology#T"/>
    <skos:prefLabel xml:lang="en">mountain</skos:prefLabel>
  </gn:Code>

  <gn:Code rdf:about="http://www.geonames.org/ontology#T.MTS">
    <skos:definition xml:lang="en">a mountain range or a group of mountains or high ridges</skos:definition>
    <skos:inScheme rdf:resource="http://www.geonames.org/ontology#T"/>
    <skos:prefLabel xml:lang="en">mountains</skos:prefLabel>
  </gn:Code>

  <gn:Code rdf:about="http://www.geonames.org/ontology#T.NKM">
    <skos:definition xml:lang="en">a narrow strip of land between the two limbs of a meander loop at its narrowest point</skos:definition>
    <skos:inScheme rdf:resource="http://www.geonames.org/ontology#T"/>
    <skos:prefLabel xml:lang="en">meander neck</skos:prefLabel>
  </gn:Code>

  <gn:Code rdf:about="http://www.geonames.org/ontology#T.NTK">
    <skos:definition xml:lang="en">a rock or mountain peak protruding through glacial ice</skos:definition>
    <skos:inScheme rdf:resource="http://www.geonames.org/ontology#T"/>
    <skos:prefLabel xml:lang="en">nunatak</skos:prefLabel>
  </gn:Code>

  <gn:Code rdf:about="http://www.geonames.org/ontology#T.NTKS">
    <skos:definition xml:lang="en">rocks or mountain peaks protruding through glacial ice</skos:definition>
    <skos:inScheme rdf:resource="http://www.geonames.org/ontology#T"/>
    <skos:prefLabel xml:lang="en">nunataks</skos:prefLabel>
  </gn:Code>

  <gn:Code rdf:about="http://www.geonames.org/ontology#T.PAN">
    <skos:definition xml:lang="en">a near-level shallow, natural depression or basin, usually containing an intermittent lake, pond, or pool</skos:definition>
    <skos:inScheme rdf:resource="http://www.geonames.org/ontology#T"/>
    <skos:prefLabel xml:lang="en">pan</skos:prefLabel>
  </gn:Code>

  <gn:Code rdf:about="http://www.geonames.org/ontology#T.PANS">
    <skos:definition xml:lang="en">a near-level shallow, natural depression or basin, usually containing an intermittent lake, pond, or pool</skos:definition>
    <skos:inScheme rdf:resource="http://www.geonames.org/ontology#T"/>
    <skos:prefLabel xml:lang="en">pans</skos:prefLabel>
  </gn:Code>

  <gn:Code rdf:about="http://www.geonames.org/ontology#T.PASS">
    <skos:definition xml:lang="en">a break in a mountain range or other high obstruction, used for transportation from one side to the other [See also gap]</skos:definition>
    <skos:inScheme rdf:resource="http://www.geonames.org/ontology#T"/>
    <skos:prefLabel xml:lang="en">pass</skos:prefLabel>
  </gn:Code>

  <gn:Code rdf:about="http://www.geonames.org/ontology#T.PEN">
    <skos:definition xml:lang="en">an elongate area of land projecting into a body of water and nearly surrounded by water</skos:definition>
    <skos:inScheme rdf:resource="http://www.geonames.org/ontology#T"/>
    <skos:prefLabel xml:lang="en">peninsula</skos:prefLabel>
  </gn:Code>

  <gn:Code rdf:about="http://www.geonames.org/ontology#T.PENX">
    <skos:definition xml:lang="en">_</skos:definition>
    <skos:inScheme rdf:resource="http://www.geonames.org/ontology#T"/>
    <skos:prefLabel xml:lang="en">section of peninsula</skos:prefLabel>
  </gn:Code>

  <gn:Code rdf:about="http://www.geonames.org/ontology#T.PK">
    <skos:definition xml:lang="en">a pointed elevation atop a mountain, ridge, or other hypsographic feature</skos:definition>
    <skos:inScheme rdf:resource="http://www.geonames.org/ontology#T"/>
    <skos:prefLabel xml:lang="en">peak</skos:prefLabel>
  </gn:Code>

  <gn:Code rdf:about="http://www.geonames.org/ontology#T.PKS">
    <skos:definition xml:lang="en">pointed elevations atop a mountain, ridge, or other hypsographic features</skos:definition>
    <skos:inScheme rdf:resource="http://www.geonames.org/ontology#T"/>
    <skos:prefLabel xml:lang="en">peaks</skos:prefLabel>
  </gn:Code>

  <gn:Code rdf:about="http://www.geonames.org/ontology#T.PLAT">
    <skos:definition xml:lang="en">an elevated plain with steep slopes on one or more sides, and often with incised streams</skos:definition>
    <skos:inScheme rdf:resource="http://www.geonames.org/ontology#T"/>
    <skos:prefLabel xml:lang="en">plateau</skos:prefLabel>
  </gn:Code>

  <gn:Code rdf:about="http://www.geonames.org/ontology#T.PLATX">
    <skos:definition xml:lang="en">_</skos:definition>
    <skos:inScheme rdf:resource="http://www.geonames.org/ontology#T"/>
    <skos:prefLabel xml:lang="en">section of plateau</skos:prefLabel>
  </gn:Code>

  <gn:Code rdf:about="http://www.geonames.org/ontology#T.PLDR">
    <skos:definition xml:lang="en">an area reclaimed from the sea by diking and draining</skos:definition>
    <skos:inScheme rdf:resource="http://www.geonames.org/ontology#T"/>
    <skos:prefLabel xml:lang="en">polder</skos:prefLabel>
  </gn:Code>

  <gn:Code rdf:about="http://www.geonames.org/ontology#T.PLN">
    <skos:definition xml:lang="en">an extensive area of comparatively level to gently undulating land, lacking surface irregularities, and usually adjacent to a higher area</skos:definition>
    <skos:inScheme rdf:resource="http://www.geonames.org/ontology#T"/>
    <skos:prefLabel xml:lang="en">plain(s)</skos:prefLabel>
  </gn:Code>

  <gn:Code rdf:about="http://www.geonames.org/ontology#T.PLNX">
    <skos:definition xml:lang="en">_</skos:definition>
    <skos:inScheme rdf:resource="http://www.geonames.org/ontology#T"/>
    <skos:prefLabel xml:lang="en">section of plain</skos:prefLabel>
  </gn:Code>

  <gn:Code rdf:about="http://www.geonames.org/ontology#T.PROM">
    <skos:definition xml:lang="en">a bluff or prominent hill overlooking or projecting into a lowland</skos:definition>
    <skos:inScheme rdf:resource="http://www.geonames.org/ontology#T"/>
    <skos:prefLabel xml:lang="en">promontory(-ies)</skos:prefLabel>
  </gn:Code>

  <gn:Code rdf:about="http://www.geonames.org/ontology#T.PT">
    <skos:definition xml:lang="en">a tapering piece of land projecting into a body of water, less prominent than a cape</skos:definition>
    <skos:inScheme rdf:resource="http://www.geonames.org/ontology#T"/>
    <skos:prefLabel xml:lang="en">point</skos:prefLabel>
  </gn:Code>

  <gn:Code rdf:about="http://www.geonames.org/ontology#T.PTS">
    <skos:definition xml:lang="en">tapering pieces of land projecting into a body of water, less prominent than a cape</skos:definition>
    <skos:inScheme rdf:resource="http://www.geonames.org/ontology#T"/>
    <skos:prefLabel xml:lang="en">points</skos:prefLabel>
  </gn:Code>

  <gn:Code rdf:about="http://www.geonames.org/ontology#T.RDGB">
    <skos:definition xml:lang="en">a ridge of sand just inland and parallel to the beach, usually in series</skos:definition>
    <skos:inScheme rdf:resource="http://www.geonames.org/ontology#T"/>
    <skos:prefLabel xml:lang="en">beach ridge</skos:prefLabel>
  </gn:Code>

  <gn:Code rdf:about="http://www.geonames.org/ontology#T.RDGE">
    <skos:definition xml:lang="en">a long narrow elevation with steep sides, and a more or less continuous crest</skos:definition>
    <skos:inScheme rdf:resource="http://www.geonames.org/ontology#T"/>
    <skos:prefLabel xml:lang="en">ridge(s)</skos:prefLabel>
  </gn:Code>

  <gn:Code rdf:about="http://www.geonames.org/ontology#T.REG">
    <skos:definition xml:lang="en">a desert plain characterized by a surface veneer of gravel and stones</skos:definition>
    <skos:inScheme rdf:resource="http://www.geonames.org/ontology#T"/>
    <skos:prefLabel xml:lang="en">stony desert</skos:prefLabel>
  </gn:Code>

  <gn:Code rdf:about="http://www.geonames.org/ontology#T.RK">
    <skos:definition xml:lang="en">a conspicuous, isolated rocky mass</skos:definition>
    <skos:inScheme rdf:resource="http://www.geonames.org/ontology#T"/>
    <skos:prefLabel xml:lang="en">rock</skos:prefLabel>
  </gn:Code>

  <gn:Code rdf:about="http://www.geonames.org/ontology#T.RKFL">
    <skos:definition xml:lang="en">an irregular mass of fallen rock at the base of a cliff or steep slope</skos:definition>
    <skos:inScheme rdf:resource="http://www.geonames.org/ontology#T"/>
    <skos:prefLabel xml:lang="en">rockfall</skos:prefLabel>
  </gn:Code>

  <gn:Code rdf:about="http://www.geonames.org/ontology#T.RKS">
    <skos:definition xml:lang="en">conspicuous, isolated rocky masses</skos:definition>
    <skos:inScheme rdf:resource="http://www.geonames.org/ontology#T"/>
    <skos:prefLabel xml:lang="en">rocks</skos:prefLabel>
  </gn:Code>

  <gn:Code rdf:about="http://www.geonames.org/ontology#T.SAND">
    <skos:definition xml:lang="en">a tract of land covered with sand</skos:definition>
    <skos:inScheme rdf:resource="http://www.geonames.org/ontology#T"/>
    <skos:prefLabel xml:lang="en">sand area</skos:prefLabel>
  </gn:Code>

  <gn:Code rdf:about="http://www.geonames.org/ontology#T.SBED">
    <skos:definition xml:lang="en">a channel formerly containing the water of a stream</skos:definition>
    <skos:inScheme rdf:resource="http://www.geonames.org/ontology#T"/>
    <skos:prefLabel xml:lang="en">dry stream bed</skos:prefLabel>
  </gn:Code>

  <gn:Code rdf:about="http://www.geonames.org/ontology#T.SCRP">
    <skos:definition xml:lang="en">a long line of cliffs or steep slopes separating level surfaces above and below</skos:definition>
    <skos:inScheme rdf:resource="http://www.geonames.org/ontology#T"/>
    <skos:prefLabel xml:lang="en">escarpment</skos:prefLabel>
  </gn:Code>

  <gn:Code rdf:about="http://www.geonames.org/ontology#T.SDL">
    <skos:definition xml:lang="en">a broad, open pass crossing a ridge or between hills or mountains</skos:definition>
    <skos:inScheme rdf:resource="http://www.geonames.org/ontology#T"/>
    <skos:prefLabel xml:lang="en">saddle</skos:prefLabel>
  </gn:Code>

  <gn:Code rdf:about="http://www.geonames.org/ontology#T.SHOR">
    <skos:definition xml:lang="en">a narrow zone bordering a waterbody which covers and uncovers at high and low water, respectively</skos:definition>
    <skos:inScheme rdf:resource="http://www.geonames.org/ontology#T"/>
    <skos:prefLabel xml:lang="en">shore</skos:prefLabel>
  </gn:Code>

  <gn:Code rdf:about="http://www.geonames.org/ontology#T.SINK">
    <skos:definition xml:lang="en">a small crater-shape depression in a karst area</skos:definition>
    <skos:inScheme rdf:resource="http://www.geonames.org/ontology#T"/>
    <skos:prefLabel xml:lang="en">sinkhole</skos:prefLabel>
  </gn:Code>

  <gn:Code rdf:about="http://www.geonames.org/ontology#T.SLID">
    <skos:definition xml:lang="en">a mound of earth material, at the base of a slope and the associated scoured area</skos:definition>
    <skos:inScheme rdf:resource="http://www.geonames.org/ontology#T"/>
    <skos:prefLabel xml:lang="en">slide</skos:prefLabel>
  </gn:Code>

  <gn:Code rdf:about="http://www.geonames.org/ontology#T.SLP">
    <skos:definition xml:lang="en">a surface with a relatively uniform slope angle</skos:definition>
    <skos:inScheme rdf:resource="http://www.geonames.org/ontology#T"/>
    <skos:prefLabel xml:lang="en">slope(s)</skos:prefLabel>
  </gn:Code>

  <gn:Code rdf:about="http://www.geonames.org/ontology#T.SPIT">
    <skos:definition xml:lang="en">a narrow, straight or curved continuation of a beach into a waterbody</skos:definition>
    <skos:inScheme rdf:resource="http://www.geonames.org/ontology#T"/>
    <skos:prefLabel xml:lang="en">spit</skos:prefLabel>
  </gn:Code>

  <gn:Code rdf:about="http://www.geonames.org/ontology#T.SPUR">
    <skos:definition xml:lang="en">a subordinate ridge projecting outward from a hill, mountain or other elevation</skos:definition>
    <skos:inScheme rdf:resource="http://www.geonames.org/ontology#T"/>
    <skos:prefLabel xml:lang="en">spur(s)</skos:prefLabel>
  </gn:Code>

  <gn:Code rdf:about="http://www.geonames.org/ontology#T.TAL">
    <skos:definition xml:lang="en">a steep concave slope formed by an accumulation of loose rock fragments at the base of a cliff or steep slope</skos:definition>
    <skos:inScheme rdf:resource="http://www.geonames.org/ontology#T"/>
    <skos:prefLabel xml:lang="en">talus slope</skos:prefLabel>
  </gn:Code>

  <gn:Code rdf:about="http://www.geonames.org/ontology#T.TRGD">
    <skos:definition xml:lang="en">a long wind-swept trough between parallel longitudinal dunes</skos:definition>
    <skos:inScheme rdf:resource="http://www.geonames.org/ontology#T"/>
    <skos:prefLabel xml:lang="en">interdune trough(s)</skos:prefLabel>
  </gn:Code>

  <gn:Code rdf:about="http://www.geonames.org/ontology#T.TRR">
    <skos:definition xml:lang="en">a long, narrow alluvial platform bounded by steeper slopes above and below, usually overlooking a waterbody</skos:definition>
    <skos:inScheme rdf:resource="http://www.geonames.org/ontology#T"/>
    <skos:prefLabel xml:lang="en">terrace</skos:prefLabel>
  </gn:Code>

  <gn:Code rdf:about="http://www.geonames.org/ontology#T.UPLD">
    <skos:definition xml:lang="en">an extensive interior region of high land with low to moderate surface relief</skos:definition>
    <skos:inScheme rdf:resource="http://www.geonames.org/ontology#T"/>
    <skos:prefLabel xml:lang="en">upland</skos:prefLabel>
  </gn:Code>

  <gn:Code rdf:about="http://www.geonames.org/ontology#T.VAL">
    <skos:definition xml:lang="en">an elongated depression usually traversed by a stream</skos:definition>
    <skos:inScheme rdf:resource="http://www.geonames.org/ontology#T"/>
    <skos:prefLabel xml:lang="en">valley</skos:prefLabel>
  </gn:Code>

  <gn:Code rdf:about="http://www.geonames.org/ontology#T.VALG">
    <skos:definition xml:lang="en">a valley the floor of which is notably higher than the valley or shore to which it leads; most common in areas that have been glaciated</skos:definition>
    <skos:inScheme rdf:resource="http://www.geonames.org/ontology#T"/>
    <skos:prefLabel xml:lang="en">hanging valley</skos:prefLabel>
  </gn:Code>

  <gn:Code rdf:about="http://www.geonames.org/ontology#T.VALS">
    <skos:definition xml:lang="en">elongated depressions usually traversed by a stream</skos:definition>
    <skos:inScheme rdf:resource="http://www.geonames.org/ontology#T"/>
    <skos:prefLabel xml:lang="en">valleys</skos:prefLabel>
  </gn:Code>

  <gn:Code rdf:about="http://www.geonames.org/ontology#T.VALX">
    <skos:definition xml:lang="en">_</skos:definition>
    <skos:inScheme rdf:resource="http://www.geonames.org/ontology#T"/>
    <skos:prefLabel xml:lang="en">section of valley</skos:prefLabel>
  </gn:Code>

  <gn:Code rdf:about="http://www.geonames.org/ontology#T.VLC">
    <skos:definition xml:lang="en">a conical elevation composed of volcanic materials with a crater at the top</skos:definition>
    <skos:inScheme rdf:resource="http://www.geonames.org/ontology#T"/>
    <skos:prefLabel xml:lang="en">volcano</skos:prefLabel>
  </gn:Code>

  <gn:Class rdf:about="http://www.geonames.org/ontology#U">
    <rdfs:comment xml:lang="en">undersea</rdfs:comment>
  </gn:Class>

  <gn:Code rdf:about="http://www.geonames.org/ontology#U.APNU">
    <skos:definition xml:lang="en">a gentle slope, with a generally smooth surface, particularly found around groups of islands and seamounts</skos:definition>
    <skos:inScheme rdf:resource="http://www.geonames.org/ontology#U"/>
    <skos:prefLabel xml:lang="en">apron</skos:prefLabel>
  </gn:Code>

  <gn:Code rdf:about="http://www.geonames.org/ontology#U.ARCU">
    <skos:definition xml:lang="en">a low bulge around the southeastern end of the island of Hawaii</skos:definition>
    <skos:inScheme rdf:resource="http://www.geonames.org/ontology#U"/>
    <skos:prefLabel xml:lang="en">arch</skos:prefLabel>
  </gn:Code>

  <gn:Code rdf:about="http://www.geonames.org/ontology#U.ARRU">
    <skos:definition xml:lang="en">an area of subdued corrugations off Baja California</skos:definition>
    <skos:inScheme rdf:resource="http://www.geonames.org/ontology#U"/>
    <skos:prefLabel xml:lang="en">arrugado</skos:prefLabel>
  </gn:Code>

  <gn:Code rdf:about="http://www.geonames.org/ontology#U.BDLU">
    <skos:definition xml:lang="en">a region adjacent to a continent, normally occupied by or bordering a shelf, that is highly irregular with depths well in excess of those typical of a shelf</skos:definition>
    <skos:inScheme rdf:resource="http://www.geonames.org/ontology#U"/>
    <skos:prefLabel xml:lang="en">borderland</skos:prefLabel>
  </gn:Code>

  <gn:Code rdf:about="http://www.geonames.org/ontology#U.BKSU">
    <skos:definition xml:lang="en">elevations, typically located on a shelf, over which the depth of water is relatively shallow but sufficient for safe surface navigation</skos:definition>
    <skos:inScheme rdf:resource="http://www.geonames.org/ontology#U"/>
    <skos:prefLabel xml:lang="en">banks</skos:prefLabel>
  </gn:Code>

  <gn:Code rdf:about="http://www.geonames.org/ontology#U.BNCU">
    <skos:definition xml:lang="en">a small terrace</skos:definition>
    <skos:inScheme rdf:resource="http://www.geonames.org/ontology#U"/>
    <skos:prefLabel xml:lang="en">bench</skos:prefLabel>
  </gn:Code>

  <gn:Code rdf:about="http://www.geonames.org/ontology#U.BNKU">
    <skos:definition xml:lang="en">an elevation, typically located on a shelf, over which the depth of water is relatively shallow but sufficient for safe surface navigation</skos:definition>
    <skos:inScheme rdf:resource="http://www.geonames.org/ontology#U"/>
    <skos:prefLabel xml:lang="en">bank</skos:prefLabel>
  </gn:Code>

  <gn:Code rdf:about="http://www.geonames.org/ontology#U.BSNU">
    <skos:definition xml:lang="en">a depression more or less equidimensional in plan and of variable extent</skos:definition>
    <skos:inScheme rdf:resource="http://www.geonames.org/ontology#U"/>
    <skos:prefLabel xml:lang="en">basin</skos:prefLabel>
  </gn:Code>

  <gn:Code rdf:about="http://www.geonames.org/ontology#U.CDAU">
    <skos:definition xml:lang="en">an entire mountain system including the subordinate ranges, interior plateaus, and basins</skos:definition>
    <skos:inScheme rdf:resource="http://www.geonames.org/ontology#U"/>
    <skos:prefLabel xml:lang="en">cordillera</skos:prefLabel>
  </gn:Code>

  <gn:Code rdf:about="http://www.geonames.org/ontology#U.CNSU">
    <skos:definition xml:lang="en">relatively narrow, deep depressions with steep sides, the bottom of which generally has a continuous slope</skos:definition>
    <skos:inScheme rdf:resource="http://www.geonames.org/ontology#U"/>
    <skos:prefLabel xml:lang="en">canyons</skos:prefLabel>
  </gn:Code>

  <gn:Code rdf:about="http://www.geonames.org/ontology#U.CNYU">
    <skos:definition xml:lang="en">a relatively narrow, deep depression with steep sides, the bottom of which generally has a continuous slope</skos:definition>
    <skos:inScheme rdf:resource="http://www.geonames.org/ontology#U"/>
    <skos:prefLabel xml:lang="en">canyon</skos:prefLabel>
  </gn:Code>

  <gn:Code rdf:about="http://www.geonames.org/ontology#U.CRSU">
    <skos:definition xml:lang="en">a gentle slope rising from oceanic depths towards the foot of a continental slope</skos:definition>
    <skos:inScheme rdf:resource="http://www.geonames.org/ontology#U"/>
    <skos:prefLabel xml:lang="en">continental rise</skos:prefLabel>
  </gn:Code>

  <gn:Code rdf:about="http://www.geonames.org/ontology#U.DEPU">
    <skos:definition xml:lang="en">a localized deep area within the confines of a larger feature, such as a trough, basin or trench</skos:definition>
    <skos:inScheme rdf:resource="http://www.geonames.org/ontology#U"/>
    <skos:prefLabel xml:lang="en">deep</skos:prefLabel>
  </gn:Code>

  <gn:Code rdf:about="http://www.geonames.org/ontology#U.EDGU">
    <skos:definition xml:lang="en">a line along which there is a marked increase of slope at the outer margin of a continental shelf or island shelf</skos:definition>
    <skos:inScheme rdf:resource="http://www.geonames.org/ontology#U"/>
    <skos:prefLabel xml:lang="en">shelf edge</skos:prefLabel>
  </gn:Code>

  <gn:Code rdf:about="http://www.geonames.org/ontology#U.ESCU">
    <skos:definition xml:lang="en">an elongated and comparatively steep slope separating flat or gently sloping areas</skos:definition>
    <skos:inScheme rdf:resource="http://www.geonames.org/ontology#U"/>
    <skos:prefLabel xml:lang="en">escarpment (or scarp)</skos:prefLabel>
  </gn:Code>

  <gn:Code rdf:about="http://www.geonames.org/ontology#U.FANU">
    <skos:definition xml:lang="en">a relatively smooth feature normally sloping away from the lower termination of a canyon or canyon system</skos:definition>
    <skos:inScheme rdf:resource="http://www.geonames.org/ontology#U"/>
    <skos:prefLabel xml:lang="en">fan</skos:prefLabel>
  </gn:Code>

  <gn:Code rdf:about="http://www.geonames.org/ontology#U.FLTU">
    <skos:definition xml:lang="en">a small level or nearly level area</skos:definition>
    <skos:inScheme rdf:resource="http://www.geonames.org/ontology#U"/>
    <skos:prefLabel xml:lang="en">flat</skos:prefLabel>
  </gn:Code>

  <gn:Code rdf:about="http://www.geonames.org/ontology#U.FRKU">
    <skos:definition xml:lang="en">a branch of a canyon or valley</skos:definition>
    <skos:inScheme rdf:resource="http://www.geonames.org/ontology#U"/>
    <skos:prefLabel xml:lang="en">fork</skos:prefLabel>
  </gn:Code>

  <gn:Code rdf:about="http://www.geonames.org/ontology#U.FRSU">
    <skos:definition xml:lang="en">a branch of a canyon or valley</skos:definition>
    <skos:inScheme rdf:resource="http://www.geonames.org/ontology#U"/>
    <skos:prefLabel xml:lang="en">forks</skos:prefLabel>
  </gn:Code>

  <gn:Code rdf:about="http://www.geonames.org/ontology#U.FRZU">
    <skos:definition xml:lang="en">an extensive linear zone of irregular topography of the sea floor, characterized by steep-sided or asymmetrical ridges, troughs, or escarpments</skos:definition>
    <skos:inScheme rdf:resource="http://www.geonames.org/ontology#U"/>
    <skos:prefLabel xml:lang="en">fracture zone</skos:prefLabel>
  </gn:Code>

  <gn:Code rdf:about="http://www.geonames.org/ontology#U.FURU">
    <skos:definition xml:lang="en">a closed, linear, narrow, shallow depression</skos:definition>
    <skos:inScheme rdf:resource="http://www.geonames.org/ontology#U"/>
    <skos:prefLabel xml:lang="en">furrow</skos:prefLabel>
  </gn:Code>

  <gn:Code rdf:about="http://www.geonames.org/ontology#U.GAPU">
    <skos:definition xml:lang="en">a narrow break in a ridge or rise</skos:definition>
    <skos:inScheme rdf:resource="http://www.geonames.org/ontology#U"/>
    <skos:prefLabel xml:lang="en">gap</skos:prefLabel>
  </gn:Code>

  <gn:Code rdf:about="http://www.geonames.org/ontology#U.GLYU">
    <skos:definition xml:lang="en">a small valley-like feature</skos:definition>
    <skos:inScheme rdf:resource="http://www.geonames.org/ontology#U"/>
    <skos:prefLabel xml:lang="en">gully</skos:prefLabel>
  </gn:Code>

  <gn:Code rdf:about="http://www.geonames.org/ontology#U.HLLU">
    <skos:definition xml:lang="en">an elevation rising generally less than 500 meters</skos:definition>
    <skos:inScheme rdf:resource="http://www.geonames.org/ontology#U"/>
    <skos:prefLabel xml:lang="en">hill</skos:prefLabel>
  </gn:Code>

  <gn:Code rdf:about="http://www.geonames.org/ontology#U.HLSU">
    <skos:definition xml:lang="en">elevations rising generally less than 500 meters</skos:definition>
    <skos:inScheme rdf:resource="http://www.geonames.org/ontology#U"/>
    <skos:prefLabel xml:lang="en">hills</skos:prefLabel>
  </gn:Code>

  <gn:Code rdf:about="http://www.geonames.org/ontology#U.HOLU">
    <skos:definition xml:lang="en">a small depression of the sea floor</skos:definition>
    <skos:inScheme rdf:resource="http://www.geonames.org/ontology#U"/>
    <skos:prefLabel xml:lang="en">hole</skos:prefLabel>
  </gn:Code>

  <gn:Code rdf:about="http://www.geonames.org/ontology#U.KNLU">
    <skos:definition xml:lang="en">an elevation rising generally more than 500 meters and less than 1,000 meters and of limited extent across the summit</skos:definition>
    <skos:inScheme rdf:resource="http://www.geonames.org/ontology#U"/>
    <skos:prefLabel xml:lang="en">knoll</skos:prefLabel>
  </gn:Code>

  <gn:Code rdf:about="http://www.geonames.org/ontology#U.KNSU">
    <skos:definition xml:lang="en">elevations rising generally more than 500 meters and less than 1,000 meters and of limited extent across the summits</skos:definition>
    <skos:inScheme rdf:resource="http://www.geonames.org/ontology#U"/>
    <skos:prefLabel xml:lang="en">knolls</skos:prefLabel>
  </gn:Code>

  <gn:Code rdf:about="http://www.geonames.org/ontology#U.LDGU">
    <skos:definition xml:lang="en">a rocky projection or outcrop, commonly linear and near shore</skos:definition>
    <skos:inScheme rdf:resource="http://www.geonames.org/ontology#U"/>
    <skos:prefLabel xml:lang="en">ledge</skos:prefLabel>
  </gn:Code>

  <gn:Code rdf:about="http://www.geonames.org/ontology#U.LEVU">
    <skos:definition xml:lang="en">an embankment bordering a canyon, valley, or seachannel</skos:definition>
    <skos:inScheme rdf:resource="http://www.geonames.org/ontology#U"/>
    <skos:prefLabel xml:lang="en">levee</skos:prefLabel>
  </gn:Code>

  <gn:Code rdf:about="http://www.geonames.org/ontology#U.MDVU">
    <skos:definition xml:lang="en">the axial depression of the mid-oceanic ridge system</skos:definition>
    <skos:inScheme rdf:resource="http://www.geonames.org/ontology#U"/>
    <skos:prefLabel xml:lang="en">median valley</skos:prefLabel>
  </gn:Code>

  <gn:Code rdf:about="http://www.geonames.org/ontology#U.MESU">
    <skos:definition xml:lang="en">an isolated, extensive, flat-topped elevation on the shelf, with relatively steep sides</skos:definition>
    <skos:inScheme rdf:resource="http://www.geonames.org/ontology#U"/>
    <skos:prefLabel xml:lang="en">mesa</skos:prefLabel>
  </gn:Code>

  <gn:Code rdf:about="http://www.geonames.org/ontology#U.MNDU">
    <skos:definition xml:lang="en">a low, isolated, rounded hill</skos:definition>
    <skos:inScheme rdf:resource="http://www.geonames.org/ontology#U"/>
    <skos:prefLabel xml:lang="en">mound</skos:prefLabel>
  </gn:Code>

  <gn:Code rdf:about="http://www.geonames.org/ontology#U.MOTU">
    <skos:definition xml:lang="en">an annular depression that may not be continuous, located at the base of many seamounts, islands, and other isolated elevations</skos:definition>
    <skos:inScheme rdf:resource="http://www.geonames.org/ontology#U"/>
    <skos:prefLabel xml:lang="en">moat</skos:prefLabel>
  </gn:Code>

  <gn:Code rdf:about="http://www.geonames.org/ontology#U.MTSU">
    <skos:definition xml:lang="en">well-delineated subdivisions of a large and complex positive feature</skos:definition>
    <skos:inScheme rdf:resource="http://www.geonames.org/ontology#U"/>
    <skos:prefLabel xml:lang="en">mountains</skos:prefLabel>
  </gn:Code>

  <gn:Code rdf:about="http://www.geonames.org/ontology#U.MTU">
    <skos:definition xml:lang="en">a well-delineated subdivision of a large and complex positive feature</skos:definition>
    <skos:inScheme rdf:resource="http://www.geonames.org/ontology#U"/>
    <skos:prefLabel xml:lang="en">mountain</skos:prefLabel>
  </gn:Code>

  <gn:Code rdf:about="http://www.geonames.org/ontology#U.PKSU">
    <skos:definition xml:lang="en">prominent elevations, part of a larger feature, either pointed or of very limited extent across the summit</skos:definition>
    <skos:inScheme rdf:resource="http://www.geonames.org/ontology#U"/>
    <skos:prefLabel xml:lang="en">peaks</skos:prefLabel>
  </gn:Code>

  <gn:Code rdf:about="http://www.geonames.org/ontology#U.PKU">
    <skos:definition xml:lang="en">a prominent elevation, part of a larger feature, either pointed or of very limited extent across the summit</skos:definition>
    <skos:inScheme rdf:resource="http://www.geonames.org/ontology#U"/>
    <skos:prefLabel xml:lang="en">peak</skos:prefLabel>
  </gn:Code>

  <gn:Code rdf:about="http://www.geonames.org/ontology#U.PLFU">
    <skos:definition xml:lang="en">a flat or gently sloping underwater surface extending seaward from the shore</skos:definition>
    <skos:inScheme rdf:resource="http://www.geonames.org/ontology#U"/>
    <skos:prefLabel xml:lang="en">platform</skos:prefLabel>
  </gn:Code>

  <gn:Code rdf:about="http://www.geonames.org/ontology#U.PLNU">
    <skos:definition xml:lang="en">a flat, gently sloping or nearly level region</skos:definition>
    <skos:inScheme rdf:resource="http://www.geonames.org/ontology#U"/>
    <skos:prefLabel xml:lang="en">plain</skos:prefLabel>
  </gn:Code>

  <gn:Code rdf:about="http://www.geonames.org/ontology#U.PLTU">
    <skos:definition xml:lang="en">a comparatively flat-topped feature of considerable extent, dropping off abruptly on one or more sides</skos:definition>
    <skos:inScheme rdf:resource="http://www.geonames.org/ontology#U"/>
    <skos:prefLabel xml:lang="en">plateau</skos:prefLabel>
  </gn:Code>

  <gn:Code rdf:about="http://www.geonames.org/ontology#U.PNLU">
    <skos:definition xml:lang="en">a high tower or spire-shaped pillar of rock or coral, alone or cresting a summit</skos:definition>
    <skos:inScheme rdf:resource="http://www.geonames.org/ontology#U"/>
    <skos:prefLabel xml:lang="en">pinnacle</skos:prefLabel>
  </gn:Code>

  <gn:Code rdf:about="http://www.geonames.org/ontology#U.PRVU">
    <skos:definition xml:lang="en">a region identifiable by a group of similar physiographic features whose characteristics are markedly in contrast with surrounding areas</skos:definition>
    <skos:inScheme rdf:resource="http://www.geonames.org/ontology#U"/>
    <skos:prefLabel xml:lang="en">province</skos:prefLabel>
  </gn:Code>

  <gn:Code rdf:about="http://www.geonames.org/ontology#U.RAVU">
    <skos:definition xml:lang="en">a small canyon</skos:definition>
    <skos:inScheme rdf:resource="http://www.geonames.org/ontology#U"/>
    <skos:prefLabel xml:lang="en">ravine</skos:prefLabel>
  </gn:Code>

  <gn:Code rdf:about="http://www.geonames.org/ontology#U.RDGU">
    <skos:definition xml:lang="en">a long narrow elevation with steep sides</skos:definition>
    <skos:inScheme rdf:resource="http://www.geonames.org/ontology#U"/>
    <skos:prefLabel xml:lang="en">ridge</skos:prefLabel>
  </gn:Code>

  <gn:Code rdf:about="http://www.geonames.org/ontology#U.RDSU">
    <skos:definition xml:lang="en">long narrow elevations with steep sides</skos:definition>
    <skos:inScheme rdf:resource="http://www.geonames.org/ontology#U"/>
    <skos:prefLabel xml:lang="en">ridges</skos:prefLabel>
  </gn:Code>

  <gn:Code rdf:about="http://www.geonames.org/ontology#U.RFSU">
    <skos:definition xml:lang="en">surface-navigation hazards composed of consolidated material</skos:definition>
    <skos:inScheme rdf:resource="http://www.geonames.org/ontology#U"/>
    <skos:prefLabel xml:lang="en">reefs</skos:prefLabel>
  </gn:Code>

  <gn:Code rdf:about="http://www.geonames.org/ontology#U.RFU">
    <skos:definition xml:lang="en">a surface-navigation hazard composed of consolidated material</skos:definition>
    <skos:inScheme rdf:resource="http://www.geonames.org/ontology#U"/>
    <skos:prefLabel xml:lang="en">reef</skos:prefLabel>
  </gn:Code>

  <gn:Code rdf:about="http://www.geonames.org/ontology#U.RISU">
    <skos:definition xml:lang="en">a broad elevation that rises gently, and generally smoothly, from the sea floor</skos:definition>
    <skos:inScheme rdf:resource="http://www.geonames.org/ontology#U"/>
    <skos:prefLabel xml:lang="en">rise</skos:prefLabel>
  </gn:Code>

  <gn:Code rdf:about="http://www.geonames.org/ontology#U.RMPU">
    <skos:definition xml:lang="en">a gentle slope connecting areas of different elevations</skos:definition>
    <skos:inScheme rdf:resource="http://www.geonames.org/ontology#U"/>
    <skos:prefLabel xml:lang="en">ramp</skos:prefLabel>
  </gn:Code>

  <gn:Code rdf:about="http://www.geonames.org/ontology#U.RNGU">
    <skos:definition xml:lang="en">a series of associated ridges or seamounts</skos:definition>
    <skos:inScheme rdf:resource="http://www.geonames.org/ontology#U"/>
    <skos:prefLabel xml:lang="en">range</skos:prefLabel>
  </gn:Code>

  <gn:Code rdf:about="http://www.geonames.org/ontology#U.SCNU">
    <skos:definition xml:lang="en">a continuously sloping, elongated depression commonly found in fans or plains and customarily bordered by levees on one or two sides</skos:definition>
    <skos:inScheme rdf:resource="http://www.geonames.org/ontology#U"/>
    <skos:prefLabel xml:lang="en">seachannel</skos:prefLabel>
  </gn:Code>

  <gn:Code rdf:about="http://www.geonames.org/ontology#U.SCSU">
    <skos:definition xml:lang="en">continuously sloping, elongated depressions commonly found in fans or plains and customarily bordered by levees on one or two sides</skos:definition>
    <skos:inScheme rdf:resource="http://www.geonames.org/ontology#U"/>
    <skos:prefLabel xml:lang="en">seachannels</skos:prefLabel>
  </gn:Code>

  <gn:Code rdf:about="http://www.geonames.org/ontology#U.SDLU">
    <skos:definition xml:lang="en">a low part, resembling in shape a saddle, in a ridge or between contiguous seamounts</skos:definition>
    <skos:inScheme rdf:resource="http://www.geonames.org/ontology#U"/>
    <skos:prefLabel xml:lang="en">saddle</skos:prefLabel>
  </gn:Code>

  <gn:Code rdf:about="http://www.geonames.org/ontology#U.SHFU">
    <skos:definition xml:lang="en">a zone adjacent to a continent (or around an island) that extends from the low water line to a depth at which there is usually a marked increase of slope towards oceanic depths</skos:definition>
    <skos:inScheme rdf:resource="http://www.geonames.org/ontology#U"/>
    <skos:prefLabel xml:lang="en">shelf</skos:prefLabel>
  </gn:Code>

  <gn:Code rdf:about="http://www.geonames.org/ontology#U.SHLU">
    <skos:definition xml:lang="en">a surface-navigation hazard composed of unconsolidated material</skos:definition>
    <skos:inScheme rdf:resource="http://www.geonames.org/ontology#U"/>
    <skos:prefLabel xml:lang="en">shoal</skos:prefLabel>
  </gn:Code>

  <gn:Code rdf:about="http://www.geonames.org/ontology#U.SHSU">
    <skos:definition xml:lang="en">hazards to surface navigation composed of unconsolidated material</skos:definition>
    <skos:inScheme rdf:resource="http://www.geonames.org/ontology#U"/>
    <skos:prefLabel xml:lang="en">shoals</skos:prefLabel>
  </gn:Code>

  <gn:Code rdf:about="http://www.geonames.org/ontology#U.SHVU">
    <skos:definition xml:lang="en">a valley on the shelf, generally the shoreward extension of a canyon</skos:definition>
    <skos:inScheme rdf:resource="http://www.geonames.org/ontology#U"/>
    <skos:prefLabel xml:lang="en">shelf valley</skos:prefLabel>
  </gn:Code>

  <gn:Code rdf:about="http://www.geonames.org/ontology#U.SILU">
    <skos:definition xml:lang="en">the low part of a gap or saddle separating basins</skos:definition>
    <skos:inScheme rdf:resource="http://www.geonames.org/ontology#U"/>
    <skos:prefLabel xml:lang="en">sill</skos:prefLabel>
  </gn:Code>

  <gn:Code rdf:about="http://www.geonames.org/ontology#U.SLPU">
    <skos:definition xml:lang="en">the slope seaward from the shelf edge to the beginning of a continental rise or the point where there is a general reduction in slope</skos:definition>
    <skos:inScheme rdf:resource="http://www.geonames.org/ontology#U"/>
    <skos:prefLabel xml:lang="en">slope</skos:prefLabel>
  </gn:Code>

  <gn:Code rdf:about="http://www.geonames.org/ontology#U.SMSU">
    <skos:definition xml:lang="en">elevations rising generally more than 1,000 meters and of limited extent across the summit</skos:definition>
    <skos:inScheme rdf:resource="http://www.geonames.org/ontology#U"/>
    <skos:prefLabel xml:lang="en">seamounts</skos:prefLabel>
  </gn:Code>

  <gn:Code rdf:about="http://www.geonames.org/ontology#U.SMU">
    <skos:definition xml:lang="en">an elevation rising generally more than 1,000 meters and of limited extent across the summit</skos:definition>
    <skos:inScheme rdf:resource="http://www.geonames.org/ontology#U"/>
    <skos:prefLabel xml:lang="en">seamount</skos:prefLabel>
  </gn:Code>

  <gn:Code rdf:about="http://www.geonames.org/ontology#U.SPRU">
    <skos:definition xml:lang="en">a subordinate elevation, ridge, or rise projecting outward from a larger feature</skos:definition>
    <skos:inScheme rdf:resource="http://www.geonames.org/ontology#U"/>
    <skos:prefLabel xml:lang="en">spur</skos:prefLabel>
  </gn:Code>

  <gn:Code rdf:about="http://www.geonames.org/ontology#U.TERU">
    <skos:definition xml:lang="en">a relatively flat horizontal or gently inclined surface, sometimes long and narrow, which is bounded by a steeper ascending slope on one side and by a steep descending slope on the opposite side</skos:definition>
    <skos:inScheme rdf:resource="http://www.geonames.org/ontology#U"/>
    <skos:prefLabel xml:lang="en">terrace</skos:prefLabel>
  </gn:Code>

  <gn:Code rdf:about="http://www.geonames.org/ontology#U.TMSU">
    <skos:definition xml:lang="en">seamounts having a comparatively smooth, flat top</skos:definition>
    <skos:inScheme rdf:resource="http://www.geonames.org/ontology#U"/>
    <skos:prefLabel xml:lang="en">tablemounts (or guyots)</skos:prefLabel>
  </gn:Code>

  <gn:Code rdf:about="http://www.geonames.org/ontology#U.TMTU">
    <skos:definition xml:lang="en">a seamount having a comparatively smooth, flat top</skos:definition>
    <skos:inScheme rdf:resource="http://www.geonames.org/ontology#U"/>
    <skos:prefLabel xml:lang="en">tablemount (or guyot)</skos:prefLabel>
  </gn:Code>

  <gn:Code rdf:about="http://www.geonames.org/ontology#U.TNGU">
    <skos:definition xml:lang="en">an elongate (tongue-like) extension of a flat sea floor into an adjacent higher feature</skos:definition>
    <skos:inScheme rdf:resource="http://www.geonames.org/ontology#U"/>
    <skos:prefLabel xml:lang="en">tongue</skos:prefLabel>
  </gn:Code>

  <gn:Code rdf:about="http://www.geonames.org/ontology#U.TRGU">
    <skos:definition xml:lang="en">a long depression of the sea floor characteristically flat bottomed and steep sided, and normally shallower than a trench</skos:definition>
    <skos:inScheme rdf:resource="http://www.geonames.org/ontology#U"/>
    <skos:prefLabel xml:lang="en">trough</skos:prefLabel>
  </gn:Code>

  <gn:Code rdf:about="http://www.geonames.org/ontology#U.TRNU">
    <skos:definition xml:lang="en">a long, narrow, characteristically very deep and asymmetrical depression of the sea floor, with relatively steep sides</skos:definition>
    <skos:inScheme rdf:resource="http://www.geonames.org/ontology#U"/>
    <skos:prefLabel xml:lang="en">trench</skos:prefLabel>
  </gn:Code>

  <gn:Code rdf:about="http://www.geonames.org/ontology#U.VALU">
    <skos:definition xml:lang="en">a relatively shallow, wide depression, the bottom of which usually has a continuous gradient</skos:definition>
    <skos:inScheme rdf:resource="http://www.geonames.org/ontology#U"/>
    <skos:prefLabel xml:lang="en">valley</skos:prefLabel>
  </gn:Code>

  <gn:Code rdf:about="http://www.geonames.org/ontology#U.VLSU">
    <skos:definition xml:lang="en">a relatively shallow, wide depression, the bottom of which usually has a continuous gradient</skos:definition>
    <skos:inScheme rdf:resource="http://www.geonames.org/ontology#U"/>
    <skos:prefLabel xml:lang="en">valleys</skos:prefLabel>
  </gn:Code>

  <gn:Class rdf:about="http://www.geonames.org/ontology#V">
    <rdfs:comment xml:lang="en">forest, heath, ...</rdfs:comment>
  </gn:Class>

  <gn:Code rdf:about="http://www.geonames.org/ontology#V.BUSH">
    <skos:definition xml:lang="en">a small clump of conspicuous bushes in an otherwise bare area</skos:definition>
    <skos:inScheme rdf:resource="http://www.geonames.org/ontology#V"/>
    <skos:prefLabel xml:lang="en">bush(es)</skos:prefLabel>
  </gn:Code>

  <gn:Code rdf:about="http://www.geonames.org/ontology#V.CULT">
    <skos:definition xml:lang="en">an area under cultivation</skos:definition>
    <skos:inScheme rdf:resource="http://www.geonames.org/ontology#V"/>
    <skos:prefLabel xml:lang="en">cultivated area</skos:prefLabel>
  </gn:Code>

  <gn:Code rdf:about="http://www.geonames.org/ontology#V.FRST">
    <skos:definition xml:lang="en">an area dominated by tree vegetation</skos:definition>
    <skos:inScheme rdf:resource="http://www.geonames.org/ontology#V"/>
    <skos:prefLabel xml:lang="en">forest(s)</skos:prefLabel>
  </gn:Code>

  <gn:Code rdf:about="http://www.geonames.org/ontology#V.FRSTF">
    <skos:definition xml:lang="en">a forest fossilized by geologic processes and now exposed at the earth's surface</skos:definition>
    <skos:inScheme rdf:resource="http://www.geonames.org/ontology#V"/>
    <skos:prefLabel xml:lang="en">fossilized forest</skos:prefLabel>
  </gn:Code>

  <gn:Code rdf:about="http://www.geonames.org/ontology#V.GRSLD">
    <skos:definition xml:lang="en">an area dominated by grass vegetation</skos:definition>
    <skos:inScheme rdf:resource="http://www.geonames.org/ontology#V"/>
    <skos:prefLabel xml:lang="en">grassland</skos:prefLabel>
  </gn:Code>

  <gn:Code rdf:about="http://www.geonames.org/ontology#V.GRVC">
    <skos:definition xml:lang="en">a planting of coconut trees</skos:definition>
    <skos:inScheme rdf:resource="http://www.geonames.org/ontology#V"/>
    <skos:prefLabel xml:lang="en">coconut grove</skos:prefLabel>
  </gn:Code>

  <gn:Code rdf:about="http://www.geonames.org/ontology#V.GRVO">
    <skos:definition xml:lang="en">a planting of olive trees</skos:definition>
    <skos:inScheme rdf:resource="http://www.geonames.org/ontology#V"/>
    <skos:prefLabel xml:lang="en">olive grove</skos:prefLabel>
  </gn:Code>

  <gn:Code rdf:about="http://www.geonames.org/ontology#V.GRVP">
    <skos:definition xml:lang="en">a planting of palm trees</skos:definition>
    <skos:inScheme rdf:resource="http://www.geonames.org/ontology#V"/>
    <skos:prefLabel xml:lang="en">palm grove</skos:prefLabel>
  </gn:Code>

  <gn:Code rdf:about="http://www.geonames.org/ontology#V.GRVPN">
    <skos:definition xml:lang="en">a planting of pine trees</skos:definition>
    <skos:inScheme rdf:resource="http://www.geonames.org/ontology#V"/>
    <skos:prefLabel xml:lang="en">pine grove</skos:prefLabel>
  </gn:Code>

  <gn:Code rdf:about="http://www.geonames.org/ontology#V.HTH">
    <skos:definition xml:lang="en">an upland moor or sandy area dominated by low shrubby vegetation including heather</skos:definition>
    <skos:inScheme rdf:resource="http://www.geonames.org/ontology#V"/>
    <skos:prefLabel xml:lang="en">heath</skos:prefLabel>
  </gn:Code>

  <gn:Code rdf:about="http://www.geonames.org/ontology#V.MDW">
    <skos:definition xml:lang="en">a small, poorly drained area dominated by grassy vegetation</skos:definition>
    <skos:inScheme rdf:resource="http://www.geonames.org/ontology#V"/>
    <skos:prefLabel xml:lang="en">meadow</skos:prefLabel>
  </gn:Code>

  <gn:Code rdf:about="http://www.geonames.org/ontology#V.OCH">
    <skos:definition xml:lang="en">a planting of fruit or nut trees</skos:definition>
    <skos:inScheme rdf:resource="http://www.geonames.org/ontology#V"/>
    <skos:prefLabel xml:lang="en">orchard(s)</skos:prefLabel>
  </gn:Code>

  <gn:Code rdf:about="http://www.geonames.org/ontology#V.SCRB">
    <skos:definition xml:lang="en">an area of low trees, bushes, and shrubs stunted by some environmental limitation</skos:definition>
    <skos:inScheme rdf:resource="http://www.geonames.org/ontology#V"/>
    <skos:prefLabel xml:lang="en">scrubland</skos:prefLabel>
  </gn:Code>

  <gn:Code rdf:about="http://www.geonames.org/ontology#V.TREE">
    <skos:definition xml:lang="en">a conspicuous tree used as a landmark</skos:definition>
    <skos:inScheme rdf:resource="http://www.geonames.org/ontology#V"/>
    <skos:prefLabel xml:lang="en">tree(s)</skos:prefLabel>
  </gn:Code>

  <gn:Code rdf:about="http://www.geonames.org/ontology#V.TUND">
    <skos:definition xml:lang="en">a marshy, treeless, high latitude plain, dominated by mosses, lichens, and low shrub vegetation under permafrost conditions</skos:definition>
    <skos:inScheme rdf:resource="http://www.geonames.org/ontology#V"/>
    <skos:prefLabel xml:lang="en">tundra</skos:prefLabel>
  </gn:Code>

  <gn:Code rdf:about="http://www.geonames.org/ontology#V.VIN">
    <skos:definition xml:lang="en">a planting of grapevines</skos:definition>
    <skos:inScheme rdf:resource="http://www.geonames.org/ontology#V"/>
    <skos:prefLabel xml:lang="en">vineyard</skos:prefLabel>
  </gn:Code>

  <gn:Code rdf:about="http://www.geonames.org/ontology#V.VINS">
    <skos:definition xml:lang="en">plantings of grapevines</skos:definition>
    <skos:inScheme rdf:resource="http://www.geonames.org/ontology#V"/>
    <skos:prefLabel xml:lang="en">vineyards</skos:prefLabel>
  </gn:Code>
</rdf:RDF>
